code/ecdsa/dist/Hacl_Impl_Blake2_Constants.d
@@ -1,11 +1,14 @@
 ./Hacl_Impl_Blake2_Constants.o Hacl_Impl_Blake2_Constants.d : Hacl_Impl_Blake2_Constants.c \
- Hacl_Impl_Blake2_Constants.h kremlin/internal/types.h \
- kremlin/internal/kremlin/lowstar_endianness.h \
- kremlin/internal/fstar_uint128_gcc64.h kremlin/internal/FStar_UInt128.h \
- kremlin/internal/kremlib.h kremlin/internal/target.h \
- kremlin/internal/callconv.h kremlin/internal/builtin.h \
- kremlin/internal/debug.h kremlin/internal/types.h \
- kremlin/internal/fstar_int.h kremlin/internal/compat.h \
- kremlin/internal/FStar_UInt_8_16_32_64.h \
- kremlin/internal/LowStar_Endianness.h kremlin/lowstar_endianness.h \
- lib_intrinsics.h
+ Hacl_Impl_Blake2_Constants.h \
+ /home/nkulatov/new/everest/kremlin/include/kremlin/internal/types.h \
+ /home/nkulatov/new/everest/kremlin/include/kremlin/lowstar_endianness.h \
+ /home/nkulatov/new/everest/kremlin/kremlib/dist/minimal/fstar_uint128_gcc64.h \
+ /home/nkulatov/new/everest/kremlin/kremlib/dist/minimal/FStar_UInt128.h \
+ /home/nkulatov/new/everest/kremlin/include/kremlin/internal/compat.h \
+ /home/nkulatov/new/everest/kremlin/include/kremlin/internal/target.h \
+ /home/nkulatov/new/everest/kremlin/include/kremlin/internal/callconv.h \
+ /home/nkulatov/new/everest/kremlin/kremlib/dist/minimal/FStar_UInt_8_16_32_64.h \
+ /home/nkulatov/new/everest/kremlin/kremlib/dist/minimal/LowStar_Endianness.h \
+ ../../../lib/c/lib_intrinsics.h Hacl_IntTypes_Intrinsics.h \
+ ../../../lib/c/evercrypt_targetconfig.h ../../../lib/c/libintvector.h \
+ ../../../lib/c/libintvector_debug.h Hacl_Kremlib.h
