code/ecdsa/dist/Hacl_P256.c
@@ -57,6 +57,18 @@ static inline void copy_conditional_p384_l(uint64_t *out, uint64_t *x, uint64_t 
   }
 }
 
+static inline void copy_conditional_generic_l(uint64_t *out, uint64_t *x, uint64_t mask)
+{
+  uint32_t len = (uint32_t)4U;
+  for (uint32_t i = (uint32_t)0U; i < len; i++)
+  {
+    uint64_t x_i = x[i];
+    uint64_t out_i = out[i];
+    uint64_t r_i = out_i ^ (mask & (out_i ^ x_i));
+    out[i] = r_i;
+  }
+}
+
 static inline void copy_conditional_p256_c(uint64_t *out, const uint64_t *x, uint64_t mask)
 {
   uint32_t len = (uint32_t)4U;
@@ -136,7 +148,7 @@ static inline uint64_t
 bn_add_eq_len_u64(uint32_t aLen, uint64_t *a, uint64_t *b, uint64_t *res)
 {
   uint64_t c = (uint64_t)0U;
-  for (uint32_t i = (uint32_t)0U; i < aLen / (uint32_t)4U * (uint32_t)4U / (uint32_t)4U; i++)
+  for (uint32_t i = (uint32_t)0U; i < aLen / (uint32_t)4U; i++)
   {
     uint64_t t1 = a[(uint32_t)4U * i];
     uint64_t t20 = b[(uint32_t)4U * i];
@@ -190,7 +202,7 @@ static inline void felem_add_p256(uint64_t *a, uint64_t *b, uint64_t *out)
 {
   uint32_t len0 = (uint32_t)4U;
   uint64_t c0 = (uint64_t)0U;
-  for (uint32_t i = (uint32_t)0U; i < len0 / (uint32_t)4U * (uint32_t)4U / (uint32_t)4U; i++)
+  for (uint32_t i = (uint32_t)0U; i < len0 / (uint32_t)4U; i++)
   {
     uint64_t t1 = a[(uint32_t)4U * i];
     uint64_t t20 = b[(uint32_t)4U * i];
@@ -232,7 +244,7 @@ static inline void felem_add_p256(uint64_t *a, uint64_t *b, uint64_t *out)
     };
   uint32_t len1 = (uint32_t)4U;
   uint64_t c = (uint64_t)0U;
-  for (uint32_t i = (uint32_t)0U; i < len1 / (uint32_t)4U * (uint32_t)4U / (uint32_t)4U; i++)
+  for (uint32_t i = (uint32_t)0U; i < len1 / (uint32_t)4U; i++)
   {
     uint64_t t1 = out[(uint32_t)4U * i];
     uint64_t t20 = p[(uint32_t)4U * i];
@@ -273,7 +285,7 @@ static inline void felem_add_p384(uint64_t *a, uint64_t *b, uint64_t *out)
 {
   uint32_t len0 = (uint32_t)6U;
   uint64_t c0 = (uint64_t)0U;
-  for (uint32_t i = (uint32_t)0U; i < len0 / (uint32_t)4U * (uint32_t)4U / (uint32_t)4U; i++)
+  for (uint32_t i = (uint32_t)0U; i < len0 / (uint32_t)4U; i++)
   {
     uint64_t t1 = a[(uint32_t)4U * i];
     uint64_t t20 = b[(uint32_t)4U * i];
@@ -313,7 +325,7 @@ static inline void felem_add_p384(uint64_t *a, uint64_t *b, uint64_t *out)
     };
   uint32_t len1 = (uint32_t)6U;
   uint64_t c = (uint64_t)0U;
-  for (uint32_t i = (uint32_t)0U; i < len1 / (uint32_t)4U * (uint32_t)4U / (uint32_t)4U; i++)
+  for (uint32_t i = (uint32_t)0U; i < len1 / (uint32_t)4U; i++)
   {
     uint64_t t1 = out[(uint32_t)4U * i];
     uint64_t t20 = p[(uint32_t)4U * i];
@@ -354,7 +366,7 @@ static inline void felem_double_p256(uint64_t *arg1, uint64_t *out)
 {
   uint32_t len0 = (uint32_t)4U;
   uint64_t c0 = (uint64_t)0U;
-  for (uint32_t i = (uint32_t)0U; i < len0 / (uint32_t)4U * (uint32_t)4U / (uint32_t)4U; i++)
+  for (uint32_t i = (uint32_t)0U; i < len0 / (uint32_t)4U; i++)
   {
     uint64_t t1 = arg1[(uint32_t)4U * i];
     uint64_t t20 = arg1[(uint32_t)4U * i];
@@ -396,7 +408,7 @@ static inline void felem_double_p256(uint64_t *arg1, uint64_t *out)
     };
   uint32_t len1 = (uint32_t)4U;
   uint64_t c = (uint64_t)0U;
-  for (uint32_t i = (uint32_t)0U; i < len1 / (uint32_t)4U * (uint32_t)4U / (uint32_t)4U; i++)
+  for (uint32_t i = (uint32_t)0U; i < len1 / (uint32_t)4U; i++)
   {
     uint64_t t1 = out[(uint32_t)4U * i];
     uint64_t t20 = p[(uint32_t)4U * i];
@@ -437,7 +449,7 @@ static inline void felem_double_p384(uint64_t *arg1, uint64_t *out)
 {
   uint32_t len0 = (uint32_t)6U;
   uint64_t c0 = (uint64_t)0U;
-  for (uint32_t i = (uint32_t)0U; i < len0 / (uint32_t)4U * (uint32_t)4U / (uint32_t)4U; i++)
+  for (uint32_t i = (uint32_t)0U; i < len0 / (uint32_t)4U; i++)
   {
     uint64_t t1 = arg1[(uint32_t)4U * i];
     uint64_t t20 = arg1[(uint32_t)4U * i];
@@ -477,7 +489,7 @@ static inline void felem_double_p384(uint64_t *arg1, uint64_t *out)
     };
   uint32_t len1 = (uint32_t)6U;
   uint64_t c = (uint64_t)0U;
-  for (uint32_t i = (uint32_t)0U; i < len1 / (uint32_t)4U * (uint32_t)4U / (uint32_t)4U; i++)
+  for (uint32_t i = (uint32_t)0U; i < len1 / (uint32_t)4U; i++)
   {
     uint64_t t1 = out[(uint32_t)4U * i];
     uint64_t t20 = p[(uint32_t)4U * i];
@@ -518,7 +530,7 @@ static inline void felem_sub_p256(uint64_t *a, uint64_t *b, uint64_t *out)
 {
   uint32_t len = (uint32_t)4U;
   uint64_t c = (uint64_t)0U;
-  for (uint32_t i = (uint32_t)0U; i < len / (uint32_t)4U * (uint32_t)4U / (uint32_t)4U; i++)
+  for (uint32_t i = (uint32_t)0U; i < len / (uint32_t)4U; i++)
   {
     uint64_t t1 = a[(uint32_t)4U * i];
     uint64_t t20 = b[(uint32_t)4U * i];
@@ -564,7 +576,7 @@ static inline void felem_sub_p384(uint64_t *a, uint64_t *b, uint64_t *out)
 {
   uint32_t len = (uint32_t)6U;
   uint64_t c = (uint64_t)0U;
-  for (uint32_t i = (uint32_t)0U; i < len / (uint32_t)4U * (uint32_t)4U / (uint32_t)4U; i++)
+  for (uint32_t i = (uint32_t)0U; i < len / (uint32_t)4U; i++)
   {
     uint64_t t1 = a[(uint32_t)4U * i];
     uint64_t t20 = b[(uint32_t)4U * i];
@@ -658,7 +670,7 @@ static inline void reduction_prime_2prime_order_p256(uint64_t *x, uint64_t *resu
     };
   uint32_t len1 = (uint32_t)4U;
   uint64_t c = (uint64_t)0U;
-  for (uint32_t i = (uint32_t)0U; i < len1 / (uint32_t)4U * (uint32_t)4U / (uint32_t)4U; i++)
+  for (uint32_t i = (uint32_t)0U; i < len1 / (uint32_t)4U; i++)
   {
     uint64_t t1 = x[(uint32_t)4U * i];
     uint64_t t20 = p[(uint32_t)4U * i];
@@ -693,7 +705,7 @@ static inline void felem_add_ecdsa_P256(uint64_t *arg1, uint64_t *arg2, uint64_t
 {
   uint32_t len0 = (uint32_t)4U;
   uint64_t c0 = (uint64_t)0U;
-  for (uint32_t i = (uint32_t)0U; i < len0 / (uint32_t)4U * (uint32_t)4U / (uint32_t)4U; i++)
+  for (uint32_t i = (uint32_t)0U; i < len0 / (uint32_t)4U; i++)
   {
     uint64_t t1 = arg1[(uint32_t)4U * i];
     uint64_t t20 = arg2[(uint32_t)4U * i];
@@ -735,7 +747,7 @@ static inline void felem_add_ecdsa_P256(uint64_t *arg1, uint64_t *arg2, uint64_t
     };
   uint32_t len1 = (uint32_t)4U;
   uint64_t c = (uint64_t)0U;
-  for (uint32_t i = (uint32_t)0U; i < len1 / (uint32_t)4U * (uint32_t)4U / (uint32_t)4U; i++)
+  for (uint32_t i = (uint32_t)0U; i < len1 / (uint32_t)4U; i++)
   {
     uint64_t t1 = out[(uint32_t)4U * i];
     uint64_t t20 = p[(uint32_t)4U * i];
@@ -780,14 +792,13 @@ montgomery_multiplication_buffer_dh_p256(uint64_t *a, uint64_t *b, uint64_t *res
   uint64_t t[(uint32_t)2U * len];
   memset(t, 0U, (uint32_t)2U * len * sizeof (uint64_t));
   uint32_t len1 = (uint32_t)4U;
-  uint32_t resLen = len1 + len1;
-  memset(t, 0U, resLen * sizeof (uint64_t));
+  memset(t, 0U, (len1 + len1) * sizeof (uint64_t));
   for (uint32_t i0 = (uint32_t)0U; i0 < len1; i0++)
   {
     uint64_t bj = b[i0];
     uint64_t *res_j = t + i0;
     uint64_t c = (uint64_t)0U;
-    for (uint32_t i = (uint32_t)0U; i < len1 / (uint32_t)4U * (uint32_t)4U / (uint32_t)4U; i++)
+    for (uint32_t i = (uint32_t)0U; i < len1 / (uint32_t)4U; i++)
     {
       uint64_t a_i = a[(uint32_t)4U * i];
       uint64_t *res_i0 = res_j + (uint32_t)4U * i;
@@ -849,7 +860,7 @@ montgomery_multiplication_buffer_dh_p256(uint64_t *a, uint64_t *b, uint64_t *res
     mul64(f3, t10, o3, o4);
     uint32_t len32 = (uint32_t)4U * (uint32_t)2U;
     uint64_t c = (uint64_t)0U;
-    for (uint32_t i = (uint32_t)0U; i < len32 / (uint32_t)4U * (uint32_t)4U / (uint32_t)4U; i++)
+    for (uint32_t i = (uint32_t)0U; i < len32 / (uint32_t)4U; i++)
     {
       uint64_t t1 = t[(uint32_t)4U * i];
       uint64_t t210 = t2[(uint32_t)4U * i];
@@ -902,7 +913,7 @@ montgomery_multiplication_buffer_dh_p256(uint64_t *a, uint64_t *b, uint64_t *res
     };
   uint32_t len4 = (uint32_t)4U;
   uint64_t c = (uint64_t)0U;
-  for (uint32_t i = (uint32_t)0U; i < len4 / (uint32_t)4U * (uint32_t)4U / (uint32_t)4U; i++)
+  for (uint32_t i = (uint32_t)0U; i < len4 / (uint32_t)4U; i++)
   {
     uint64_t t1 = x_[(uint32_t)4U * i];
     uint64_t t210 = p[(uint32_t)4U * i];
@@ -947,14 +958,13 @@ montgomery_multiplication_buffer_dh_p384(uint64_t *a, uint64_t *b, uint64_t *res
   uint64_t t[(uint32_t)2U * len];
   memset(t, 0U, (uint32_t)2U * len * sizeof (uint64_t));
   uint32_t len1 = (uint32_t)6U;
-  uint32_t resLen0 = len1 + len1;
-  memset(t, 0U, resLen0 * sizeof (uint64_t));
+  memset(t, 0U, (len1 + len1) * sizeof (uint64_t));
   for (uint32_t i0 = (uint32_t)0U; i0 < len1; i0++)
   {
     uint64_t bj = b[i0];
     uint64_t *res_j = t + i0;
     uint64_t c = (uint64_t)0U;
-    for (uint32_t i = (uint32_t)0U; i < len1 / (uint32_t)4U * (uint32_t)4U / (uint32_t)4U; i++)
+    for (uint32_t i = (uint32_t)0U; i < len1 / (uint32_t)4U; i++)
     {
       uint64_t a_i = a[(uint32_t)4U * i];
       uint64_t *res_i0 = res_j + (uint32_t)4U * i;
@@ -1011,14 +1021,13 @@ montgomery_multiplication_buffer_dh_p384(uint64_t *a, uint64_t *b, uint64_t *res
     uint32_t len32 = (uint32_t)6U;
     uint64_t bBuffer = y_;
     uint64_t *partResult = t2;
-    uint32_t resLen = len32 + (uint32_t)1U;
-    memset(partResult, 0U, resLen * sizeof (uint64_t));
+    memset(partResult, 0U, (len32 + (uint32_t)1U) * sizeof (uint64_t));
     for (uint32_t i1 = (uint32_t)0U; i1 < (uint32_t)1U; i1++)
     {
       uint64_t bj = (&bBuffer)[i1];
       uint64_t *res_j = partResult + i1;
       uint64_t c = (uint64_t)0U;
-      for (uint32_t i = (uint32_t)0U; i < len32 / (uint32_t)4U * (uint32_t)4U / (uint32_t)4U; i++)
+      for (uint32_t i = (uint32_t)0U; i < len32 / (uint32_t)4U; i++)
       {
         uint64_t a_i = p[(uint32_t)4U * i];
         uint64_t *res_i0 = res_j + (uint32_t)4U * i;
@@ -1044,7 +1053,7 @@ montgomery_multiplication_buffer_dh_p384(uint64_t *a, uint64_t *b, uint64_t *res
     }
     uint32_t len33 = (uint32_t)6U * (uint32_t)2U;
     uint64_t c = (uint64_t)0U;
-    for (uint32_t i = (uint32_t)0U; i < len33 / (uint32_t)4U * (uint32_t)4U / (uint32_t)4U; i++)
+    for (uint32_t i = (uint32_t)0U; i < len33 / (uint32_t)4U; i++)
     {
       uint64_t t1 = t[(uint32_t)4U * i];
       uint64_t t210 = t2[(uint32_t)4U * i];
@@ -1095,7 +1104,7 @@ montgomery_multiplication_buffer_dh_p384(uint64_t *a, uint64_t *b, uint64_t *res
     };
   uint32_t len4 = (uint32_t)6U;
   uint64_t c = (uint64_t)0U;
-  for (uint32_t i = (uint32_t)0U; i < len4 / (uint32_t)4U * (uint32_t)4U / (uint32_t)4U; i++)
+  for (uint32_t i = (uint32_t)0U; i < len4 / (uint32_t)4U; i++)
   {
     uint64_t t1 = x_[(uint32_t)4U * i];
     uint64_t t210 = p[(uint32_t)4U * i];
@@ -1140,14 +1149,13 @@ montgomery_multiplication_buffer_dsa_p256(uint64_t *a, uint64_t *b, uint64_t *re
   uint64_t t[(uint32_t)2U * len];
   memset(t, 0U, (uint32_t)2U * len * sizeof (uint64_t));
   uint32_t len1 = (uint32_t)4U;
-  uint32_t resLen0 = len1 + len1;
-  memset(t, 0U, resLen0 * sizeof (uint64_t));
+  memset(t, 0U, (len1 + len1) * sizeof (uint64_t));
   for (uint32_t i0 = (uint32_t)0U; i0 < len1; i0++)
   {
     uint64_t bj = b[i0];
     uint64_t *res_j = t + i0;
     uint64_t c = (uint64_t)0U;
-    for (uint32_t i = (uint32_t)0U; i < len1 / (uint32_t)4U * (uint32_t)4U / (uint32_t)4U; i++)
+    for (uint32_t i = (uint32_t)0U; i < len1 / (uint32_t)4U; i++)
     {
       uint64_t a_i = a[(uint32_t)4U * i];
       uint64_t *res_i0 = res_j + (uint32_t)4U * i;
@@ -1206,14 +1214,13 @@ montgomery_multiplication_buffer_dsa_p256(uint64_t *a, uint64_t *b, uint64_t *re
     uint32_t len32 = (uint32_t)4U;
     uint64_t bBuffer = y_;
     uint64_t *partResult = t2;
-    uint32_t resLen = len32 + (uint32_t)1U;
-    memset(partResult, 0U, resLen * sizeof (uint64_t));
+    memset(partResult, 0U, (len32 + (uint32_t)1U) * sizeof (uint64_t));
     for (uint32_t i1 = (uint32_t)0U; i1 < (uint32_t)1U; i1++)
     {
       uint64_t bj = (&bBuffer)[i1];
       uint64_t *res_j = partResult + i1;
       uint64_t c = (uint64_t)0U;
-      for (uint32_t i = (uint32_t)0U; i < len32 / (uint32_t)4U * (uint32_t)4U / (uint32_t)4U; i++)
+      for (uint32_t i = (uint32_t)0U; i < len32 / (uint32_t)4U; i++)
       {
         uint64_t a_i = p[(uint32_t)4U * i];
         uint64_t *res_i0 = res_j + (uint32_t)4U * i;
@@ -1239,7 +1246,7 @@ montgomery_multiplication_buffer_dsa_p256(uint64_t *a, uint64_t *b, uint64_t *re
     }
     uint32_t len33 = (uint32_t)4U * (uint32_t)2U;
     uint64_t c = (uint64_t)0U;
-    for (uint32_t i = (uint32_t)0U; i < len33 / (uint32_t)4U * (uint32_t)4U / (uint32_t)4U; i++)
+    for (uint32_t i = (uint32_t)0U; i < len33 / (uint32_t)4U; i++)
     {
       uint64_t t1 = t[(uint32_t)4U * i];
       uint64_t t210 = t2[(uint32_t)4U * i];
@@ -1292,7 +1299,7 @@ montgomery_multiplication_buffer_dsa_p256(uint64_t *a, uint64_t *b, uint64_t *re
     };
   uint32_t len4 = (uint32_t)4U;
   uint64_t c = (uint64_t)0U;
-  for (uint32_t i = (uint32_t)0U; i < len4 / (uint32_t)4U * (uint32_t)4U / (uint32_t)4U; i++)
+  for (uint32_t i = (uint32_t)0U; i < len4 / (uint32_t)4U; i++)
   {
     uint64_t t1 = x_[(uint32_t)4U * i];
     uint64_t t210 = p[(uint32_t)4U * i];
@@ -1336,15 +1343,14 @@ static inline void montgomery_square_buffer_dh_p256(uint64_t *a, uint64_t *resul
   uint64_t t[(uint32_t)2U * len];
   memset(t, 0U, (uint32_t)2U * len * sizeof (uint64_t));
   uint32_t len1 = (uint32_t)4U;
-  uint32_t resLen = len1 + len1;
-  memset(t, 0U, resLen * sizeof (uint64_t));
+  memset(t, 0U, (len1 + len1) * sizeof (uint64_t));
   for (uint32_t i0 = (uint32_t)0U; i0 < len1; i0++)
   {
     uint64_t *ab = a;
     uint64_t a_j = a[i0];
     uint64_t *res_j = t + i0;
     uint64_t c = (uint64_t)0U;
-    for (uint32_t i = (uint32_t)0U; i < i0 / (uint32_t)4U * (uint32_t)4U / (uint32_t)4U; i++)
+    for (uint32_t i = (uint32_t)0U; i < i0 / (uint32_t)4U; i++)
     {
       uint64_t a_i = ab[(uint32_t)4U * i];
       uint64_t *res_i0 = res_j + (uint32_t)4U * i;
@@ -1368,10 +1374,10 @@ static inline void montgomery_square_buffer_dh_p256(uint64_t *a, uint64_t *resul
     uint64_t r = c;
     t[i0 + i0] = r;
   }
-  uint64_t c0 = bn_add_eq_len_u64(resLen, t, t, t);
-  KRML_CHECK_SIZE(sizeof (uint64_t), resLen);
-  uint64_t tmp[resLen];
-  memset(tmp, 0U, resLen * sizeof (uint64_t));
+  uint64_t c0 = bn_add_eq_len_u64(len1 + len1, t, t, t);
+  KRML_CHECK_SIZE(sizeof (uint64_t), len1 + len1);
+  uint64_t tmp[len1 + len1];
+  memset(tmp, 0U, (len1 + len1) * sizeof (uint64_t));
   for (uint32_t i = (uint32_t)0U; i < len1; i++)
   {
     uint128_t res = (uint128_t)a[i] * a[i];
@@ -1380,7 +1386,7 @@ static inline void montgomery_square_buffer_dh_p256(uint64_t *a, uint64_t *resul
     tmp[(uint32_t)2U * i] = lo;
     tmp[(uint32_t)2U * i + (uint32_t)1U] = hi;
   }
-  uint64_t c1 = bn_add_eq_len_u64(resLen, t, tmp, t);
+  uint64_t c1 = bn_add_eq_len_u64(len1 + len1, t, tmp, t);
   uint32_t len10 = (uint32_t)4U;
   KRML_CHECK_SIZE(sizeof (uint64_t), (uint32_t)2U * len10);
   uint64_t t2[(uint32_t)2U * len10];
@@ -1419,7 +1425,7 @@ static inline void montgomery_square_buffer_dh_p256(uint64_t *a, uint64_t *resul
     mul64(f3, t10, o3, o4);
     uint32_t len32 = (uint32_t)4U * (uint32_t)2U;
     uint64_t c = (uint64_t)0U;
-    for (uint32_t i = (uint32_t)0U; i < len32 / (uint32_t)4U * (uint32_t)4U / (uint32_t)4U; i++)
+    for (uint32_t i = (uint32_t)0U; i < len32 / (uint32_t)4U; i++)
     {
       uint64_t t1 = t[(uint32_t)4U * i];
       uint64_t t210 = t2[(uint32_t)4U * i];
@@ -1472,7 +1478,7 @@ static inline void montgomery_square_buffer_dh_p256(uint64_t *a, uint64_t *resul
     };
   uint32_t len4 = (uint32_t)4U;
   uint64_t c = (uint64_t)0U;
-  for (uint32_t i = (uint32_t)0U; i < len4 / (uint32_t)4U * (uint32_t)4U / (uint32_t)4U; i++)
+  for (uint32_t i = (uint32_t)0U; i < len4 / (uint32_t)4U; i++)
   {
     uint64_t t1 = x_[(uint32_t)4U * i];
     uint64_t t210 = p[(uint32_t)4U * i];
@@ -1516,15 +1522,14 @@ static inline void montgomery_square_buffer_dh_p384(uint64_t *a, uint64_t *resul
   uint64_t t[(uint32_t)2U * len];
   memset(t, 0U, (uint32_t)2U * len * sizeof (uint64_t));
   uint32_t len1 = (uint32_t)6U;
-  uint32_t resLen0 = len1 + len1;
-  memset(t, 0U, resLen0 * sizeof (uint64_t));
+  memset(t, 0U, (len1 + len1) * sizeof (uint64_t));
   for (uint32_t i0 = (uint32_t)0U; i0 < len1; i0++)
   {
     uint64_t *ab = a;
     uint64_t a_j = a[i0];
     uint64_t *res_j = t + i0;
     uint64_t c = (uint64_t)0U;
-    for (uint32_t i = (uint32_t)0U; i < i0 / (uint32_t)4U * (uint32_t)4U / (uint32_t)4U; i++)
+    for (uint32_t i = (uint32_t)0U; i < i0 / (uint32_t)4U; i++)
     {
       uint64_t a_i = ab[(uint32_t)4U * i];
       uint64_t *res_i0 = res_j + (uint32_t)4U * i;
@@ -1548,10 +1553,10 @@ static inline void montgomery_square_buffer_dh_p384(uint64_t *a, uint64_t *resul
     uint64_t r = c;
     t[i0 + i0] = r;
   }
-  uint64_t c0 = bn_add_eq_len_u64(resLen0, t, t, t);
-  KRML_CHECK_SIZE(sizeof (uint64_t), resLen0);
-  uint64_t tmp[resLen0];
-  memset(tmp, 0U, resLen0 * sizeof (uint64_t));
+  uint64_t c0 = bn_add_eq_len_u64(len1 + len1, t, t, t);
+  KRML_CHECK_SIZE(sizeof (uint64_t), len1 + len1);
+  uint64_t tmp[len1 + len1];
+  memset(tmp, 0U, (len1 + len1) * sizeof (uint64_t));
   for (uint32_t i = (uint32_t)0U; i < len1; i++)
   {
     uint128_t res = (uint128_t)a[i] * a[i];
@@ -1560,7 +1565,7 @@ static inline void montgomery_square_buffer_dh_p384(uint64_t *a, uint64_t *resul
     tmp[(uint32_t)2U * i] = lo;
     tmp[(uint32_t)2U * i + (uint32_t)1U] = hi;
   }
-  uint64_t c1 = bn_add_eq_len_u64(resLen0, t, tmp, t);
+  uint64_t c1 = bn_add_eq_len_u64(len1 + len1, t, tmp, t);
   uint32_t len10 = (uint32_t)6U;
   KRML_CHECK_SIZE(sizeof (uint64_t), (uint32_t)2U * len10);
   uint64_t t2[(uint32_t)2U * len10];
@@ -1594,14 +1599,13 @@ static inline void montgomery_square_buffer_dh_p384(uint64_t *a, uint64_t *resul
     uint32_t len32 = (uint32_t)6U;
     uint64_t bBuffer = y_;
     uint64_t *partResult = t2;
-    uint32_t resLen = len32 + (uint32_t)1U;
-    memset(partResult, 0U, resLen * sizeof (uint64_t));
+    memset(partResult, 0U, (len32 + (uint32_t)1U) * sizeof (uint64_t));
     for (uint32_t i1 = (uint32_t)0U; i1 < (uint32_t)1U; i1++)
     {
       uint64_t bj = (&bBuffer)[i1];
       uint64_t *res_j = partResult + i1;
       uint64_t c = (uint64_t)0U;
-      for (uint32_t i = (uint32_t)0U; i < len32 / (uint32_t)4U * (uint32_t)4U / (uint32_t)4U; i++)
+      for (uint32_t i = (uint32_t)0U; i < len32 / (uint32_t)4U; i++)
       {
         uint64_t a_i = p[(uint32_t)4U * i];
         uint64_t *res_i0 = res_j + (uint32_t)4U * i;
@@ -1627,7 +1631,7 @@ static inline void montgomery_square_buffer_dh_p384(uint64_t *a, uint64_t *resul
     }
     uint32_t len33 = (uint32_t)6U * (uint32_t)2U;
     uint64_t c = (uint64_t)0U;
-    for (uint32_t i = (uint32_t)0U; i < len33 / (uint32_t)4U * (uint32_t)4U / (uint32_t)4U; i++)
+    for (uint32_t i = (uint32_t)0U; i < len33 / (uint32_t)4U; i++)
     {
       uint64_t t1 = t[(uint32_t)4U * i];
       uint64_t t210 = t2[(uint32_t)4U * i];
@@ -1678,7 +1682,7 @@ static inline void montgomery_square_buffer_dh_p384(uint64_t *a, uint64_t *resul
     };
   uint32_t len4 = (uint32_t)6U;
   uint64_t c = (uint64_t)0U;
-  for (uint32_t i = (uint32_t)0U; i < len4 / (uint32_t)4U * (uint32_t)4U / (uint32_t)4U; i++)
+  for (uint32_t i = (uint32_t)0U; i < len4 / (uint32_t)4U; i++)
   {
     uint64_t t1 = x_[(uint32_t)4U * i];
     uint64_t t210 = p[(uint32_t)4U * i];
@@ -1745,14 +1749,13 @@ montgomery_ladder_power_p256_dsa(uint64_t *a, const uint8_t *scalar, uint64_t *r
     uint64_t t[(uint32_t)2U * len11];
     memset(t, 0U, (uint32_t)2U * len11 * sizeof (uint64_t));
     uint32_t len20 = (uint32_t)4U;
-    uint32_t resLen0 = len20 + len20;
-    memset(t, 0U, resLen0 * sizeof (uint64_t));
+    memset(t, 0U, (len20 + len20) * sizeof (uint64_t));
     for (uint32_t i1 = (uint32_t)0U; i1 < len20; i1++)
     {
       uint64_t bj = a[i1];
       uint64_t *res_j = t + i1;
       uint64_t c = (uint64_t)0U;
-      for (uint32_t i = (uint32_t)0U; i < len20 / (uint32_t)4U * (uint32_t)4U / (uint32_t)4U; i++)
+      for (uint32_t i = (uint32_t)0U; i < len20 / (uint32_t)4U; i++)
       {
         uint64_t a_i = p[(uint32_t)4U * i];
         uint64_t *res_i0 = res_j + (uint32_t)4U * i;
@@ -1811,14 +1814,13 @@ montgomery_ladder_power_p256_dsa(uint64_t *a, const uint8_t *scalar, uint64_t *r
       uint32_t len42 = (uint32_t)4U;
       uint64_t bBuffer = y_;
       uint64_t *partResult = t20;
-      uint32_t resLen = len42 + (uint32_t)1U;
-      memset(partResult, 0U, resLen * sizeof (uint64_t));
+      memset(partResult, 0U, (len42 + (uint32_t)1U) * sizeof (uint64_t));
       for (uint32_t i2 = (uint32_t)0U; i2 < (uint32_t)1U; i2++)
       {
         uint64_t bj = (&bBuffer)[i2];
         uint64_t *res_j = partResult + i2;
         uint64_t c = (uint64_t)0U;
-        for (uint32_t i = (uint32_t)0U; i < len42 / (uint32_t)4U * (uint32_t)4U / (uint32_t)4U; i++)
+        for (uint32_t i = (uint32_t)0U; i < len42 / (uint32_t)4U; i++)
         {
           uint64_t a_i = p1[(uint32_t)4U * i];
           uint64_t *res_i0 = res_j + (uint32_t)4U * i;
@@ -1844,7 +1846,7 @@ montgomery_ladder_power_p256_dsa(uint64_t *a, const uint8_t *scalar, uint64_t *r
       }
       uint32_t len43 = (uint32_t)4U * (uint32_t)2U;
       uint64_t c = (uint64_t)0U;
-      for (uint32_t i = (uint32_t)0U; i < len43 / (uint32_t)4U * (uint32_t)4U / (uint32_t)4U; i++)
+      for (uint32_t i = (uint32_t)0U; i < len43 / (uint32_t)4U; i++)
       {
         uint64_t t1 = t[(uint32_t)4U * i];
         uint64_t t210 = t20[(uint32_t)4U * i];
@@ -1897,7 +1899,7 @@ montgomery_ladder_power_p256_dsa(uint64_t *a, const uint8_t *scalar, uint64_t *r
       };
     uint32_t len50 = (uint32_t)4U;
     uint64_t c1 = (uint64_t)0U;
-    for (uint32_t i = (uint32_t)0U; i < len50 / (uint32_t)4U * (uint32_t)4U / (uint32_t)4U; i++)
+    for (uint32_t i = (uint32_t)0U; i < len50 / (uint32_t)4U; i++)
     {
       uint64_t t1 = x_0[(uint32_t)4U * i];
       uint64_t t210 = p10[(uint32_t)4U * i];
@@ -1937,15 +1939,14 @@ montgomery_ladder_power_p256_dsa(uint64_t *a, const uint8_t *scalar, uint64_t *r
     uint64_t t0[(uint32_t)2U * len12];
     memset(t0, 0U, (uint32_t)2U * len12 * sizeof (uint64_t));
     uint32_t len2 = (uint32_t)4U;
-    uint32_t resLen1 = len2 + len2;
-    memset(t0, 0U, resLen1 * sizeof (uint64_t));
+    memset(t0, 0U, (len2 + len2) * sizeof (uint64_t));
     for (uint32_t i1 = (uint32_t)0U; i1 < len2; i1++)
     {
       uint64_t *ab = p;
       uint64_t a_j = p[i1];
       uint64_t *res_j = t0 + i1;
       uint64_t c = (uint64_t)0U;
-      for (uint32_t i = (uint32_t)0U; i < i1 / (uint32_t)4U * (uint32_t)4U / (uint32_t)4U; i++)
+      for (uint32_t i = (uint32_t)0U; i < i1 / (uint32_t)4U; i++)
       {
         uint64_t a_i = ab[(uint32_t)4U * i];
         uint64_t *res_i0 = res_j + (uint32_t)4U * i;
@@ -1969,10 +1970,10 @@ montgomery_ladder_power_p256_dsa(uint64_t *a, const uint8_t *scalar, uint64_t *r
       uint64_t r0 = c;
       t0[i1 + i1] = r0;
     }
-    uint64_t c0 = bn_add_eq_len_u64(resLen1, t0, t0, t0);
-    KRML_CHECK_SIZE(sizeof (uint64_t), resLen1);
-    uint64_t tmp[resLen1];
-    memset(tmp, 0U, resLen1 * sizeof (uint64_t));
+    uint64_t c0 = bn_add_eq_len_u64(len2 + len2, t0, t0, t0);
+    KRML_CHECK_SIZE(sizeof (uint64_t), len2 + len2);
+    uint64_t tmp[len2 + len2];
+    memset(tmp, 0U, (len2 + len2) * sizeof (uint64_t));
     for (uint32_t i = (uint32_t)0U; i < len2; i++)
     {
       uint128_t res = (uint128_t)p[i] * p[i];
@@ -1981,7 +1982,7 @@ montgomery_ladder_power_p256_dsa(uint64_t *a, const uint8_t *scalar, uint64_t *r
       tmp[(uint32_t)2U * i] = lo;
       tmp[(uint32_t)2U * i + (uint32_t)1U] = hi;
     }
-    uint64_t c10 = bn_add_eq_len_u64(resLen1, t0, tmp, t0);
+    uint64_t c10 = bn_add_eq_len_u64(len2 + len2, t0, tmp, t0);
     uint32_t len22 = (uint32_t)4U;
     KRML_CHECK_SIZE(sizeof (uint64_t), (uint32_t)2U * len22);
     uint64_t t2[(uint32_t)2U * len22];
@@ -2017,14 +2018,13 @@ montgomery_ladder_power_p256_dsa(uint64_t *a, const uint8_t *scalar, uint64_t *r
       uint32_t len43 = (uint32_t)4U;
       uint64_t bBuffer = y_;
       uint64_t *partResult = t2;
-      uint32_t resLen = len43 + (uint32_t)1U;
-      memset(partResult, 0U, resLen * sizeof (uint64_t));
+      memset(partResult, 0U, (len43 + (uint32_t)1U) * sizeof (uint64_t));
       for (uint32_t i2 = (uint32_t)0U; i2 < (uint32_t)1U; i2++)
       {
         uint64_t bj = (&bBuffer)[i2];
         uint64_t *res_j = partResult + i2;
         uint64_t c = (uint64_t)0U;
-        for (uint32_t i = (uint32_t)0U; i < len43 / (uint32_t)4U * (uint32_t)4U / (uint32_t)4U; i++)
+        for (uint32_t i = (uint32_t)0U; i < len43 / (uint32_t)4U; i++)
         {
           uint64_t a_i = p1[(uint32_t)4U * i];
           uint64_t *res_i0 = res_j + (uint32_t)4U * i;
@@ -2050,7 +2050,7 @@ montgomery_ladder_power_p256_dsa(uint64_t *a, const uint8_t *scalar, uint64_t *r
       }
       uint32_t len44 = (uint32_t)4U * (uint32_t)2U;
       uint64_t c = (uint64_t)0U;
-      for (uint32_t i = (uint32_t)0U; i < len44 / (uint32_t)4U * (uint32_t)4U / (uint32_t)4U; i++)
+      for (uint32_t i = (uint32_t)0U; i < len44 / (uint32_t)4U; i++)
       {
         uint64_t t1 = t0[(uint32_t)4U * i];
         uint64_t t210 = t2[(uint32_t)4U * i];
@@ -2103,7 +2103,7 @@ montgomery_ladder_power_p256_dsa(uint64_t *a, const uint8_t *scalar, uint64_t *r
       };
     uint32_t len5 = (uint32_t)4U;
     uint64_t c = (uint64_t)0U;
-    for (uint32_t i = (uint32_t)0U; i < len5 / (uint32_t)4U * (uint32_t)4U / (uint32_t)4U; i++)
+    for (uint32_t i = (uint32_t)0U; i < len5 / (uint32_t)4U; i++)
     {
       uint64_t t1 = x_[(uint32_t)4U * i];
       uint64_t t210 = p1[(uint32_t)4U * i];
@@ -2344,7 +2344,7 @@ static inline void toUint64ChangeEndian_p384(uint8_t *i, uint64_t *o)
   }
 }
 
-static inline void montgomery_multiplication_buffer_by_one_mixed_p256(uint64_t *result)
+static void montgomery_multiplication_buffer_by_one_mixed_p256(uint64_t *result)
 {
   uint32_t len = (uint32_t)4U;
   KRML_CHECK_SIZE(sizeof (uint64_t), (uint32_t)2U * len);
@@ -2395,7 +2395,7 @@ static inline void montgomery_multiplication_buffer_by_one_mixed_p256(uint64_t *
     mul64(f3, t10, o3, o4);
     uint32_t len32 = (uint32_t)4U * (uint32_t)2U;
     uint64_t c = (uint64_t)0U;
-    for (uint32_t i = (uint32_t)0U; i < len32 / (uint32_t)4U * (uint32_t)4U / (uint32_t)4U; i++)
+    for (uint32_t i = (uint32_t)0U; i < len32 / (uint32_t)4U; i++)
     {
       uint64_t t1 = t[(uint32_t)4U * i];
       uint64_t t210 = t2[(uint32_t)4U * i];
@@ -2448,7 +2448,7 @@ static inline void montgomery_multiplication_buffer_by_one_mixed_p256(uint64_t *
     };
   uint32_t len4 = (uint32_t)4U;
   uint64_t c = (uint64_t)0U;
-  for (uint32_t i = (uint32_t)0U; i < len4 / (uint32_t)4U * (uint32_t)4U / (uint32_t)4U; i++)
+  for (uint32_t i = (uint32_t)0U; i < len4 / (uint32_t)4U; i++)
   {
     uint64_t t1 = x_[(uint32_t)4U * i];
     uint64_t t210 = p[(uint32_t)4U * i];
@@ -2485,6 +2485,538 @@ static inline void montgomery_multiplication_buffer_by_one_mixed_p256(uint64_t *
   cmovznz4_p256(carry, tempBuffer, x_, result);
 }
 
+static void montgomery_multiplication_buffer_by_one_mixed_p384(uint64_t *result)
+{
+  uint32_t len = (uint32_t)6U;
+  KRML_CHECK_SIZE(sizeof (uint64_t), (uint32_t)2U * len);
+  uint64_t t[(uint32_t)2U * len];
+  memset(t, 0U, (uint32_t)2U * len * sizeof (uint64_t));
+  uint64_t *t_low = t;
+  t_low[0U] = (uint64_t)1U;
+  uint32_t len1 = (uint32_t)6U;
+  for (uint32_t i = (uint32_t)1U; i < len1; i++)
+  {
+    t_low[i] = (uint64_t)0U;
+  }
+  uint32_t len10 = (uint32_t)6U;
+  KRML_CHECK_SIZE(sizeof (uint64_t), (uint32_t)2U * len10);
+  uint64_t t2[(uint32_t)2U * len10];
+  memset(t2, 0U, (uint32_t)2U * len10 * sizeof (uint64_t));
+  for (uint32_t i0 = (uint32_t)0U; i0 < len10; i0++)
+  {
+    uint64_t k0 = (uint64_t)4294967297U;
+    uint64_t t10 = t[0U];
+    uint64_t y = (uint64_t)0U;
+    uint64_t temp = (uint64_t)0U;
+    mul_atomic(t10, k0, &y, &temp);
+    uint64_t y_ = y;
+    uint64_t *uu____0 = t2;
+    uint32_t len30 = (uint32_t)6U;
+    for (uint32_t i = (uint32_t)0U; i < len30; i++)
+    {
+      uu____0[i] = (uint64_t)0U;
+    }
+    uint64_t *uu____1 = t2 + (uint32_t)6U;
+    uint32_t len31 = (uint32_t)6U;
+    for (uint32_t i = (uint32_t)0U; i < len31; i++)
+    {
+      uu____1[i] = (uint64_t)0U;
+    }
+    uint64_t
+    p[6U] =
+      {
+        (uint64_t)0xffffffffU, (uint64_t)0xffffffff00000000U, (uint64_t)0xfffffffffffffffeU,
+        (uint64_t)0xffffffffffffffffU, (uint64_t)0xffffffffffffffffU, (uint64_t)0xffffffffffffffffU
+      };
+    uint32_t len32 = (uint32_t)6U;
+    uint64_t bBuffer = y_;
+    uint64_t *partResult = t2;
+    memset(partResult, 0U, (len32 + (uint32_t)1U) * sizeof (uint64_t));
+    for (uint32_t i1 = (uint32_t)0U; i1 < (uint32_t)1U; i1++)
+    {
+      uint64_t bj = (&bBuffer)[i1];
+      uint64_t *res_j = partResult + i1;
+      uint64_t c = (uint64_t)0U;
+      for (uint32_t i = (uint32_t)0U; i < len32 / (uint32_t)4U; i++)
+      {
+        uint64_t a_i = p[(uint32_t)4U * i];
+        uint64_t *res_i0 = res_j + (uint32_t)4U * i;
+        c = mul_wide_add2_u64(a_i, bj, c, res_i0);
+        uint64_t a_i0 = p[(uint32_t)4U * i + (uint32_t)1U];
+        uint64_t *res_i1 = res_j + (uint32_t)4U * i + (uint32_t)1U;
+        c = mul_wide_add2_u64(a_i0, bj, c, res_i1);
+        uint64_t a_i1 = p[(uint32_t)4U * i + (uint32_t)2U];
+        uint64_t *res_i2 = res_j + (uint32_t)4U * i + (uint32_t)2U;
+        c = mul_wide_add2_u64(a_i1, bj, c, res_i2);
+        uint64_t a_i2 = p[(uint32_t)4U * i + (uint32_t)3U];
+        uint64_t *res_i = res_j + (uint32_t)4U * i + (uint32_t)3U;
+        c = mul_wide_add2_u64(a_i2, bj, c, res_i);
+      }
+      for (uint32_t i = len32 / (uint32_t)4U * (uint32_t)4U; i < len32; i++)
+      {
+        uint64_t a_i = p[i];
+        uint64_t *res_i = res_j + i;
+        c = mul_wide_add2_u64(a_i, bj, c, res_i);
+      }
+      uint64_t r = c;
+      partResult[len32 + i1] = r;
+    }
+    uint32_t len33 = (uint32_t)6U * (uint32_t)2U;
+    uint64_t c = (uint64_t)0U;
+    for (uint32_t i = (uint32_t)0U; i < len33 / (uint32_t)4U; i++)
+    {
+      uint64_t t1 = t[(uint32_t)4U * i];
+      uint64_t t210 = t2[(uint32_t)4U * i];
+      uint64_t *res_i0 = t2 + (uint32_t)4U * i;
+      c = Lib_IntTypes_Intrinsics_add_carry_u64(c, t1, t210, res_i0);
+      uint64_t t11 = t[(uint32_t)4U * i + (uint32_t)1U];
+      uint64_t t211 = t2[(uint32_t)4U * i + (uint32_t)1U];
+      uint64_t *res_i1 = t2 + (uint32_t)4U * i + (uint32_t)1U;
+      c = Lib_IntTypes_Intrinsics_add_carry_u64(c, t11, t211, res_i1);
+      uint64_t t12 = t[(uint32_t)4U * i + (uint32_t)2U];
+      uint64_t t212 = t2[(uint32_t)4U * i + (uint32_t)2U];
+      uint64_t *res_i2 = t2 + (uint32_t)4U * i + (uint32_t)2U;
+      c = Lib_IntTypes_Intrinsics_add_carry_u64(c, t12, t212, res_i2);
+      uint64_t t13 = t[(uint32_t)4U * i + (uint32_t)3U];
+      uint64_t t21 = t2[(uint32_t)4U * i + (uint32_t)3U];
+      uint64_t *res_i = t2 + (uint32_t)4U * i + (uint32_t)3U;
+      c = Lib_IntTypes_Intrinsics_add_carry_u64(c, t13, t21, res_i);
+    }
+    for (uint32_t i = len33 / (uint32_t)4U * (uint32_t)4U; i < len33; i++)
+    {
+      uint64_t t1 = t[i];
+      uint64_t t21 = t2[i];
+      uint64_t *res_i = t2 + i;
+      c = Lib_IntTypes_Intrinsics_add_carry_u64(c, t1, t21, res_i);
+    }
+    uint64_t carry = c;
+    uint32_t len3 = (uint32_t)11U;
+    for (uint32_t i = (uint32_t)0U; i < len3; i++)
+    {
+      uint64_t elem = t2[(uint32_t)1U + i];
+      t[i] = elem;
+    }
+    t[len3] = carry;
+  }
+  uint32_t len2 = (uint32_t)6U;
+  uint64_t cin = t[len2];
+  uint64_t *x_ = t;
+  uint32_t len3 = (uint32_t)6U;
+  KRML_CHECK_SIZE(sizeof (uint64_t), len3);
+  uint64_t tempBuffer[len3];
+  memset(tempBuffer, 0U, len3 * sizeof (uint64_t));
+  uint64_t tempBufferForSubborrow = (uint64_t)0U;
+  uint64_t
+  p[6U] =
+    {
+      (uint64_t)0xffffffffU, (uint64_t)0xffffffff00000000U, (uint64_t)0xfffffffffffffffeU,
+      (uint64_t)0xffffffffffffffffU, (uint64_t)0xffffffffffffffffU, (uint64_t)0xffffffffffffffffU
+    };
+  uint32_t len4 = (uint32_t)6U;
+  uint64_t c = (uint64_t)0U;
+  for (uint32_t i = (uint32_t)0U; i < len4 / (uint32_t)4U; i++)
+  {
+    uint64_t t1 = x_[(uint32_t)4U * i];
+    uint64_t t210 = p[(uint32_t)4U * i];
+    uint64_t *res_i0 = tempBuffer + (uint32_t)4U * i;
+    c = Lib_IntTypes_Intrinsics_sub_borrow_u64(c, t1, t210, res_i0);
+    uint64_t t10 = x_[(uint32_t)4U * i + (uint32_t)1U];
+    uint64_t t211 = p[(uint32_t)4U * i + (uint32_t)1U];
+    uint64_t *res_i1 = tempBuffer + (uint32_t)4U * i + (uint32_t)1U;
+    c = Lib_IntTypes_Intrinsics_sub_borrow_u64(c, t10, t211, res_i1);
+    uint64_t t11 = x_[(uint32_t)4U * i + (uint32_t)2U];
+    uint64_t t212 = p[(uint32_t)4U * i + (uint32_t)2U];
+    uint64_t *res_i2 = tempBuffer + (uint32_t)4U * i + (uint32_t)2U;
+    c = Lib_IntTypes_Intrinsics_sub_borrow_u64(c, t11, t212, res_i2);
+    uint64_t t12 = x_[(uint32_t)4U * i + (uint32_t)3U];
+    uint64_t t21 = p[(uint32_t)4U * i + (uint32_t)3U];
+    uint64_t *res_i = tempBuffer + (uint32_t)4U * i + (uint32_t)3U;
+    c = Lib_IntTypes_Intrinsics_sub_borrow_u64(c, t12, t21, res_i);
+  }
+  for (uint32_t i = len4 / (uint32_t)4U * (uint32_t)4U; i < len4; i++)
+  {
+    uint64_t t1 = x_[i];
+    uint64_t t21 = p[i];
+    uint64_t *res_i = tempBuffer + i;
+    c = Lib_IntTypes_Intrinsics_sub_borrow_u64(c, t1, t21, res_i);
+  }
+  uint64_t r = c;
+  uint64_t carry0 = r;
+  uint64_t
+  carry =
+    Lib_IntTypes_Intrinsics_sub_borrow_u64(carry0,
+      cin,
+      (uint64_t)0U,
+      &tempBufferForSubborrow);
+  cmovznz4_p384(carry, tempBuffer, x_, result);
+}
+
+static void
+copy_point_conditional(
+  Spec_ECC_Curves_curve c,
+  uint64_t *x3_out,
+  uint64_t *y3_out,
+  uint64_t *z3_out,
+  uint64_t *p,
+  uint64_t *maskPoint,
+  uint64_t *temp
+)
+{
+  uint32_t sw0;
+  switch (c)
+  {
+    case Spec_ECC_Curves_P256:
+      {
+        sw0 = (uint32_t)4U;
+        break;
+      }
+    case Spec_ECC_Curves_P384:
+      {
+        sw0 = (uint32_t)6U;
+        break;
+      }
+    default:
+      {
+        sw0 = (uint32_t)4U;
+      }
+  }
+  uint64_t *z = maskPoint + (uint32_t)2U * sw0;
+  uint64_t tmp = (uint64_t)18446744073709551615U;
+  uint32_t len0;
+  switch (c)
+  {
+    case Spec_ECC_Curves_P256:
+      {
+        len0 = (uint32_t)4U;
+        break;
+      }
+    case Spec_ECC_Curves_P384:
+      {
+        len0 = (uint32_t)6U;
+        break;
+      }
+    default:
+      {
+        len0 = (uint32_t)4U;
+      }
+  }
+  for (uint32_t i = (uint32_t)0U; i < len0; i++)
+  {
+    uint64_t a_i = z[i];
+    uint64_t r_i = FStar_UInt64_eq_mask(a_i, (uint64_t)0U);
+    uint64_t tmp0 = tmp;
+    tmp = r_i & tmp0;
+  }
+  uint64_t mask = tmp;
+  uint64_t *p_x = p;
+  uint32_t sw;
+  switch (c)
+  {
+    case Spec_ECC_Curves_P256:
+      {
+        sw = (uint32_t)4U;
+        break;
+      }
+    case Spec_ECC_Curves_P384:
+      {
+        sw = (uint32_t)6U;
+        break;
+      }
+    default:
+      {
+        sw = (uint32_t)4U;
+      }
+  }
+  uint64_t *p_y = p + sw;
+  temp[0U] = (uint64_t)1U;
+  uint32_t len;
+  switch (c)
+  {
+    case Spec_ECC_Curves_P256:
+      {
+        len = (uint32_t)4U;
+        break;
+      }
+    case Spec_ECC_Curves_P384:
+      {
+        len = (uint32_t)6U;
+        break;
+      }
+    default:
+      {
+        len = (uint32_t)4U;
+      }
+  }
+  for (uint32_t i = (uint32_t)1U; i < len; i++)
+  {
+    temp[i] = (uint64_t)0U;
+  }
+  switch (c)
+  {
+    case Spec_ECC_Curves_P256:
+      {
+        copy_conditional_p256_l(x3_out, p_x, mask);
+        break;
+      }
+    case Spec_ECC_Curves_P384:
+      {
+        copy_conditional_p384_l(x3_out, p_x, mask);
+        break;
+      }
+    case Spec_ECC_Curves_Default:
+      {
+        copy_conditional_generic_l(x3_out, p_x, mask);
+        break;
+      }
+    default:
+      {
+        KRML_HOST_EPRINTF("KreMLin incomplete match at %s:%d\n", __FILE__, __LINE__);
+        KRML_HOST_EXIT(253U);
+      }
+  }
+  switch (c)
+  {
+    case Spec_ECC_Curves_P256:
+      {
+        copy_conditional_p256_l(y3_out, p_y, mask);
+        break;
+      }
+    case Spec_ECC_Curves_P384:
+      {
+        copy_conditional_p384_l(y3_out, p_y, mask);
+        break;
+      }
+    case Spec_ECC_Curves_Default:
+      {
+        copy_conditional_generic_l(y3_out, p_y, mask);
+        break;
+      }
+    default:
+      {
+        KRML_HOST_EPRINTF("KreMLin incomplete match at %s:%d\n", __FILE__, __LINE__);
+        KRML_HOST_EXIT(253U);
+      }
+  }
+  switch (c)
+  {
+    case Spec_ECC_Curves_P256:
+      {
+        copy_conditional_p256_l(z3_out, temp, mask);
+        break;
+      }
+    case Spec_ECC_Curves_P384:
+      {
+        copy_conditional_p384_l(z3_out, temp, mask);
+        break;
+      }
+    case Spec_ECC_Curves_Default:
+      {
+        copy_conditional_generic_l(z3_out, temp, mask);
+        break;
+      }
+    default:
+      {
+        KRML_HOST_EPRINTF("KreMLin incomplete match at %s:%d\n", __FILE__, __LINE__);
+        KRML_HOST_EXIT(253U);
+      }
+  }
+}
+
+static void
+copy_point_conditional1(
+  Spec_ECC_Curves_curve c,
+  uint64_t *x3_out,
+  uint64_t *y3_out,
+  uint64_t *z3_out,
+  uint64_t *p,
+  uint64_t *q
+)
+{
+  uint32_t len;
+  switch (c)
+  {
+    case Spec_ECC_Curves_P256:
+      {
+        len = (uint32_t)4U;
+        break;
+      }
+    case Spec_ECC_Curves_P384:
+      {
+        len = (uint32_t)6U;
+        break;
+      }
+    default:
+      {
+        len = (uint32_t)4U;
+      }
+  }
+  uint64_t *x = q;
+  uint64_t *y = q + len;
+  uint64_t tmp1 = (uint64_t)18446744073709551615U;
+  uint32_t len10;
+  switch (c)
+  {
+    case Spec_ECC_Curves_P256:
+      {
+        len10 = (uint32_t)4U;
+        break;
+      }
+    case Spec_ECC_Curves_P384:
+      {
+        len10 = (uint32_t)6U;
+        break;
+      }
+    default:
+      {
+        len10 = (uint32_t)4U;
+      }
+  }
+  for (uint32_t i = (uint32_t)0U; i < len10; i++)
+  {
+    uint64_t a_i = x[i];
+    uint64_t r_i = FStar_UInt64_eq_mask(a_i, (uint64_t)0U);
+    uint64_t tmp0 = tmp1;
+    tmp1 = r_i & tmp0;
+  }
+  uint64_t xZero = tmp1;
+  uint64_t tmp = (uint64_t)18446744073709551615U;
+  uint32_t len1;
+  switch (c)
+  {
+    case Spec_ECC_Curves_P256:
+      {
+        len1 = (uint32_t)4U;
+        break;
+      }
+    case Spec_ECC_Curves_P384:
+      {
+        len1 = (uint32_t)6U;
+        break;
+      }
+    default:
+      {
+        len1 = (uint32_t)4U;
+      }
+  }
+  for (uint32_t i = (uint32_t)0U; i < len1; i++)
+  {
+    uint64_t a_i = y[i];
+    uint64_t r_i = FStar_UInt64_eq_mask(a_i, (uint64_t)0U);
+    uint64_t tmp0 = tmp;
+    tmp = r_i & tmp0;
+  }
+  uint64_t yZero = tmp;
+  uint64_t mask = xZero & yZero;
+  uint64_t *p_x = p;
+  uint32_t sw0;
+  switch (c)
+  {
+    case Spec_ECC_Curves_P256:
+      {
+        sw0 = (uint32_t)4U;
+        break;
+      }
+    case Spec_ECC_Curves_P384:
+      {
+        sw0 = (uint32_t)6U;
+        break;
+      }
+    default:
+      {
+        sw0 = (uint32_t)4U;
+      }
+  }
+  uint64_t *p_y = p + sw0;
+  uint32_t sw;
+  switch (c)
+  {
+    case Spec_ECC_Curves_P256:
+      {
+        sw = (uint32_t)4U;
+        break;
+      }
+    case Spec_ECC_Curves_P384:
+      {
+        sw = (uint32_t)6U;
+        break;
+      }
+    default:
+      {
+        sw = (uint32_t)4U;
+      }
+  }
+  uint64_t *p_z = p + (uint32_t)2U * sw;
+  switch (c)
+  {
+    case Spec_ECC_Curves_P256:
+      {
+        copy_conditional_p256_l(x3_out, p_x, mask);
+        break;
+      }
+    case Spec_ECC_Curves_P384:
+      {
+        copy_conditional_p384_l(x3_out, p_x, mask);
+        break;
+      }
+    case Spec_ECC_Curves_Default:
+      {
+        copy_conditional_generic_l(x3_out, p_x, mask);
+        break;
+      }
+    default:
+      {
+        KRML_HOST_EPRINTF("KreMLin incomplete match at %s:%d\n", __FILE__, __LINE__);
+        KRML_HOST_EXIT(253U);
+      }
+  }
+  switch (c)
+  {
+    case Spec_ECC_Curves_P256:
+      {
+        copy_conditional_p256_l(y3_out, p_y, mask);
+        break;
+      }
+    case Spec_ECC_Curves_P384:
+      {
+        copy_conditional_p384_l(y3_out, p_y, mask);
+        break;
+      }
+    case Spec_ECC_Curves_Default:
+      {
+        copy_conditional_generic_l(y3_out, p_y, mask);
+        break;
+      }
+    default:
+      {
+        KRML_HOST_EPRINTF("KreMLin incomplete match at %s:%d\n", __FILE__, __LINE__);
+        KRML_HOST_EXIT(253U);
+      }
+  }
+  switch (c)
+  {
+    case Spec_ECC_Curves_P256:
+      {
+        copy_conditional_p256_l(z3_out, p_z, mask);
+        break;
+      }
+    case Spec_ECC_Curves_P384:
+      {
+        copy_conditional_p384_l(z3_out, p_z, mask);
+        break;
+      }
+    case Spec_ECC_Curves_Default:
+      {
+        copy_conditional_generic_l(z3_out, p_z, mask);
+        break;
+      }
+    default:
+      {
+        KRML_HOST_EPRINTF("KreMLin incomplete match at %s:%d\n", __FILE__, __LINE__);
+        KRML_HOST_EXIT(253U);
+      }
+  }
+}
+
 static inline void
 point_add_mixed_p256(uint64_t *p, uint64_t *q, uint64_t *result, uint64_t *tempBuffer)
 {
@@ -2512,11 +3044,11 @@ point_add_mixed_p256(uint64_t *p, uint64_t *q, uint64_t *result, uint64_t *tempB
   memset(t0, 0U, (uint32_t)2U * len0 * sizeof (uint64_t));
   uint64_t *t_low0 = t0;
   memcpy(t_low0, z2Square, len0 * sizeof (uint64_t));
-  uint32_t len10 = (uint32_t)4U;
-  KRML_CHECK_SIZE(sizeof (uint64_t), (uint32_t)2U * len10);
-  uint64_t t20[(uint32_t)2U * len10];
-  memset(t20, 0U, (uint32_t)2U * len10 * sizeof (uint64_t));
-  for (uint32_t i0 = (uint32_t)0U; i0 < len10; i0++)
+  uint32_t len1 = (uint32_t)4U;
+  KRML_CHECK_SIZE(sizeof (uint64_t), (uint32_t)2U * len1);
+  uint64_t t20[(uint32_t)2U * len1];
+  memset(t20, 0U, (uint32_t)2U * len1 * sizeof (uint64_t));
+  for (uint32_t i0 = (uint32_t)0U; i0 < len1; i0++)
   {
     uint64_t t10 = t0[0U];
     uint64_t *uu____0 = t20;
@@ -2550,7 +3082,7 @@ point_add_mixed_p256(uint64_t *p, uint64_t *q, uint64_t *result, uint64_t *tempB
     mul64(f3, t10, o3, o4);
     uint32_t len32 = (uint32_t)4U * (uint32_t)2U;
     uint64_t c = (uint64_t)0U;
-    for (uint32_t i = (uint32_t)0U; i < len32 / (uint32_t)4U * (uint32_t)4U / (uint32_t)4U; i++)
+    for (uint32_t i = (uint32_t)0U; i < len32 / (uint32_t)4U; i++)
     {
       uint64_t t1 = t0[(uint32_t)4U * i];
       uint64_t t210 = t20[(uint32_t)4U * i];
@@ -2603,7 +3135,7 @@ point_add_mixed_p256(uint64_t *p, uint64_t *q, uint64_t *result, uint64_t *tempB
     };
   uint32_t len40 = (uint32_t)4U;
   uint64_t c0 = (uint64_t)0U;
-  for (uint32_t i = (uint32_t)0U; i < len40 / (uint32_t)4U * (uint32_t)4U / (uint32_t)4U; i++)
+  for (uint32_t i = (uint32_t)0U; i < len40 / (uint32_t)4U; i++)
   {
     uint64_t t1 = x_0[(uint32_t)4U * i];
     uint64_t t210 = p10[(uint32_t)4U * i];
@@ -2643,7 +3175,7 @@ point_add_mixed_p256(uint64_t *p, uint64_t *q, uint64_t *result, uint64_t *tempB
   montgomery_multiplication_buffer_dh_p256(z1Square, qX, u20);
   montgomery_multiplication_buffer_dh_p256(z2Cube, pY, s10);
   montgomery_multiplication_buffer_dh_p256(z1Cube, qY, s20);
-  uint64_t *temp = t12;
+  uint64_t *temp0 = t12;
   uint64_t *u1 = t12 + (uint32_t)16U;
   uint64_t *u2 = t12 + (uint32_t)20U;
   uint64_t *s11 = t12 + (uint32_t)24U;
@@ -2654,9 +3186,9 @@ point_add_mixed_p256(uint64_t *p, uint64_t *q, uint64_t *result, uint64_t *tempB
   uint64_t *hCube0 = t12 + (uint32_t)44U;
   felem_sub_p256(u2, u1, h);
   felem_sub_p256(s2, s11, r1);
-  montgomery_square_buffer_dh_p256(h, temp);
-  montgomery_multiplication_buffer_dh_p256(temp, u1, uh0);
-  montgomery_multiplication_buffer_dh_p256(temp, h, hCube0);
+  montgomery_square_buffer_dh_p256(h, temp0);
+  montgomery_multiplication_buffer_dh_p256(temp0, u1, uh0);
+  montgomery_multiplication_buffer_dh_p256(temp0, h, hCube0);
   uint64_t *h0 = t12 + (uint32_t)32U;
   uint64_t *r = t12 + (uint32_t)36U;
   uint64_t *uh = t12 + (uint32_t)40U;
@@ -2682,17 +3214,17 @@ point_add_mixed_p256(uint64_t *p, uint64_t *q, uint64_t *result, uint64_t *tempB
   uint64_t *z1 = p + (uint32_t)8U;
   uint64_t *z3 = t5 + (uint32_t)8U;
   uint64_t *z1z2 = t5 + (uint32_t)12U;
-  uint32_t len5 = (uint32_t)4U;
-  KRML_CHECK_SIZE(sizeof (uint64_t), (uint32_t)2U * len5);
-  uint64_t t[(uint32_t)2U * len5];
-  memset(t, 0U, (uint32_t)2U * len5 * sizeof (uint64_t));
+  uint32_t len = (uint32_t)4U;
+  KRML_CHECK_SIZE(sizeof (uint64_t), (uint32_t)2U * len);
+  uint64_t t[(uint32_t)2U * len];
+  memset(t, 0U, (uint32_t)2U * len * sizeof (uint64_t));
   uint64_t *t_low = t;
-  memcpy(t_low, z1, len5 * sizeof (uint64_t));
-  uint32_t len11 = (uint32_t)4U;
-  KRML_CHECK_SIZE(sizeof (uint64_t), (uint32_t)2U * len11);
-  uint64_t t2[(uint32_t)2U * len11];
-  memset(t2, 0U, (uint32_t)2U * len11 * sizeof (uint64_t));
-  for (uint32_t i0 = (uint32_t)0U; i0 < len11; i0++)
+  memcpy(t_low, z1, len * sizeof (uint64_t));
+  uint32_t len10 = (uint32_t)4U;
+  KRML_CHECK_SIZE(sizeof (uint64_t), (uint32_t)2U * len10);
+  uint64_t t2[(uint32_t)2U * len10];
+  memset(t2, 0U, (uint32_t)2U * len10 * sizeof (uint64_t));
+  for (uint32_t i0 = (uint32_t)0U; i0 < len10; i0++)
   {
     uint64_t t10 = t[0U];
     uint64_t *uu____2 = t2;
@@ -2707,7 +3239,7 @@ point_add_mixed_p256(uint64_t *p, uint64_t *q, uint64_t *result, uint64_t *tempB
     {
       uu____3[i] = (uint64_t)0U;
     }
-    uint64_t temp0 = (uint64_t)0U;
+    uint64_t temp = (uint64_t)0U;
     uint64_t f0 = (uint64_t)0xffffffffffffffffU;
     uint64_t f1 = (uint64_t)0xffffffffU;
     uint64_t f3 = (uint64_t)0xffffffff00000001U;
@@ -2716,17 +3248,17 @@ point_add_mixed_p256(uint64_t *p, uint64_t *q, uint64_t *result, uint64_t *tempB
     uint64_t *o2 = t2 + (uint32_t)2U;
     uint64_t *o3 = t2 + (uint32_t)3U;
     uint64_t *o4 = t2 + (uint32_t)4U;
-    mul64(f0, t10, o0, &temp0);
-    uint64_t h2 = temp0;
-    mul64(f1, t10, o1, &temp0);
+    mul64(f0, t10, o0, &temp);
+    uint64_t h2 = temp;
+    mul64(f1, t10, o1, &temp);
     uint64_t l = o1[0U];
     uint64_t c1 = Lib_IntTypes_Intrinsics_add_carry_u64((uint64_t)0U, l, h2, o1);
-    uint64_t h3 = temp0;
+    uint64_t h3 = temp;
     o2[0U] = h3 + c1;
     mul64(f3, t10, o3, o4);
     uint32_t len33 = (uint32_t)4U * (uint32_t)2U;
     uint64_t c = (uint64_t)0U;
-    for (uint32_t i = (uint32_t)0U; i < len33 / (uint32_t)4U * (uint32_t)4U / (uint32_t)4U; i++)
+    for (uint32_t i = (uint32_t)0U; i < len33 / (uint32_t)4U; i++)
     {
       uint64_t t1 = t[(uint32_t)4U * i];
       uint64_t t210 = t2[(uint32_t)4U * i];
@@ -2779,7 +3311,7 @@ point_add_mixed_p256(uint64_t *p, uint64_t *q, uint64_t *result, uint64_t *tempB
     };
   uint32_t len4 = (uint32_t)4U;
   uint64_t c = (uint64_t)0U;
-  for (uint32_t i = (uint32_t)0U; i < len4 / (uint32_t)4U * (uint32_t)4U / (uint32_t)4U; i++)
+  for (uint32_t i = (uint32_t)0U; i < len4 / (uint32_t)4U; i++)
   {
     uint64_t t1 = x_[(uint32_t)4U * i];
     uint64_t t210 = p1[(uint32_t)4U * i];
@@ -2818,61 +3350,408 @@ point_add_mixed_p256(uint64_t *p, uint64_t *q, uint64_t *result, uint64_t *tempB
   uint64_t *x3_out = t5;
   uint64_t *y3_out = t5 + (uint32_t)4U;
   uint64_t *z3_out = t5 + (uint32_t)8U;
-  uint64_t *z = p + (uint32_t)8U;
-  uint64_t tmp1 = (uint64_t)18446744073709551615U;
-  uint32_t len = (uint32_t)4U;
-  for (uint32_t i = (uint32_t)0U; i < len; i++)
-  {
-    uint64_t a_i = z[i];
-    uint64_t r_i = FStar_UInt64_eq_mask(a_i, (uint64_t)0U);
-    uint64_t tmp0 = tmp1;
-    tmp1 = r_i & tmp0;
-  }
-  uint64_t mask = tmp1;
-  uint64_t *p_x0 = q;
-  uint64_t *p_y0 = q + (uint32_t)4U;
-  uint64_t *p_z0 = q + (uint32_t)8U;
-  copy_conditional_p256_l(x3_out, p_x0, mask);
-  copy_conditional_p256_l(y3_out, p_y0, mask);
-  copy_conditional_p256_l(z3_out, p_z0, mask);
-  uint32_t len6 = (uint32_t)4U;
-  uint64_t *x = q;
-  uint64_t *y = q + len6;
-  uint64_t tmp2 = (uint64_t)18446744073709551615U;
-  uint32_t len12 = (uint32_t)4U;
-  for (uint32_t i = (uint32_t)0U; i < len12; i++)
-  {
-    uint64_t a_i = x[i];
-    uint64_t r_i = FStar_UInt64_eq_mask(a_i, (uint64_t)0U);
-    uint64_t tmp0 = tmp2;
-    tmp2 = r_i & tmp0;
-  }
-  uint64_t xZero = tmp2;
-  uint64_t tmp = (uint64_t)18446744073709551615U;
-  uint32_t len1 = (uint32_t)4U;
-  for (uint32_t i = (uint32_t)0U; i < len1; i++)
-  {
-    uint64_t a_i = y[i];
-    uint64_t r_i = FStar_UInt64_eq_mask(a_i, (uint64_t)0U);
-    uint64_t tmp0 = tmp;
-    tmp = r_i & tmp0;
-  }
-  uint64_t yZero = tmp;
-  uint64_t mask0 = xZero & yZero;
-  uint64_t *p_x = p;
-  uint64_t *p_y = p + (uint32_t)4U;
-  uint64_t *p_z = p + (uint32_t)8U;
-  copy_conditional_p256_l(x3_out, p_x, mask0);
-  copy_conditional_p256_l(y3_out, p_y, mask0);
-  copy_conditional_p256_l(z3_out, p_z, mask0);
+  uint64_t *temp = t5 + (uint32_t)12U;
+  copy_point_conditional(Spec_ECC_Curves_P256, x3_out, y3_out, z3_out, q, p, temp);
+  copy_point_conditional1(Spec_ECC_Curves_P256, x3_out, y3_out, z3_out, p, q);
   memcpy(result, x3_out, (uint32_t)4U * sizeof (uint64_t));
   memcpy(result + (uint32_t)4U, y3_out, (uint32_t)4U * sizeof (uint64_t));
   memcpy(result + (uint32_t)8U, z3_out, (uint32_t)4U * sizeof (uint64_t));
 }
 
+static inline void
+point_add_mixed_p384(uint64_t *p, uint64_t *q, uint64_t *result, uint64_t *tempBuffer)
+{
+  uint64_t *t12 = tempBuffer;
+  uint64_t *t5 = tempBuffer + (uint32_t)72U;
+  uint64_t *t4 = t12;
+  uint64_t *u10 = t12 + (uint32_t)24U;
+  uint64_t *u20 = t12 + (uint32_t)30U;
+  uint64_t *s10 = t12 + (uint32_t)36U;
+  uint64_t *s20 = t12 + (uint32_t)42U;
+  uint64_t *pX = p;
+  uint64_t *pY = p + (uint32_t)6U;
+  uint64_t *pZ = p + (uint32_t)12U;
+  uint64_t *qX = q;
+  uint64_t *qY = q + (uint32_t)6U;
+  uint64_t *z2Square = t4;
+  uint64_t *z1Square = t4 + (uint32_t)6U;
+  uint64_t *z2Cube = t4 + (uint32_t)12U;
+  uint64_t *z1Cube = t4 + (uint32_t)18U;
+  montgomery_multiplication_buffer_by_one_mixed_p384(z2Square);
+  montgomery_square_buffer_dh_p384(pZ, z1Square);
+  uint32_t len0 = (uint32_t)6U;
+  KRML_CHECK_SIZE(sizeof (uint64_t), (uint32_t)2U * len0);
+  uint64_t t0[(uint32_t)2U * len0];
+  memset(t0, 0U, (uint32_t)2U * len0 * sizeof (uint64_t));
+  uint64_t *t_low0 = t0;
+  memcpy(t_low0, z2Square, len0 * sizeof (uint64_t));
+  uint32_t len1 = (uint32_t)6U;
+  KRML_CHECK_SIZE(sizeof (uint64_t), (uint32_t)2U * len1);
+  uint64_t t20[(uint32_t)2U * len1];
+  memset(t20, 0U, (uint32_t)2U * len1 * sizeof (uint64_t));
+  for (uint32_t i0 = (uint32_t)0U; i0 < len1; i0++)
+  {
+    uint64_t k0 = (uint64_t)4294967297U;
+    uint64_t t10 = t0[0U];
+    uint64_t y = (uint64_t)0U;
+    uint64_t temp = (uint64_t)0U;
+    mul_atomic(t10, k0, &y, &temp);
+    uint64_t y_ = y;
+    uint64_t *uu____0 = t20;
+    uint32_t len30 = (uint32_t)6U;
+    for (uint32_t i = (uint32_t)0U; i < len30; i++)
+    {
+      uu____0[i] = (uint64_t)0U;
+    }
+    uint64_t *uu____1 = t20 + (uint32_t)6U;
+    uint32_t len31 = (uint32_t)6U;
+    for (uint32_t i = (uint32_t)0U; i < len31; i++)
+    {
+      uu____1[i] = (uint64_t)0U;
+    }
+    uint64_t
+    p1[6U] =
+      {
+        (uint64_t)0xffffffffU, (uint64_t)0xffffffff00000000U, (uint64_t)0xfffffffffffffffeU,
+        (uint64_t)0xffffffffffffffffU, (uint64_t)0xffffffffffffffffU, (uint64_t)0xffffffffffffffffU
+      };
+    uint32_t len32 = (uint32_t)6U;
+    uint64_t bBuffer = y_;
+    uint64_t *partResult = t20;
+    memset(partResult, 0U, (len32 + (uint32_t)1U) * sizeof (uint64_t));
+    for (uint32_t i1 = (uint32_t)0U; i1 < (uint32_t)1U; i1++)
+    {
+      uint64_t bj = (&bBuffer)[i1];
+      uint64_t *res_j = partResult + i1;
+      uint64_t c = (uint64_t)0U;
+      for (uint32_t i = (uint32_t)0U; i < len32 / (uint32_t)4U; i++)
+      {
+        uint64_t a_i = p1[(uint32_t)4U * i];
+        uint64_t *res_i0 = res_j + (uint32_t)4U * i;
+        c = mul_wide_add2_u64(a_i, bj, c, res_i0);
+        uint64_t a_i0 = p1[(uint32_t)4U * i + (uint32_t)1U];
+        uint64_t *res_i1 = res_j + (uint32_t)4U * i + (uint32_t)1U;
+        c = mul_wide_add2_u64(a_i0, bj, c, res_i1);
+        uint64_t a_i1 = p1[(uint32_t)4U * i + (uint32_t)2U];
+        uint64_t *res_i2 = res_j + (uint32_t)4U * i + (uint32_t)2U;
+        c = mul_wide_add2_u64(a_i1, bj, c, res_i2);
+        uint64_t a_i2 = p1[(uint32_t)4U * i + (uint32_t)3U];
+        uint64_t *res_i = res_j + (uint32_t)4U * i + (uint32_t)3U;
+        c = mul_wide_add2_u64(a_i2, bj, c, res_i);
+      }
+      for (uint32_t i = len32 / (uint32_t)4U * (uint32_t)4U; i < len32; i++)
+      {
+        uint64_t a_i = p1[i];
+        uint64_t *res_i = res_j + i;
+        c = mul_wide_add2_u64(a_i, bj, c, res_i);
+      }
+      uint64_t r = c;
+      partResult[len32 + i1] = r;
+    }
+    uint32_t len33 = (uint32_t)6U * (uint32_t)2U;
+    uint64_t c = (uint64_t)0U;
+    for (uint32_t i = (uint32_t)0U; i < len33 / (uint32_t)4U; i++)
+    {
+      uint64_t t1 = t0[(uint32_t)4U * i];
+      uint64_t t210 = t20[(uint32_t)4U * i];
+      uint64_t *res_i0 = t20 + (uint32_t)4U * i;
+      c = Lib_IntTypes_Intrinsics_add_carry_u64(c, t1, t210, res_i0);
+      uint64_t t11 = t0[(uint32_t)4U * i + (uint32_t)1U];
+      uint64_t t211 = t20[(uint32_t)4U * i + (uint32_t)1U];
+      uint64_t *res_i1 = t20 + (uint32_t)4U * i + (uint32_t)1U;
+      c = Lib_IntTypes_Intrinsics_add_carry_u64(c, t11, t211, res_i1);
+      uint64_t t13 = t0[(uint32_t)4U * i + (uint32_t)2U];
+      uint64_t t212 = t20[(uint32_t)4U * i + (uint32_t)2U];
+      uint64_t *res_i2 = t20 + (uint32_t)4U * i + (uint32_t)2U;
+      c = Lib_IntTypes_Intrinsics_add_carry_u64(c, t13, t212, res_i2);
+      uint64_t t14 = t0[(uint32_t)4U * i + (uint32_t)3U];
+      uint64_t t21 = t20[(uint32_t)4U * i + (uint32_t)3U];
+      uint64_t *res_i = t20 + (uint32_t)4U * i + (uint32_t)3U;
+      c = Lib_IntTypes_Intrinsics_add_carry_u64(c, t14, t21, res_i);
+    }
+    for (uint32_t i = len33 / (uint32_t)4U * (uint32_t)4U; i < len33; i++)
+    {
+      uint64_t t1 = t0[i];
+      uint64_t t21 = t20[i];
+      uint64_t *res_i = t20 + i;
+      c = Lib_IntTypes_Intrinsics_add_carry_u64(c, t1, t21, res_i);
+    }
+    uint64_t carry = c;
+    uint32_t len3 = (uint32_t)11U;
+    for (uint32_t i = (uint32_t)0U; i < len3; i++)
+    {
+      uint64_t elem = t20[(uint32_t)1U + i];
+      t0[i] = elem;
+    }
+    t0[len3] = carry;
+  }
+  uint32_t len2 = (uint32_t)6U;
+  uint64_t cin = t0[len2];
+  uint64_t *x_0 = t0;
+  uint32_t len30 = (uint32_t)6U;
+  KRML_CHECK_SIZE(sizeof (uint64_t), len30);
+  uint64_t tempBuffer1[len30];
+  memset(tempBuffer1, 0U, len30 * sizeof (uint64_t));
+  uint64_t tempBufferForSubborrow0 = (uint64_t)0U;
+  uint64_t
+  p10[6U] =
+    {
+      (uint64_t)0xffffffffU, (uint64_t)0xffffffff00000000U, (uint64_t)0xfffffffffffffffeU,
+      (uint64_t)0xffffffffffffffffU, (uint64_t)0xffffffffffffffffU, (uint64_t)0xffffffffffffffffU
+    };
+  uint32_t len40 = (uint32_t)6U;
+  uint64_t c0 = (uint64_t)0U;
+  for (uint32_t i = (uint32_t)0U; i < len40 / (uint32_t)4U; i++)
+  {
+    uint64_t t1 = x_0[(uint32_t)4U * i];
+    uint64_t t210 = p10[(uint32_t)4U * i];
+    uint64_t *res_i0 = tempBuffer1 + (uint32_t)4U * i;
+    c0 = Lib_IntTypes_Intrinsics_sub_borrow_u64(c0, t1, t210, res_i0);
+    uint64_t t10 = x_0[(uint32_t)4U * i + (uint32_t)1U];
+    uint64_t t211 = p10[(uint32_t)4U * i + (uint32_t)1U];
+    uint64_t *res_i1 = tempBuffer1 + (uint32_t)4U * i + (uint32_t)1U;
+    c0 = Lib_IntTypes_Intrinsics_sub_borrow_u64(c0, t10, t211, res_i1);
+    uint64_t t11 = x_0[(uint32_t)4U * i + (uint32_t)2U];
+    uint64_t t212 = p10[(uint32_t)4U * i + (uint32_t)2U];
+    uint64_t *res_i2 = tempBuffer1 + (uint32_t)4U * i + (uint32_t)2U;
+    c0 = Lib_IntTypes_Intrinsics_sub_borrow_u64(c0, t11, t212, res_i2);
+    uint64_t t13 = x_0[(uint32_t)4U * i + (uint32_t)3U];
+    uint64_t t21 = p10[(uint32_t)4U * i + (uint32_t)3U];
+    uint64_t *res_i = tempBuffer1 + (uint32_t)4U * i + (uint32_t)3U;
+    c0 = Lib_IntTypes_Intrinsics_sub_borrow_u64(c0, t13, t21, res_i);
+  }
+  for (uint32_t i = len40 / (uint32_t)4U * (uint32_t)4U; i < len40; i++)
+  {
+    uint64_t t1 = x_0[i];
+    uint64_t t21 = p10[i];
+    uint64_t *res_i = tempBuffer1 + i;
+    c0 = Lib_IntTypes_Intrinsics_sub_borrow_u64(c0, t1, t21, res_i);
+  }
+  uint64_t r0 = c0;
+  uint64_t carry0 = r0;
+  uint64_t
+  carry =
+    Lib_IntTypes_Intrinsics_sub_borrow_u64(carry0,
+      cin,
+      (uint64_t)0U,
+      &tempBufferForSubborrow0);
+  cmovznz4_p384(carry, tempBuffer1, x_0, z2Cube);
+  montgomery_multiplication_buffer_dh_p384(z1Square, pZ, z1Cube);
+  montgomery_multiplication_buffer_dh_p384(z2Square, pX, u10);
+  montgomery_multiplication_buffer_dh_p384(z1Square, qX, u20);
+  montgomery_multiplication_buffer_dh_p384(z2Cube, pY, s10);
+  montgomery_multiplication_buffer_dh_p384(z1Cube, qY, s20);
+  uint64_t *temp0 = t12;
+  uint64_t *u1 = t12 + (uint32_t)24U;
+  uint64_t *u2 = t12 + (uint32_t)30U;
+  uint64_t *s11 = t12 + (uint32_t)36U;
+  uint64_t *s2 = t12 + (uint32_t)42U;
+  uint64_t *h = t12 + (uint32_t)48U;
+  uint64_t *r1 = t12 + (uint32_t)54U;
+  uint64_t *uh0 = t12 + (uint32_t)60U;
+  uint64_t *hCube0 = t12 + (uint32_t)66U;
+  felem_sub_p384(u2, u1, h);
+  felem_sub_p384(s2, s11, r1);
+  montgomery_square_buffer_dh_p384(h, temp0);
+  montgomery_multiplication_buffer_dh_p384(temp0, u1, uh0);
+  montgomery_multiplication_buffer_dh_p384(temp0, h, hCube0);
+  uint64_t *h0 = t12 + (uint32_t)48U;
+  uint64_t *r = t12 + (uint32_t)54U;
+  uint64_t *uh = t12 + (uint32_t)60U;
+  uint64_t *hCube = t12 + (uint32_t)66U;
+  uint64_t *s1 = t12 + (uint32_t)36U;
+  uint64_t *x3 = t5;
+  uint64_t *rSquare = t5 + (uint32_t)6U;
+  uint64_t *rH = t5 + (uint32_t)12U;
+  uint64_t *twoUh = t5 + (uint32_t)18U;
+  montgomery_square_buffer_dh_p384(r, rSquare);
+  felem_sub_p384(rSquare, hCube, rH);
+  felem_add_p384(uh, uh, twoUh);
+  felem_sub_p384(rH, twoUh, x3);
+  uint64_t *x30 = t5;
+  uint64_t *y3 = t5 + (uint32_t)6U;
+  uint64_t *s1hCube = t5 + (uint32_t)12U;
+  uint64_t *u1hx3 = t5 + (uint32_t)18U;
+  uint64_t *ru1hx3 = t5 + (uint32_t)24U;
+  montgomery_multiplication_buffer_dh_p384(s1, hCube, s1hCube);
+  felem_sub_p384(uh, x30, u1hx3);
+  montgomery_multiplication_buffer_dh_p384(u1hx3, r, ru1hx3);
+  felem_sub_p384(ru1hx3, s1hCube, y3);
+  uint64_t *z1 = p + (uint32_t)12U;
+  uint64_t *z3 = t5 + (uint32_t)12U;
+  uint64_t *z1z2 = t5 + (uint32_t)18U;
+  uint32_t len = (uint32_t)6U;
+  KRML_CHECK_SIZE(sizeof (uint64_t), (uint32_t)2U * len);
+  uint64_t t[(uint32_t)2U * len];
+  memset(t, 0U, (uint32_t)2U * len * sizeof (uint64_t));
+  uint64_t *t_low = t;
+  memcpy(t_low, z1, len * sizeof (uint64_t));
+  uint32_t len10 = (uint32_t)6U;
+  KRML_CHECK_SIZE(sizeof (uint64_t), (uint32_t)2U * len10);
+  uint64_t t2[(uint32_t)2U * len10];
+  memset(t2, 0U, (uint32_t)2U * len10 * sizeof (uint64_t));
+  for (uint32_t i0 = (uint32_t)0U; i0 < len10; i0++)
+  {
+    uint64_t k0 = (uint64_t)4294967297U;
+    uint64_t t10 = t[0U];
+    uint64_t y = (uint64_t)0U;
+    uint64_t temp = (uint64_t)0U;
+    mul_atomic(t10, k0, &y, &temp);
+    uint64_t y_ = y;
+    uint64_t *uu____2 = t2;
+    uint32_t len31 = (uint32_t)6U;
+    for (uint32_t i = (uint32_t)0U; i < len31; i++)
+    {
+      uu____2[i] = (uint64_t)0U;
+    }
+    uint64_t *uu____3 = t2 + (uint32_t)6U;
+    uint32_t len32 = (uint32_t)6U;
+    for (uint32_t i = (uint32_t)0U; i < len32; i++)
+    {
+      uu____3[i] = (uint64_t)0U;
+    }
+    uint64_t
+    p1[6U] =
+      {
+        (uint64_t)0xffffffffU, (uint64_t)0xffffffff00000000U, (uint64_t)0xfffffffffffffffeU,
+        (uint64_t)0xffffffffffffffffU, (uint64_t)0xffffffffffffffffU, (uint64_t)0xffffffffffffffffU
+      };
+    uint32_t len33 = (uint32_t)6U;
+    uint64_t bBuffer = y_;
+    uint64_t *partResult = t2;
+    memset(partResult, 0U, (len33 + (uint32_t)1U) * sizeof (uint64_t));
+    for (uint32_t i1 = (uint32_t)0U; i1 < (uint32_t)1U; i1++)
+    {
+      uint64_t bj = (&bBuffer)[i1];
+      uint64_t *res_j = partResult + i1;
+      uint64_t c = (uint64_t)0U;
+      for (uint32_t i = (uint32_t)0U; i < len33 / (uint32_t)4U; i++)
+      {
+        uint64_t a_i = p1[(uint32_t)4U * i];
+        uint64_t *res_i0 = res_j + (uint32_t)4U * i;
+        c = mul_wide_add2_u64(a_i, bj, c, res_i0);
+        uint64_t a_i0 = p1[(uint32_t)4U * i + (uint32_t)1U];
+        uint64_t *res_i1 = res_j + (uint32_t)4U * i + (uint32_t)1U;
+        c = mul_wide_add2_u64(a_i0, bj, c, res_i1);
+        uint64_t a_i1 = p1[(uint32_t)4U * i + (uint32_t)2U];
+        uint64_t *res_i2 = res_j + (uint32_t)4U * i + (uint32_t)2U;
+        c = mul_wide_add2_u64(a_i1, bj, c, res_i2);
+        uint64_t a_i2 = p1[(uint32_t)4U * i + (uint32_t)3U];
+        uint64_t *res_i = res_j + (uint32_t)4U * i + (uint32_t)3U;
+        c = mul_wide_add2_u64(a_i2, bj, c, res_i);
+      }
+      for (uint32_t i = len33 / (uint32_t)4U * (uint32_t)4U; i < len33; i++)
+      {
+        uint64_t a_i = p1[i];
+        uint64_t *res_i = res_j + i;
+        c = mul_wide_add2_u64(a_i, bj, c, res_i);
+      }
+      uint64_t r10 = c;
+      partResult[len33 + i1] = r10;
+    }
+    uint32_t len34 = (uint32_t)6U * (uint32_t)2U;
+    uint64_t c = (uint64_t)0U;
+    for (uint32_t i = (uint32_t)0U; i < len34 / (uint32_t)4U; i++)
+    {
+      uint64_t t1 = t[(uint32_t)4U * i];
+      uint64_t t210 = t2[(uint32_t)4U * i];
+      uint64_t *res_i0 = t2 + (uint32_t)4U * i;
+      c = Lib_IntTypes_Intrinsics_add_carry_u64(c, t1, t210, res_i0);
+      uint64_t t11 = t[(uint32_t)4U * i + (uint32_t)1U];
+      uint64_t t211 = t2[(uint32_t)4U * i + (uint32_t)1U];
+      uint64_t *res_i1 = t2 + (uint32_t)4U * i + (uint32_t)1U;
+      c = Lib_IntTypes_Intrinsics_add_carry_u64(c, t11, t211, res_i1);
+      uint64_t t13 = t[(uint32_t)4U * i + (uint32_t)2U];
+      uint64_t t212 = t2[(uint32_t)4U * i + (uint32_t)2U];
+      uint64_t *res_i2 = t2 + (uint32_t)4U * i + (uint32_t)2U;
+      c = Lib_IntTypes_Intrinsics_add_carry_u64(c, t13, t212, res_i2);
+      uint64_t t14 = t[(uint32_t)4U * i + (uint32_t)3U];
+      uint64_t t21 = t2[(uint32_t)4U * i + (uint32_t)3U];
+      uint64_t *res_i = t2 + (uint32_t)4U * i + (uint32_t)3U;
+      c = Lib_IntTypes_Intrinsics_add_carry_u64(c, t14, t21, res_i);
+    }
+    for (uint32_t i = len34 / (uint32_t)4U * (uint32_t)4U; i < len34; i++)
+    {
+      uint64_t t1 = t[i];
+      uint64_t t21 = t2[i];
+      uint64_t *res_i = t2 + i;
+      c = Lib_IntTypes_Intrinsics_add_carry_u64(c, t1, t21, res_i);
+    }
+    uint64_t carry1 = c;
+    uint32_t len3 = (uint32_t)11U;
+    for (uint32_t i = (uint32_t)0U; i < len3; i++)
+    {
+      uint64_t elem = t2[(uint32_t)1U + i];
+      t[i] = elem;
+    }
+    t[len3] = carry1;
+  }
+  uint32_t len20 = (uint32_t)6U;
+  uint64_t cin0 = t[len20];
+  uint64_t *x_ = t;
+  uint32_t len3 = (uint32_t)6U;
+  KRML_CHECK_SIZE(sizeof (uint64_t), len3);
+  uint64_t tempBuffer10[len3];
+  memset(tempBuffer10, 0U, len3 * sizeof (uint64_t));
+  uint64_t tempBufferForSubborrow = (uint64_t)0U;
+  uint64_t
+  p1[6U] =
+    {
+      (uint64_t)0xffffffffU, (uint64_t)0xffffffff00000000U, (uint64_t)0xfffffffffffffffeU,
+      (uint64_t)0xffffffffffffffffU, (uint64_t)0xffffffffffffffffU, (uint64_t)0xffffffffffffffffU
+    };
+  uint32_t len4 = (uint32_t)6U;
+  uint64_t c = (uint64_t)0U;
+  for (uint32_t i = (uint32_t)0U; i < len4 / (uint32_t)4U; i++)
+  {
+    uint64_t t1 = x_[(uint32_t)4U * i];
+    uint64_t t210 = p1[(uint32_t)4U * i];
+    uint64_t *res_i0 = tempBuffer10 + (uint32_t)4U * i;
+    c = Lib_IntTypes_Intrinsics_sub_borrow_u64(c, t1, t210, res_i0);
+    uint64_t t10 = x_[(uint32_t)4U * i + (uint32_t)1U];
+    uint64_t t211 = p1[(uint32_t)4U * i + (uint32_t)1U];
+    uint64_t *res_i1 = tempBuffer10 + (uint32_t)4U * i + (uint32_t)1U;
+    c = Lib_IntTypes_Intrinsics_sub_borrow_u64(c, t10, t211, res_i1);
+    uint64_t t11 = x_[(uint32_t)4U * i + (uint32_t)2U];
+    uint64_t t212 = p1[(uint32_t)4U * i + (uint32_t)2U];
+    uint64_t *res_i2 = tempBuffer10 + (uint32_t)4U * i + (uint32_t)2U;
+    c = Lib_IntTypes_Intrinsics_sub_borrow_u64(c, t11, t212, res_i2);
+    uint64_t t13 = x_[(uint32_t)4U * i + (uint32_t)3U];
+    uint64_t t21 = p1[(uint32_t)4U * i + (uint32_t)3U];
+    uint64_t *res_i = tempBuffer10 + (uint32_t)4U * i + (uint32_t)3U;
+    c = Lib_IntTypes_Intrinsics_sub_borrow_u64(c, t13, t21, res_i);
+  }
+  for (uint32_t i = len4 / (uint32_t)4U * (uint32_t)4U; i < len4; i++)
+  {
+    uint64_t t1 = x_[i];
+    uint64_t t21 = p1[i];
+    uint64_t *res_i = tempBuffer10 + i;
+    c = Lib_IntTypes_Intrinsics_sub_borrow_u64(c, t1, t21, res_i);
+  }
+  uint64_t r10 = c;
+  uint64_t carry00 = r10;
+  uint64_t
+  carry1 =
+    Lib_IntTypes_Intrinsics_sub_borrow_u64(carry00,
+      cin0,
+      (uint64_t)0U,
+      &tempBufferForSubborrow);
+  cmovznz4_p384(carry1, tempBuffer10, x_, z1z2);
+  montgomery_multiplication_buffer_dh_p384(z1z2, h0, z3);
+  uint64_t *x3_out = t5;
+  uint64_t *y3_out = t5 + (uint32_t)6U;
+  uint64_t *z3_out = t5 + (uint32_t)12U;
+  uint64_t *temp = t5 + (uint32_t)18U;
+  copy_point_conditional(Spec_ECC_Curves_P384, x3_out, y3_out, z3_out, q, p, temp);
+  copy_point_conditional1(Spec_ECC_Curves_P384, x3_out, y3_out, z3_out, p, q);
+  memcpy(result, x3_out, (uint32_t)6U * sizeof (uint64_t));
+  memcpy(result + (uint32_t)6U, y3_out, (uint32_t)6U * sizeof (uint64_t));
+  memcpy(result + (uint32_t)12U, z3_out, (uint32_t)6U * sizeof (uint64_t));
+}
+
 static const
 uint64_t
-points_radix_16[128U] =
+points_radix_p256_16[128U] =
   {
     (uint64_t)0x0U, (uint64_t)0x0U, (uint64_t)0x0U, (uint64_t)0x0U, (uint64_t)0x0U, (uint64_t)0x0U,
     (uint64_t)0x0U, (uint64_t)0x0U, (uint64_t)0x1fb38ab1388ad777U, (uint64_t)0x1dfee06615fa309dU,
@@ -3016,25 +3895,26 @@ static inline void point_double_p384(uint64_t *p, uint64_t *result, uint64_t *te
   felem_sub_p384(y3, eightGamma, y3);
 }
 
-static inline void getPointPrecomputedMixed_p256(uint8_t *scalar, uint32_t i, uint64_t *pointToAdd)
+static void getPointPrecomputedMixed_p256(void *scalar, uint32_t i, uint64_t *pointToAdd)
 {
   uint32_t half = i >> (uint32_t)1U;
-  uint32_t word = (uint32_t)scalar[half];
+  uint32_t word = (uint32_t)((uint8_t *)scalar)[half];
   uint32_t bitShift = i & (uint32_t)1U;
   uint32_t bitShiftAsPrivate = bitShift;
+  uint32_t leftWord = word >> (uint32_t)0x4U;
+  uint32_t rightWord = word & (uint32_t)0x0fU;
   uint64_t mask0 = (uint64_t)0U - (uint64_t)bitShiftAsPrivate;
-  uint32_t mask2 = (uint32_t)0xf0U ^ (uint32_t)(mask0 & (uint64_t)(uint32_t)255U);
-  uint64_t mask1 = (uint64_t)0U - (uint64_t)bitShift;
-  uint32_t shiftMask = (uint32_t)0x4U ^ (uint32_t)(mask1 & (uint64_t)(uint32_t)4U);
-  uint32_t result = word & mask2;
-  uint32_t bits = result >> shiftMask;
+  uint32_t bits = leftWord ^ (uint32_t)(mask0 & (uint64_t)(leftWord ^ rightWord));
   for (uint32_t i0 = (uint32_t)0U; i0 < (uint32_t)16U; i0++)
   {
     uint64_t mask = FStar_UInt64_eq_mask((uint64_t)bits, (uint64_t)i0);
-    const uint64_t *lut_cmb_x = points_radix_16 + i0 * (uint32_t)8U;
-    const uint64_t *lut_cmb_y = points_radix_16 + i0 * (uint32_t)8U + (uint32_t)4U;
+    uint32_t lenPoint = (uint32_t)8U;
+    uint32_t lenCoordinate = (uint32_t)4U;
+    uint32_t pointLen = (uint32_t)2U * lenCoordinate;
+    const uint64_t *lut_cmb_x = points_radix_p256_16 + i0 * lenPoint * pointLen;
+    const uint64_t *lut_cmb_y = points_radix_p256_16 + i0 * lenPoint * pointLen + lenCoordinate;
     copy_conditional_p256_c(pointToAdd, lut_cmb_x, mask);
-    copy_conditional_p256_c(pointToAdd + (uint32_t)4U, lut_cmb_y, mask);
+    copy_conditional_p256_c(pointToAdd + lenCoordinate, lut_cmb_y, mask);
   }
 }
 
@@ -3404,7 +4284,7 @@ static inline void solinas_reduction_impl_p256(uint64_t *i, uint64_t *o)
     };
   uint32_t len10 = (uint32_t)4U;
   uint64_t c16 = (uint64_t)0U;
-  for (uint32_t i8 = (uint32_t)0U; i8 < len10 / (uint32_t)4U * (uint32_t)4U / (uint32_t)4U; i8++)
+  for (uint32_t i8 = (uint32_t)0U; i8 < len10 / (uint32_t)4U; i8++)
   {
     uint64_t t12 = t01[(uint32_t)4U * i8];
     uint64_t t220 = p0[(uint32_t)4U * i8];
@@ -3464,7 +4344,7 @@ static inline void solinas_reduction_impl_p256(uint64_t *i, uint64_t *o)
     };
   uint32_t len11 = (uint32_t)4U;
   uint64_t c17 = (uint64_t)0U;
-  for (uint32_t i8 = (uint32_t)0U; i8 < len11 / (uint32_t)4U * (uint32_t)4U / (uint32_t)4U; i8++)
+  for (uint32_t i8 = (uint32_t)0U; i8 < len11 / (uint32_t)4U; i8++)
   {
     uint64_t t12 = t110[(uint32_t)4U * i8];
     uint64_t t220 = p1[(uint32_t)4U * i8];
@@ -3541,7 +4421,7 @@ static inline void solinas_reduction_impl_p256(uint64_t *i, uint64_t *o)
     };
   uint32_t len12 = (uint32_t)4U;
   uint64_t c18 = (uint64_t)0U;
-  for (uint32_t i8 = (uint32_t)0U; i8 < len12 / (uint32_t)4U * (uint32_t)4U / (uint32_t)4U; i8++)
+  for (uint32_t i8 = (uint32_t)0U; i8 < len12 / (uint32_t)4U; i8++)
   {
     uint64_t t12 = t310[(uint32_t)4U * i8];
     uint64_t t220 = p2[(uint32_t)4U * i8];
@@ -3604,7 +4484,7 @@ static inline void solinas_reduction_impl_p256(uint64_t *i, uint64_t *o)
     };
   uint32_t len13 = (uint32_t)4U;
   uint64_t c19 = (uint64_t)0U;
-  for (uint32_t i8 = (uint32_t)0U; i8 < len13 / (uint32_t)4U * (uint32_t)4U / (uint32_t)4U; i8++)
+  for (uint32_t i8 = (uint32_t)0U; i8 < len13 / (uint32_t)4U; i8++)
   {
     uint64_t t12 = t410[(uint32_t)4U * i8];
     uint64_t t220 = p3[(uint32_t)4U * i8];
@@ -3664,7 +4544,7 @@ static inline void solinas_reduction_impl_p256(uint64_t *i, uint64_t *o)
     };
   uint32_t len14 = (uint32_t)4U;
   uint64_t c20 = (uint64_t)0U;
-  for (uint32_t i8 = (uint32_t)0U; i8 < len14 / (uint32_t)4U * (uint32_t)4U / (uint32_t)4U; i8++)
+  for (uint32_t i8 = (uint32_t)0U; i8 < len14 / (uint32_t)4U; i8++)
   {
     uint64_t t12 = t510[(uint32_t)4U * i8];
     uint64_t t220 = p4[(uint32_t)4U * i8];
@@ -3724,7 +4604,7 @@ static inline void solinas_reduction_impl_p256(uint64_t *i, uint64_t *o)
     };
   uint32_t len15 = (uint32_t)4U;
   uint64_t c21 = (uint64_t)0U;
-  for (uint32_t i8 = (uint32_t)0U; i8 < len15 / (uint32_t)4U * (uint32_t)4U / (uint32_t)4U; i8++)
+  for (uint32_t i8 = (uint32_t)0U; i8 < len15 / (uint32_t)4U; i8++)
   {
     uint64_t t12 = t610[(uint32_t)4U * i8];
     uint64_t t220 = p5[(uint32_t)4U * i8];
@@ -3787,7 +4667,7 @@ static inline void solinas_reduction_impl_p256(uint64_t *i, uint64_t *o)
     };
   uint32_t len16 = (uint32_t)4U;
   uint64_t c22 = (uint64_t)0U;
-  for (uint32_t i8 = (uint32_t)0U; i8 < len16 / (uint32_t)4U * (uint32_t)4U / (uint32_t)4U; i8++)
+  for (uint32_t i8 = (uint32_t)0U; i8 < len16 / (uint32_t)4U; i8++)
   {
     uint64_t t12 = t710[(uint32_t)4U * i8];
     uint64_t t220 = p6[(uint32_t)4U * i8];
@@ -3850,7 +4730,7 @@ static inline void solinas_reduction_impl_p256(uint64_t *i, uint64_t *o)
     };
   uint32_t len1 = (uint32_t)4U;
   uint64_t c = (uint64_t)0U;
-  for (uint32_t i8 = (uint32_t)0U; i8 < len1 / (uint32_t)4U * (uint32_t)4U / (uint32_t)4U; i8++)
+  for (uint32_t i8 = (uint32_t)0U; i8 < len1 / (uint32_t)4U; i8++)
   {
     uint64_t t12 = t810[(uint32_t)4U * i8];
     uint64_t t220 = p[(uint32_t)4U * i8];
@@ -3991,12 +4871,7 @@ static inline void solinas_reduction_impl_p384(uint64_t *i, uint64_t *o)
     };
   uint32_t len10 = (uint32_t)6U;
   uint64_t c24 = (uint64_t)0U;
-  for
-  (uint32_t
-    i12 = (uint32_t)0U;
-    i12
-    < len10 / (uint32_t)4U * (uint32_t)4U / (uint32_t)4U;
-    i12++)
+  for (uint32_t i12 = (uint32_t)0U; i12 < len10 / (uint32_t)4U; i12++)
   {
     uint64_t t12 = t01[(uint32_t)4U * i12];
     uint64_t t220 = p0[(uint32_t)4U * i12];
@@ -4097,12 +4972,7 @@ static inline void solinas_reduction_impl_p384(uint64_t *i, uint64_t *o)
     };
   uint32_t len11 = (uint32_t)6U;
   uint64_t c25 = (uint64_t)0U;
-  for
-  (uint32_t
-    i12 = (uint32_t)0U;
-    i12
-    < len11 / (uint32_t)4U * (uint32_t)4U / (uint32_t)4U;
-    i12++)
+  for (uint32_t i12 = (uint32_t)0U; i12 < len11 / (uint32_t)4U; i12++)
   {
     uint64_t t12 = t210[(uint32_t)4U * i12];
     uint64_t t220 = p1[(uint32_t)4U * i12];
@@ -4173,12 +5043,7 @@ static inline void solinas_reduction_impl_p384(uint64_t *i, uint64_t *o)
     };
   uint32_t len12 = (uint32_t)6U;
   uint64_t c26 = (uint64_t)0U;
-  for
-  (uint32_t
-    i12 = (uint32_t)0U;
-    i12
-    < len12 / (uint32_t)4U * (uint32_t)4U / (uint32_t)4U;
-    i12++)
+  for (uint32_t i12 = (uint32_t)0U; i12 < len12 / (uint32_t)4U; i12++)
   {
     uint64_t t12 = t310[(uint32_t)4U * i12];
     uint64_t t220 = p2[(uint32_t)4U * i12];
@@ -4249,12 +5114,7 @@ static inline void solinas_reduction_impl_p384(uint64_t *i, uint64_t *o)
     };
   uint32_t len13 = (uint32_t)6U;
   uint64_t c27 = (uint64_t)0U;
-  for
-  (uint32_t
-    i12 = (uint32_t)0U;
-    i12
-    < len13 / (uint32_t)4U * (uint32_t)4U / (uint32_t)4U;
-    i12++)
+  for (uint32_t i12 = (uint32_t)0U; i12 < len13 / (uint32_t)4U; i12++)
   {
     uint64_t t12 = t410[(uint32_t)4U * i12];
     uint64_t t220 = p3[(uint32_t)4U * i12];
@@ -4325,12 +5185,7 @@ static inline void solinas_reduction_impl_p384(uint64_t *i, uint64_t *o)
     };
   uint32_t len14 = (uint32_t)6U;
   uint64_t c28 = (uint64_t)0U;
-  for
-  (uint32_t
-    i12 = (uint32_t)0U;
-    i12
-    < len14 / (uint32_t)4U * (uint32_t)4U / (uint32_t)4U;
-    i12++)
+  for (uint32_t i12 = (uint32_t)0U; i12 < len14 / (uint32_t)4U; i12++)
   {
     uint64_t t12 = t510[(uint32_t)4U * i12];
     uint64_t t220 = p4[(uint32_t)4U * i12];
@@ -4401,12 +5256,7 @@ static inline void solinas_reduction_impl_p384(uint64_t *i, uint64_t *o)
     };
   uint32_t len15 = (uint32_t)6U;
   uint64_t c29 = (uint64_t)0U;
-  for
-  (uint32_t
-    i12 = (uint32_t)0U;
-    i12
-    < len15 / (uint32_t)4U * (uint32_t)4U / (uint32_t)4U;
-    i12++)
+  for (uint32_t i12 = (uint32_t)0U; i12 < len15 / (uint32_t)4U; i12++)
   {
     uint64_t t12 = t610[(uint32_t)4U * i12];
     uint64_t t220 = p5[(uint32_t)4U * i12];
@@ -4477,12 +5327,7 @@ static inline void solinas_reduction_impl_p384(uint64_t *i, uint64_t *o)
     };
   uint32_t len16 = (uint32_t)6U;
   uint64_t c30 = (uint64_t)0U;
-  for
-  (uint32_t
-    i12 = (uint32_t)0U;
-    i12
-    < len16 / (uint32_t)4U * (uint32_t)4U / (uint32_t)4U;
-    i12++)
+  for (uint32_t i12 = (uint32_t)0U; i12 < len16 / (uint32_t)4U; i12++)
   {
     uint64_t t12 = t710[(uint32_t)4U * i12];
     uint64_t t220 = p6[(uint32_t)4U * i12];
@@ -4553,12 +5398,7 @@ static inline void solinas_reduction_impl_p384(uint64_t *i, uint64_t *o)
     };
   uint32_t len17 = (uint32_t)6U;
   uint64_t c31 = (uint64_t)0U;
-  for
-  (uint32_t
-    i12 = (uint32_t)0U;
-    i12
-    < len17 / (uint32_t)4U * (uint32_t)4U / (uint32_t)4U;
-    i12++)
+  for (uint32_t i12 = (uint32_t)0U; i12 < len17 / (uint32_t)4U; i12++)
   {
     uint64_t t12 = t810[(uint32_t)4U * i12];
     uint64_t t220 = p7[(uint32_t)4U * i12];
@@ -4629,12 +5469,7 @@ static inline void solinas_reduction_impl_p384(uint64_t *i, uint64_t *o)
     };
   uint32_t len1 = (uint32_t)6U;
   uint64_t c = (uint64_t)0U;
-  for
-  (uint32_t
-    i12 = (uint32_t)0U;
-    i12
-    < len1 / (uint32_t)4U * (uint32_t)4U / (uint32_t)4U;
-    i12++)
+  for (uint32_t i12 = (uint32_t)0U; i12 < len1 / (uint32_t)4U; i12++)
   {
     uint64_t t12 = t910[(uint32_t)4U * i12];
     uint64_t t220 = p[(uint32_t)4U * i12];
@@ -4767,7 +5602,7 @@ static inline void fromDomain_p256(uint64_t *f, uint64_t *result)
     mul64(f3, t10, o3, o4);
     uint32_t len32 = (uint32_t)4U * (uint32_t)2U;
     uint64_t c = (uint64_t)0U;
-    for (uint32_t i = (uint32_t)0U; i < len32 / (uint32_t)4U * (uint32_t)4U / (uint32_t)4U; i++)
+    for (uint32_t i = (uint32_t)0U; i < len32 / (uint32_t)4U; i++)
     {
       uint64_t t1 = t[(uint32_t)4U * i];
       uint64_t t210 = t2[(uint32_t)4U * i];
@@ -4820,7 +5655,7 @@ static inline void fromDomain_p256(uint64_t *f, uint64_t *result)
     };
   uint32_t len4 = (uint32_t)4U;
   uint64_t c = (uint64_t)0U;
-  for (uint32_t i = (uint32_t)0U; i < len4 / (uint32_t)4U * (uint32_t)4U / (uint32_t)4U; i++)
+  for (uint32_t i = (uint32_t)0U; i < len4 / (uint32_t)4U; i++)
   {
     uint64_t t1 = x_[(uint32_t)4U * i];
     uint64_t t210 = p[(uint32_t)4U * i];
@@ -4898,14 +5733,13 @@ static inline void fromDomain_p384(uint64_t *f, uint64_t *result)
     uint32_t len32 = (uint32_t)6U;
     uint64_t bBuffer = y_;
     uint64_t *partResult = t2;
-    uint32_t resLen = len32 + (uint32_t)1U;
-    memset(partResult, 0U, resLen * sizeof (uint64_t));
+    memset(partResult, 0U, (len32 + (uint32_t)1U) * sizeof (uint64_t));
     for (uint32_t i1 = (uint32_t)0U; i1 < (uint32_t)1U; i1++)
     {
       uint64_t bj = (&bBuffer)[i1];
       uint64_t *res_j = partResult + i1;
       uint64_t c = (uint64_t)0U;
-      for (uint32_t i = (uint32_t)0U; i < len32 / (uint32_t)4U * (uint32_t)4U / (uint32_t)4U; i++)
+      for (uint32_t i = (uint32_t)0U; i < len32 / (uint32_t)4U; i++)
       {
         uint64_t a_i = p[(uint32_t)4U * i];
         uint64_t *res_i0 = res_j + (uint32_t)4U * i;
@@ -4931,7 +5765,7 @@ static inline void fromDomain_p384(uint64_t *f, uint64_t *result)
     }
     uint32_t len33 = (uint32_t)6U * (uint32_t)2U;
     uint64_t c = (uint64_t)0U;
-    for (uint32_t i = (uint32_t)0U; i < len33 / (uint32_t)4U * (uint32_t)4U / (uint32_t)4U; i++)
+    for (uint32_t i = (uint32_t)0U; i < len33 / (uint32_t)4U; i++)
     {
       uint64_t t1 = t[(uint32_t)4U * i];
       uint64_t t210 = t2[(uint32_t)4U * i];
@@ -4982,7 +5816,7 @@ static inline void fromDomain_p384(uint64_t *f, uint64_t *result)
     };
   uint32_t len4 = (uint32_t)6U;
   uint64_t c = (uint64_t)0U;
-  for (uint32_t i = (uint32_t)0U; i < len4 / (uint32_t)4U * (uint32_t)4U / (uint32_t)4U; i++)
+  for (uint32_t i = (uint32_t)0U; i < len4 / (uint32_t)4U; i++)
   {
     uint64_t t1 = x_[(uint32_t)4U * i];
     uint64_t t210 = p[(uint32_t)4U * i];
@@ -5431,7 +6265,7 @@ static bool verifyQValidCurvePoint_p256(uint64_t *pubKey)
     };
   uint32_t len10 = (uint32_t)4U;
   uint64_t c0 = (uint64_t)0U;
-  for (uint32_t i = (uint32_t)0U; i < len10 / (uint32_t)4U * (uint32_t)4U / (uint32_t)4U; i++)
+  for (uint32_t i = (uint32_t)0U; i < len10 / (uint32_t)4U; i++)
   {
     uint64_t t1 = x[(uint32_t)4U * i];
     uint64_t t20 = p0[(uint32_t)4U * i];
@@ -5469,7 +6303,7 @@ static bool verifyQValidCurvePoint_p256(uint64_t *pubKey)
     };
   uint32_t len1 = (uint32_t)4U;
   uint64_t c = (uint64_t)0U;
-  for (uint32_t i = (uint32_t)0U; i < len1 / (uint32_t)4U * (uint32_t)4U / (uint32_t)4U; i++)
+  for (uint32_t i = (uint32_t)0U; i < len1 / (uint32_t)4U; i++)
   {
     uint64_t t1 = y[(uint32_t)4U * i];
     uint64_t t20 = p[(uint32_t)4U * i];
@@ -5524,7 +6358,7 @@ static bool verifyQValidCurvePoint_p384(uint64_t *pubKey)
     };
   uint32_t len10 = (uint32_t)6U;
   uint64_t c0 = (uint64_t)0U;
-  for (uint32_t i = (uint32_t)0U; i < len10 / (uint32_t)4U * (uint32_t)4U / (uint32_t)4U; i++)
+  for (uint32_t i = (uint32_t)0U; i < len10 / (uint32_t)4U; i++)
   {
     uint64_t t1 = x[(uint32_t)4U * i];
     uint64_t t20 = p0[(uint32_t)4U * i];
@@ -5560,7 +6394,7 @@ static bool verifyQValidCurvePoint_p384(uint64_t *pubKey)
     };
   uint32_t len1 = (uint32_t)6U;
   uint64_t c = (uint64_t)0U;
-  for (uint32_t i = (uint32_t)0U; i < len1 / (uint32_t)4U * (uint32_t)4U / (uint32_t)4U; i++)
+  for (uint32_t i = (uint32_t)0U; i < len1 / (uint32_t)4U; i++)
   {
     uint64_t t1 = y[(uint32_t)4U * i];
     uint64_t t20 = p[(uint32_t)4U * i];
@@ -6287,7 +7121,7 @@ Hacl_P256_ecdsa_verif_p256_sha2(
       };
     uint32_t len31 = (uint32_t)4U;
     uint64_t c1 = (uint64_t)0U;
-    for (uint32_t i = (uint32_t)0U; i < len31 / (uint32_t)4U * (uint32_t)4U / (uint32_t)4U; i++)
+    for (uint32_t i = (uint32_t)0U; i < len31 / (uint32_t)4U; i++)
     {
       uint64_t t1 = rAsFelem[(uint32_t)4U * i];
       uint64_t t20 = p0[(uint32_t)4U * i];
@@ -6342,7 +7176,7 @@ Hacl_P256_ecdsa_verif_p256_sha2(
       };
     uint32_t len33 = (uint32_t)4U;
     uint64_t c2 = (uint64_t)0U;
-    for (uint32_t i = (uint32_t)0U; i < len33 / (uint32_t)4U * (uint32_t)4U / (uint32_t)4U; i++)
+    for (uint32_t i = (uint32_t)0U; i < len33 / (uint32_t)4U; i++)
     {
       uint64_t t1 = sAsFelem[(uint32_t)4U * i];
       uint64_t t20 = p2[(uint32_t)4U * i];
@@ -6540,15 +7374,14 @@ Hacl_P256_ecdsa_verif_p256_sha2(
       uint64_t t[(uint32_t)2U * len6];
       memset(t, 0U, (uint32_t)2U * len6 * sizeof (uint64_t));
       uint32_t len70 = (uint32_t)4U;
-      uint32_t resLen0 = len70 + len70;
-      memset(t, 0U, resLen0 * sizeof (uint64_t));
+      memset(t, 0U, (len70 + len70) * sizeof (uint64_t));
       for (uint32_t i0 = (uint32_t)0U; i0 < len70; i0++)
       {
         uint64_t *ab = z1;
         uint64_t a_j = z1[i0];
         uint64_t *res_j = t + i0;
         uint64_t c = (uint64_t)0U;
-        for (uint32_t i = (uint32_t)0U; i < i0 / (uint32_t)4U * (uint32_t)4U / (uint32_t)4U; i++)
+        for (uint32_t i = (uint32_t)0U; i < i0 / (uint32_t)4U; i++)
         {
           uint64_t a_i = ab[(uint32_t)4U * i];
           uint64_t *res_i0 = res_j + (uint32_t)4U * i;
@@ -6572,10 +7405,10 @@ Hacl_P256_ecdsa_verif_p256_sha2(
         uint64_t r12 = c;
         t[i0 + i0] = r12;
       }
-      uint64_t c00 = bn_add_eq_len_u64(resLen0, t, t, t);
-      KRML_CHECK_SIZE(sizeof (uint64_t), resLen0);
-      uint64_t tmp3[resLen0];
-      memset(tmp3, 0U, resLen0 * sizeof (uint64_t));
+      uint64_t c00 = bn_add_eq_len_u64(len70 + len70, t, t, t);
+      KRML_CHECK_SIZE(sizeof (uint64_t), len70 + len70);
+      uint64_t tmp3[len70 + len70];
+      memset(tmp3, 0U, (len70 + len70) * sizeof (uint64_t));
       for (uint32_t i = (uint32_t)0U; i < len70; i++)
       {
         uint128_t res = (uint128_t)z1[i] * z1[i];
@@ -6584,7 +7417,7 @@ Hacl_P256_ecdsa_verif_p256_sha2(
         tmp3[(uint32_t)2U * i] = lo;
         tmp3[(uint32_t)2U * i + (uint32_t)1U] = hi;
       }
-      uint64_t c10 = bn_add_eq_len_u64(resLen0, t, tmp3, t);
+      uint64_t c10 = bn_add_eq_len_u64(len70 + len70, t, tmp3, t);
       uint32_t len71 = (uint32_t)4U;
       KRML_CHECK_SIZE(sizeof (uint64_t), (uint32_t)2U * len71);
       uint64_t t20[(uint32_t)2U * len71];
@@ -6623,7 +7456,7 @@ Hacl_P256_ecdsa_verif_p256_sha2(
         mul64(f3, t10, o3, o4);
         uint32_t len92 = (uint32_t)4U * (uint32_t)2U;
         uint64_t c = (uint64_t)0U;
-        for (uint32_t i = (uint32_t)0U; i < len92 / (uint32_t)4U * (uint32_t)4U / (uint32_t)4U; i++)
+        for (uint32_t i = (uint32_t)0U; i < len92 / (uint32_t)4U; i++)
         {
           uint64_t t1 = t[(uint32_t)4U * i];
           uint64_t t210 = t20[(uint32_t)4U * i];
@@ -6676,7 +7509,7 @@ Hacl_P256_ecdsa_verif_p256_sha2(
         };
       uint32_t len100 = (uint32_t)4U;
       uint64_t c3 = (uint64_t)0U;
-      for (uint32_t i = (uint32_t)0U; i < len100 / (uint32_t)4U * (uint32_t)4U / (uint32_t)4U; i++)
+      for (uint32_t i = (uint32_t)0U; i < len100 / (uint32_t)4U; i++)
       {
         uint64_t t1 = x_0[(uint32_t)4U * i];
         uint64_t t210 = p10[(uint32_t)4U * i];
@@ -6716,15 +7549,14 @@ Hacl_P256_ecdsa_verif_p256_sha2(
       uint64_t t0[(uint32_t)2U * len64];
       memset(t0, 0U, (uint32_t)2U * len64 * sizeof (uint64_t));
       uint32_t len72 = (uint32_t)4U;
-      uint32_t resLen1 = len72 + len72;
-      memset(t0, 0U, resLen1 * sizeof (uint64_t));
+      memset(t0, 0U, (len72 + len72) * sizeof (uint64_t));
       for (uint32_t i0 = (uint32_t)0U; i0 < len72; i0++)
       {
         uint64_t *ab = z2;
         uint64_t a_j = z2[i0];
         uint64_t *res_j = t0 + i0;
         uint64_t c = (uint64_t)0U;
-        for (uint32_t i = (uint32_t)0U; i < i0 / (uint32_t)4U * (uint32_t)4U / (uint32_t)4U; i++)
+        for (uint32_t i = (uint32_t)0U; i < i0 / (uint32_t)4U; i++)
         {
           uint64_t a_i = ab[(uint32_t)4U * i];
           uint64_t *res_i0 = res_j + (uint32_t)4U * i;
@@ -6748,10 +7580,10 @@ Hacl_P256_ecdsa_verif_p256_sha2(
         uint64_t r13 = c;
         t0[i0 + i0] = r13;
       }
-      uint64_t c0 = bn_add_eq_len_u64(resLen1, t0, t0, t0);
-      KRML_CHECK_SIZE(sizeof (uint64_t), resLen1);
-      uint64_t tmp4[resLen1];
-      memset(tmp4, 0U, resLen1 * sizeof (uint64_t));
+      uint64_t c0 = bn_add_eq_len_u64(len72 + len72, t0, t0, t0);
+      KRML_CHECK_SIZE(sizeof (uint64_t), len72 + len72);
+      uint64_t tmp4[len72 + len72];
+      memset(tmp4, 0U, (len72 + len72) * sizeof (uint64_t));
       for (uint32_t i = (uint32_t)0U; i < len72; i++)
       {
         uint128_t res = (uint128_t)z2[i] * z2[i];
@@ -6760,7 +7592,7 @@ Hacl_P256_ecdsa_verif_p256_sha2(
         tmp4[(uint32_t)2U * i] = lo;
         tmp4[(uint32_t)2U * i + (uint32_t)1U] = hi;
       }
-      uint64_t c11 = bn_add_eq_len_u64(resLen1, t0, tmp4, t0);
+      uint64_t c11 = bn_add_eq_len_u64(len72 + len72, t0, tmp4, t0);
       uint32_t len73 = (uint32_t)4U;
       KRML_CHECK_SIZE(sizeof (uint64_t), (uint32_t)2U * len73);
       uint64_t t22[(uint32_t)2U * len73];
@@ -6799,7 +7631,7 @@ Hacl_P256_ecdsa_verif_p256_sha2(
         mul64(f3, t10, o3, o4);
         uint32_t len93 = (uint32_t)4U * (uint32_t)2U;
         uint64_t c = (uint64_t)0U;
-        for (uint32_t i = (uint32_t)0U; i < len93 / (uint32_t)4U * (uint32_t)4U / (uint32_t)4U; i++)
+        for (uint32_t i = (uint32_t)0U; i < len93 / (uint32_t)4U; i++)
         {
           uint64_t t1 = t0[(uint32_t)4U * i];
           uint64_t t210 = t22[(uint32_t)4U * i];
@@ -6852,7 +7684,7 @@ Hacl_P256_ecdsa_verif_p256_sha2(
         };
       uint32_t len101 = (uint32_t)4U;
       uint64_t c4 = (uint64_t)0U;
-      for (uint32_t i = (uint32_t)0U; i < len101 / (uint32_t)4U * (uint32_t)4U / (uint32_t)4U; i++)
+      for (uint32_t i = (uint32_t)0U; i < len101 / (uint32_t)4U; i++)
       {
         uint64_t t1 = x_1[(uint32_t)4U * i];
         uint64_t t210 = p11[(uint32_t)4U * i];
@@ -6892,14 +7724,13 @@ Hacl_P256_ecdsa_verif_p256_sha2(
       uint64_t t3[(uint32_t)2U * len65];
       memset(t3, 0U, (uint32_t)2U * len65 * sizeof (uint64_t));
       uint32_t len74 = (uint32_t)4U;
-      uint32_t resLen2 = len74 + len74;
-      memset(t3, 0U, resLen2 * sizeof (uint64_t));
+      memset(t3, 0U, (len74 + len74) * sizeof (uint64_t));
       for (uint32_t i0 = (uint32_t)0U; i0 < len74; i0++)
       {
         uint64_t bj = z1[i0];
         uint64_t *res_j = t3 + i0;
         uint64_t c = (uint64_t)0U;
-        for (uint32_t i = (uint32_t)0U; i < len74 / (uint32_t)4U * (uint32_t)4U / (uint32_t)4U; i++)
+        for (uint32_t i = (uint32_t)0U; i < len74 / (uint32_t)4U; i++)
         {
           uint64_t a_i = sq_z1[(uint32_t)4U * i];
           uint64_t *res_i0 = res_j + (uint32_t)4U * i;
@@ -6961,7 +7792,7 @@ Hacl_P256_ecdsa_verif_p256_sha2(
         mul64(f3, t10, o3, o4);
         uint32_t len94 = (uint32_t)4U * (uint32_t)2U;
         uint64_t c = (uint64_t)0U;
-        for (uint32_t i = (uint32_t)0U; i < len94 / (uint32_t)4U * (uint32_t)4U / (uint32_t)4U; i++)
+        for (uint32_t i = (uint32_t)0U; i < len94 / (uint32_t)4U; i++)
         {
           uint64_t t1 = t3[(uint32_t)4U * i];
           uint64_t t210 = t23[(uint32_t)4U * i];
@@ -7014,7 +7845,7 @@ Hacl_P256_ecdsa_verif_p256_sha2(
         };
       uint32_t len102 = (uint32_t)4U;
       uint64_t c5 = (uint64_t)0U;
-      for (uint32_t i = (uint32_t)0U; i < len102 / (uint32_t)4U * (uint32_t)4U / (uint32_t)4U; i++)
+      for (uint32_t i = (uint32_t)0U; i < len102 / (uint32_t)4U; i++)
       {
         uint64_t t1 = x_2[(uint32_t)4U * i];
         uint64_t t210 = p12[(uint32_t)4U * i];
@@ -7054,14 +7885,13 @@ Hacl_P256_ecdsa_verif_p256_sha2(
       uint64_t t4[(uint32_t)2U * len66];
       memset(t4, 0U, (uint32_t)2U * len66 * sizeof (uint64_t));
       uint32_t len76 = (uint32_t)4U;
-      uint32_t resLen3 = len76 + len76;
-      memset(t4, 0U, resLen3 * sizeof (uint64_t));
+      memset(t4, 0U, (len76 + len76) * sizeof (uint64_t));
       for (uint32_t i0 = (uint32_t)0U; i0 < len76; i0++)
       {
         uint64_t bj = z2[i0];
         uint64_t *res_j = t4 + i0;
         uint64_t c = (uint64_t)0U;
-        for (uint32_t i = (uint32_t)0U; i < len76 / (uint32_t)4U * (uint32_t)4U / (uint32_t)4U; i++)
+        for (uint32_t i = (uint32_t)0U; i < len76 / (uint32_t)4U; i++)
         {
           uint64_t a_i = sq_z2[(uint32_t)4U * i];
           uint64_t *res_i0 = res_j + (uint32_t)4U * i;
@@ -7123,7 +7953,7 @@ Hacl_P256_ecdsa_verif_p256_sha2(
         mul64(f3, t10, o3, o4);
         uint32_t len95 = (uint32_t)4U * (uint32_t)2U;
         uint64_t c = (uint64_t)0U;
-        for (uint32_t i = (uint32_t)0U; i < len95 / (uint32_t)4U * (uint32_t)4U / (uint32_t)4U; i++)
+        for (uint32_t i = (uint32_t)0U; i < len95 / (uint32_t)4U; i++)
         {
           uint64_t t1 = t4[(uint32_t)4U * i];
           uint64_t t210 = t24[(uint32_t)4U * i];
@@ -7176,7 +8006,7 @@ Hacl_P256_ecdsa_verif_p256_sha2(
         };
       uint32_t len103 = (uint32_t)4U;
       uint64_t c6 = (uint64_t)0U;
-      for (uint32_t i = (uint32_t)0U; i < len103 / (uint32_t)4U * (uint32_t)4U / (uint32_t)4U; i++)
+      for (uint32_t i = (uint32_t)0U; i < len103 / (uint32_t)4U; i++)
       {
         uint64_t t1 = x_3[(uint32_t)4U * i];
         uint64_t t210 = p13[(uint32_t)4U * i];
@@ -7216,14 +8046,13 @@ Hacl_P256_ecdsa_verif_p256_sha2(
       uint64_t t5[(uint32_t)2U * len67];
       memset(t5, 0U, (uint32_t)2U * len67 * sizeof (uint64_t));
       uint32_t len78 = (uint32_t)4U;
-      uint32_t resLen4 = len78 + len78;
-      memset(t5, 0U, resLen4 * sizeof (uint64_t));
+      memset(t5, 0U, (len78 + len78) * sizeof (uint64_t));
       for (uint32_t i0 = (uint32_t)0U; i0 < len78; i0++)
       {
         uint64_t bj = x2[i0];
         uint64_t *res_j = t5 + i0;
         uint64_t c = (uint64_t)0U;
-        for (uint32_t i = (uint32_t)0U; i < len78 / (uint32_t)4U * (uint32_t)4U / (uint32_t)4U; i++)
+        for (uint32_t i = (uint32_t)0U; i < len78 / (uint32_t)4U; i++)
         {
           uint64_t a_i = sq_z1[(uint32_t)4U * i];
           uint64_t *res_i0 = res_j + (uint32_t)4U * i;
@@ -7285,7 +8114,7 @@ Hacl_P256_ecdsa_verif_p256_sha2(
         mul64(f3, t10, o3, o4);
         uint32_t len96 = (uint32_t)4U * (uint32_t)2U;
         uint64_t c = (uint64_t)0U;
-        for (uint32_t i = (uint32_t)0U; i < len96 / (uint32_t)4U * (uint32_t)4U / (uint32_t)4U; i++)
+        for (uint32_t i = (uint32_t)0U; i < len96 / (uint32_t)4U; i++)
         {
           uint64_t t1 = t5[(uint32_t)4U * i];
           uint64_t t210 = t25[(uint32_t)4U * i];
@@ -7338,7 +8167,7 @@ Hacl_P256_ecdsa_verif_p256_sha2(
         };
       uint32_t len104 = (uint32_t)4U;
       uint64_t c7 = (uint64_t)0U;
-      for (uint32_t i = (uint32_t)0U; i < len104 / (uint32_t)4U * (uint32_t)4U / (uint32_t)4U; i++)
+      for (uint32_t i = (uint32_t)0U; i < len104 / (uint32_t)4U; i++)
       {
         uint64_t t1 = x_4[(uint32_t)4U * i];
         uint64_t t210 = p14[(uint32_t)4U * i];
@@ -7378,19 +8207,13 @@ Hacl_P256_ecdsa_verif_p256_sha2(
       uint64_t t6[(uint32_t)2U * len68];
       memset(t6, 0U, (uint32_t)2U * len68 * sizeof (uint64_t));
       uint32_t len710 = (uint32_t)4U;
-      uint32_t resLen5 = len710 + len710;
-      memset(t6, 0U, resLen5 * sizeof (uint64_t));
+      memset(t6, 0U, (len710 + len710) * sizeof (uint64_t));
       for (uint32_t i0 = (uint32_t)0U; i0 < len710; i0++)
       {
         uint64_t bj = x1[i0];
         uint64_t *res_j = t6 + i0;
         uint64_t c = (uint64_t)0U;
-        for
-        (uint32_t
-          i = (uint32_t)0U;
-          i
-          < len710 / (uint32_t)4U * (uint32_t)4U / (uint32_t)4U;
-          i++)
+        for (uint32_t i = (uint32_t)0U; i < len710 / (uint32_t)4U; i++)
         {
           uint64_t a_i = sq_z2[(uint32_t)4U * i];
           uint64_t *res_i0 = res_j + (uint32_t)4U * i;
@@ -7452,7 +8275,7 @@ Hacl_P256_ecdsa_verif_p256_sha2(
         mul64(f3, t10, o3, o4);
         uint32_t len97 = (uint32_t)4U * (uint32_t)2U;
         uint64_t c = (uint64_t)0U;
-        for (uint32_t i = (uint32_t)0U; i < len97 / (uint32_t)4U * (uint32_t)4U / (uint32_t)4U; i++)
+        for (uint32_t i = (uint32_t)0U; i < len97 / (uint32_t)4U; i++)
         {
           uint64_t t1 = t6[(uint32_t)4U * i];
           uint64_t t210 = t26[(uint32_t)4U * i];
@@ -7505,7 +8328,7 @@ Hacl_P256_ecdsa_verif_p256_sha2(
         };
       uint32_t len105 = (uint32_t)4U;
       uint64_t c8 = (uint64_t)0U;
-      for (uint32_t i = (uint32_t)0U; i < len105 / (uint32_t)4U * (uint32_t)4U / (uint32_t)4U; i++)
+      for (uint32_t i = (uint32_t)0U; i < len105 / (uint32_t)4U; i++)
       {
         uint64_t t1 = x_5[(uint32_t)4U * i];
         uint64_t t210 = p15[(uint32_t)4U * i];
@@ -7545,19 +8368,13 @@ Hacl_P256_ecdsa_verif_p256_sha2(
       uint64_t t7[(uint32_t)2U * len69];
       memset(t7, 0U, (uint32_t)2U * len69 * sizeof (uint64_t));
       uint32_t len712 = (uint32_t)4U;
-      uint32_t resLen6 = len712 + len712;
-      memset(t7, 0U, resLen6 * sizeof (uint64_t));
+      memset(t7, 0U, (len712 + len712) * sizeof (uint64_t));
       for (uint32_t i0 = (uint32_t)0U; i0 < len712; i0++)
       {
         uint64_t bj = y2[i0];
         uint64_t *res_j = t7 + i0;
         uint64_t c = (uint64_t)0U;
-        for
-        (uint32_t
-          i = (uint32_t)0U;
-          i
-          < len712 / (uint32_t)4U * (uint32_t)4U / (uint32_t)4U;
-          i++)
+        for (uint32_t i = (uint32_t)0U; i < len712 / (uint32_t)4U; i++)
         {
           uint64_t a_i = tr_z1[(uint32_t)4U * i];
           uint64_t *res_i0 = res_j + (uint32_t)4U * i;
@@ -7619,7 +8436,7 @@ Hacl_P256_ecdsa_verif_p256_sha2(
         mul64(f3, t10, o3, o4);
         uint32_t len98 = (uint32_t)4U * (uint32_t)2U;
         uint64_t c = (uint64_t)0U;
-        for (uint32_t i = (uint32_t)0U; i < len98 / (uint32_t)4U * (uint32_t)4U / (uint32_t)4U; i++)
+        for (uint32_t i = (uint32_t)0U; i < len98 / (uint32_t)4U; i++)
         {
           uint64_t t1 = t7[(uint32_t)4U * i];
           uint64_t t210 = t27[(uint32_t)4U * i];
@@ -7672,7 +8489,7 @@ Hacl_P256_ecdsa_verif_p256_sha2(
         };
       uint32_t len106 = (uint32_t)4U;
       uint64_t c9 = (uint64_t)0U;
-      for (uint32_t i = (uint32_t)0U; i < len106 / (uint32_t)4U * (uint32_t)4U / (uint32_t)4U; i++)
+      for (uint32_t i = (uint32_t)0U; i < len106 / (uint32_t)4U; i++)
       {
         uint64_t t1 = x_6[(uint32_t)4U * i];
         uint64_t t210 = p16[(uint32_t)4U * i];
@@ -7712,14 +8529,13 @@ Hacl_P256_ecdsa_verif_p256_sha2(
       uint64_t t8[(uint32_t)2U * len610];
       memset(t8, 0U, (uint32_t)2U * len610 * sizeof (uint64_t));
       uint32_t len7 = (uint32_t)4U;
-      uint32_t resLen = len7 + len7;
-      memset(t8, 0U, resLen * sizeof (uint64_t));
+      memset(t8, 0U, (len7 + len7) * sizeof (uint64_t));
       for (uint32_t i0 = (uint32_t)0U; i0 < len7; i0++)
       {
         uint64_t bj = y1[i0];
         uint64_t *res_j = t8 + i0;
         uint64_t c = (uint64_t)0U;
-        for (uint32_t i = (uint32_t)0U; i < len7 / (uint32_t)4U * (uint32_t)4U / (uint32_t)4U; i++)
+        for (uint32_t i = (uint32_t)0U; i < len7 / (uint32_t)4U; i++)
         {
           uint64_t a_i = tr_z2[(uint32_t)4U * i];
           uint64_t *res_i0 = res_j + (uint32_t)4U * i;
@@ -7781,7 +8597,7 @@ Hacl_P256_ecdsa_verif_p256_sha2(
         mul64(f3, t10, o3, o4);
         uint32_t len99 = (uint32_t)4U * (uint32_t)2U;
         uint64_t c = (uint64_t)0U;
-        for (uint32_t i = (uint32_t)0U; i < len99 / (uint32_t)4U * (uint32_t)4U / (uint32_t)4U; i++)
+        for (uint32_t i = (uint32_t)0U; i < len99 / (uint32_t)4U; i++)
         {
           uint64_t t1 = t8[(uint32_t)4U * i];
           uint64_t t210 = t2[(uint32_t)4U * i];
@@ -7834,7 +8650,7 @@ Hacl_P256_ecdsa_verif_p256_sha2(
         };
       uint32_t len10 = (uint32_t)4U;
       uint64_t c = (uint64_t)0U;
-      for (uint32_t i = (uint32_t)0U; i < len10 / (uint32_t)4U * (uint32_t)4U / (uint32_t)4U; i++)
+      for (uint32_t i = (uint32_t)0U; i < len10 / (uint32_t)4U; i++)
       {
         uint64_t t1 = x_[(uint32_t)4U * i];
         uint64_t t210 = p1[(uint32_t)4U * i];
@@ -8038,7 +8854,7 @@ Hacl_P256_ecdsa_verif_p256_sha384(
       };
     uint32_t len31 = (uint32_t)4U;
     uint64_t c1 = (uint64_t)0U;
-    for (uint32_t i = (uint32_t)0U; i < len31 / (uint32_t)4U * (uint32_t)4U / (uint32_t)4U; i++)
+    for (uint32_t i = (uint32_t)0U; i < len31 / (uint32_t)4U; i++)
     {
       uint64_t t1 = rAsFelem[(uint32_t)4U * i];
       uint64_t t20 = p0[(uint32_t)4U * i];
@@ -8093,7 +8909,7 @@ Hacl_P256_ecdsa_verif_p256_sha384(
       };
     uint32_t len33 = (uint32_t)4U;
     uint64_t c2 = (uint64_t)0U;
-    for (uint32_t i = (uint32_t)0U; i < len33 / (uint32_t)4U * (uint32_t)4U / (uint32_t)4U; i++)
+    for (uint32_t i = (uint32_t)0U; i < len33 / (uint32_t)4U; i++)
     {
       uint64_t t1 = sAsFelem[(uint32_t)4U * i];
       uint64_t t20 = p2[(uint32_t)4U * i];
@@ -8291,15 +9107,14 @@ Hacl_P256_ecdsa_verif_p256_sha384(
       uint64_t t[(uint32_t)2U * len6];
       memset(t, 0U, (uint32_t)2U * len6 * sizeof (uint64_t));
       uint32_t len70 = (uint32_t)4U;
-      uint32_t resLen0 = len70 + len70;
-      memset(t, 0U, resLen0 * sizeof (uint64_t));
+      memset(t, 0U, (len70 + len70) * sizeof (uint64_t));
       for (uint32_t i0 = (uint32_t)0U; i0 < len70; i0++)
       {
         uint64_t *ab = z1;
         uint64_t a_j = z1[i0];
         uint64_t *res_j = t + i0;
         uint64_t c = (uint64_t)0U;
-        for (uint32_t i = (uint32_t)0U; i < i0 / (uint32_t)4U * (uint32_t)4U / (uint32_t)4U; i++)
+        for (uint32_t i = (uint32_t)0U; i < i0 / (uint32_t)4U; i++)
         {
           uint64_t a_i = ab[(uint32_t)4U * i];
           uint64_t *res_i0 = res_j + (uint32_t)4U * i;
@@ -8323,10 +9138,10 @@ Hacl_P256_ecdsa_verif_p256_sha384(
         uint64_t r12 = c;
         t[i0 + i0] = r12;
       }
-      uint64_t c00 = bn_add_eq_len_u64(resLen0, t, t, t);
-      KRML_CHECK_SIZE(sizeof (uint64_t), resLen0);
-      uint64_t tmp3[resLen0];
-      memset(tmp3, 0U, resLen0 * sizeof (uint64_t));
+      uint64_t c00 = bn_add_eq_len_u64(len70 + len70, t, t, t);
+      KRML_CHECK_SIZE(sizeof (uint64_t), len70 + len70);
+      uint64_t tmp3[len70 + len70];
+      memset(tmp3, 0U, (len70 + len70) * sizeof (uint64_t));
       for (uint32_t i = (uint32_t)0U; i < len70; i++)
       {
         uint128_t res = (uint128_t)z1[i] * z1[i];
@@ -8335,7 +9150,7 @@ Hacl_P256_ecdsa_verif_p256_sha384(
         tmp3[(uint32_t)2U * i] = lo;
         tmp3[(uint32_t)2U * i + (uint32_t)1U] = hi;
       }
-      uint64_t c10 = bn_add_eq_len_u64(resLen0, t, tmp3, t);
+      uint64_t c10 = bn_add_eq_len_u64(len70 + len70, t, tmp3, t);
       uint32_t len71 = (uint32_t)4U;
       KRML_CHECK_SIZE(sizeof (uint64_t), (uint32_t)2U * len71);
       uint64_t t20[(uint32_t)2U * len71];
@@ -8374,7 +9189,7 @@ Hacl_P256_ecdsa_verif_p256_sha384(
         mul64(f3, t10, o3, o4);
         uint32_t len92 = (uint32_t)4U * (uint32_t)2U;
         uint64_t c = (uint64_t)0U;
-        for (uint32_t i = (uint32_t)0U; i < len92 / (uint32_t)4U * (uint32_t)4U / (uint32_t)4U; i++)
+        for (uint32_t i = (uint32_t)0U; i < len92 / (uint32_t)4U; i++)
         {
           uint64_t t1 = t[(uint32_t)4U * i];
           uint64_t t210 = t20[(uint32_t)4U * i];
@@ -8427,7 +9242,7 @@ Hacl_P256_ecdsa_verif_p256_sha384(
         };
       uint32_t len100 = (uint32_t)4U;
       uint64_t c3 = (uint64_t)0U;
-      for (uint32_t i = (uint32_t)0U; i < len100 / (uint32_t)4U * (uint32_t)4U / (uint32_t)4U; i++)
+      for (uint32_t i = (uint32_t)0U; i < len100 / (uint32_t)4U; i++)
       {
         uint64_t t1 = x_0[(uint32_t)4U * i];
         uint64_t t210 = p10[(uint32_t)4U * i];
@@ -8467,15 +9282,14 @@ Hacl_P256_ecdsa_verif_p256_sha384(
       uint64_t t0[(uint32_t)2U * len64];
       memset(t0, 0U, (uint32_t)2U * len64 * sizeof (uint64_t));
       uint32_t len72 = (uint32_t)4U;
-      uint32_t resLen1 = len72 + len72;
-      memset(t0, 0U, resLen1 * sizeof (uint64_t));
+      memset(t0, 0U, (len72 + len72) * sizeof (uint64_t));
       for (uint32_t i0 = (uint32_t)0U; i0 < len72; i0++)
       {
         uint64_t *ab = z2;
         uint64_t a_j = z2[i0];
         uint64_t *res_j = t0 + i0;
         uint64_t c = (uint64_t)0U;
-        for (uint32_t i = (uint32_t)0U; i < i0 / (uint32_t)4U * (uint32_t)4U / (uint32_t)4U; i++)
+        for (uint32_t i = (uint32_t)0U; i < i0 / (uint32_t)4U; i++)
         {
           uint64_t a_i = ab[(uint32_t)4U * i];
           uint64_t *res_i0 = res_j + (uint32_t)4U * i;
@@ -8499,10 +9313,10 @@ Hacl_P256_ecdsa_verif_p256_sha384(
         uint64_t r13 = c;
         t0[i0 + i0] = r13;
       }
-      uint64_t c0 = bn_add_eq_len_u64(resLen1, t0, t0, t0);
-      KRML_CHECK_SIZE(sizeof (uint64_t), resLen1);
-      uint64_t tmp4[resLen1];
-      memset(tmp4, 0U, resLen1 * sizeof (uint64_t));
+      uint64_t c0 = bn_add_eq_len_u64(len72 + len72, t0, t0, t0);
+      KRML_CHECK_SIZE(sizeof (uint64_t), len72 + len72);
+      uint64_t tmp4[len72 + len72];
+      memset(tmp4, 0U, (len72 + len72) * sizeof (uint64_t));
       for (uint32_t i = (uint32_t)0U; i < len72; i++)
       {
         uint128_t res = (uint128_t)z2[i] * z2[i];
@@ -8511,7 +9325,7 @@ Hacl_P256_ecdsa_verif_p256_sha384(
         tmp4[(uint32_t)2U * i] = lo;
         tmp4[(uint32_t)2U * i + (uint32_t)1U] = hi;
       }
-      uint64_t c11 = bn_add_eq_len_u64(resLen1, t0, tmp4, t0);
+      uint64_t c11 = bn_add_eq_len_u64(len72 + len72, t0, tmp4, t0);
       uint32_t len73 = (uint32_t)4U;
       KRML_CHECK_SIZE(sizeof (uint64_t), (uint32_t)2U * len73);
       uint64_t t22[(uint32_t)2U * len73];
@@ -8550,7 +9364,7 @@ Hacl_P256_ecdsa_verif_p256_sha384(
         mul64(f3, t10, o3, o4);
         uint32_t len93 = (uint32_t)4U * (uint32_t)2U;
         uint64_t c = (uint64_t)0U;
-        for (uint32_t i = (uint32_t)0U; i < len93 / (uint32_t)4U * (uint32_t)4U / (uint32_t)4U; i++)
+        for (uint32_t i = (uint32_t)0U; i < len93 / (uint32_t)4U; i++)
         {
           uint64_t t1 = t0[(uint32_t)4U * i];
           uint64_t t210 = t22[(uint32_t)4U * i];
@@ -8603,7 +9417,7 @@ Hacl_P256_ecdsa_verif_p256_sha384(
         };
       uint32_t len101 = (uint32_t)4U;
       uint64_t c4 = (uint64_t)0U;
-      for (uint32_t i = (uint32_t)0U; i < len101 / (uint32_t)4U * (uint32_t)4U / (uint32_t)4U; i++)
+      for (uint32_t i = (uint32_t)0U; i < len101 / (uint32_t)4U; i++)
       {
         uint64_t t1 = x_1[(uint32_t)4U * i];
         uint64_t t210 = p11[(uint32_t)4U * i];
@@ -8643,14 +9457,13 @@ Hacl_P256_ecdsa_verif_p256_sha384(
       uint64_t t3[(uint32_t)2U * len65];
       memset(t3, 0U, (uint32_t)2U * len65 * sizeof (uint64_t));
       uint32_t len74 = (uint32_t)4U;
-      uint32_t resLen2 = len74 + len74;
-      memset(t3, 0U, resLen2 * sizeof (uint64_t));
+      memset(t3, 0U, (len74 + len74) * sizeof (uint64_t));
       for (uint32_t i0 = (uint32_t)0U; i0 < len74; i0++)
       {
         uint64_t bj = z1[i0];
         uint64_t *res_j = t3 + i0;
         uint64_t c = (uint64_t)0U;
-        for (uint32_t i = (uint32_t)0U; i < len74 / (uint32_t)4U * (uint32_t)4U / (uint32_t)4U; i++)
+        for (uint32_t i = (uint32_t)0U; i < len74 / (uint32_t)4U; i++)
         {
           uint64_t a_i = sq_z1[(uint32_t)4U * i];
           uint64_t *res_i0 = res_j + (uint32_t)4U * i;
@@ -8712,7 +9525,7 @@ Hacl_P256_ecdsa_verif_p256_sha384(
         mul64(f3, t10, o3, o4);
         uint32_t len94 = (uint32_t)4U * (uint32_t)2U;
         uint64_t c = (uint64_t)0U;
-        for (uint32_t i = (uint32_t)0U; i < len94 / (uint32_t)4U * (uint32_t)4U / (uint32_t)4U; i++)
+        for (uint32_t i = (uint32_t)0U; i < len94 / (uint32_t)4U; i++)
         {
           uint64_t t1 = t3[(uint32_t)4U * i];
           uint64_t t210 = t23[(uint32_t)4U * i];
@@ -8765,7 +9578,7 @@ Hacl_P256_ecdsa_verif_p256_sha384(
         };
       uint32_t len102 = (uint32_t)4U;
       uint64_t c5 = (uint64_t)0U;
-      for (uint32_t i = (uint32_t)0U; i < len102 / (uint32_t)4U * (uint32_t)4U / (uint32_t)4U; i++)
+      for (uint32_t i = (uint32_t)0U; i < len102 / (uint32_t)4U; i++)
       {
         uint64_t t1 = x_2[(uint32_t)4U * i];
         uint64_t t210 = p12[(uint32_t)4U * i];
@@ -8805,14 +9618,13 @@ Hacl_P256_ecdsa_verif_p256_sha384(
       uint64_t t4[(uint32_t)2U * len66];
       memset(t4, 0U, (uint32_t)2U * len66 * sizeof (uint64_t));
       uint32_t len76 = (uint32_t)4U;
-      uint32_t resLen3 = len76 + len76;
-      memset(t4, 0U, resLen3 * sizeof (uint64_t));
+      memset(t4, 0U, (len76 + len76) * sizeof (uint64_t));
       for (uint32_t i0 = (uint32_t)0U; i0 < len76; i0++)
       {
         uint64_t bj = z2[i0];
         uint64_t *res_j = t4 + i0;
         uint64_t c = (uint64_t)0U;
-        for (uint32_t i = (uint32_t)0U; i < len76 / (uint32_t)4U * (uint32_t)4U / (uint32_t)4U; i++)
+        for (uint32_t i = (uint32_t)0U; i < len76 / (uint32_t)4U; i++)
         {
           uint64_t a_i = sq_z2[(uint32_t)4U * i];
           uint64_t *res_i0 = res_j + (uint32_t)4U * i;
@@ -8874,7 +9686,7 @@ Hacl_P256_ecdsa_verif_p256_sha384(
         mul64(f3, t10, o3, o4);
         uint32_t len95 = (uint32_t)4U * (uint32_t)2U;
         uint64_t c = (uint64_t)0U;
-        for (uint32_t i = (uint32_t)0U; i < len95 / (uint32_t)4U * (uint32_t)4U / (uint32_t)4U; i++)
+        for (uint32_t i = (uint32_t)0U; i < len95 / (uint32_t)4U; i++)
         {
           uint64_t t1 = t4[(uint32_t)4U * i];
           uint64_t t210 = t24[(uint32_t)4U * i];
@@ -8927,7 +9739,7 @@ Hacl_P256_ecdsa_verif_p256_sha384(
         };
       uint32_t len103 = (uint32_t)4U;
       uint64_t c6 = (uint64_t)0U;
-      for (uint32_t i = (uint32_t)0U; i < len103 / (uint32_t)4U * (uint32_t)4U / (uint32_t)4U; i++)
+      for (uint32_t i = (uint32_t)0U; i < len103 / (uint32_t)4U; i++)
       {
         uint64_t t1 = x_3[(uint32_t)4U * i];
         uint64_t t210 = p13[(uint32_t)4U * i];
@@ -8967,14 +9779,13 @@ Hacl_P256_ecdsa_verif_p256_sha384(
       uint64_t t5[(uint32_t)2U * len67];
       memset(t5, 0U, (uint32_t)2U * len67 * sizeof (uint64_t));
       uint32_t len78 = (uint32_t)4U;
-      uint32_t resLen4 = len78 + len78;
-      memset(t5, 0U, resLen4 * sizeof (uint64_t));
+      memset(t5, 0U, (len78 + len78) * sizeof (uint64_t));
       for (uint32_t i0 = (uint32_t)0U; i0 < len78; i0++)
       {
         uint64_t bj = x2[i0];
         uint64_t *res_j = t5 + i0;
         uint64_t c = (uint64_t)0U;
-        for (uint32_t i = (uint32_t)0U; i < len78 / (uint32_t)4U * (uint32_t)4U / (uint32_t)4U; i++)
+        for (uint32_t i = (uint32_t)0U; i < len78 / (uint32_t)4U; i++)
         {
           uint64_t a_i = sq_z1[(uint32_t)4U * i];
           uint64_t *res_i0 = res_j + (uint32_t)4U * i;
@@ -9036,7 +9847,7 @@ Hacl_P256_ecdsa_verif_p256_sha384(
         mul64(f3, t10, o3, o4);
         uint32_t len96 = (uint32_t)4U * (uint32_t)2U;
         uint64_t c = (uint64_t)0U;
-        for (uint32_t i = (uint32_t)0U; i < len96 / (uint32_t)4U * (uint32_t)4U / (uint32_t)4U; i++)
+        for (uint32_t i = (uint32_t)0U; i < len96 / (uint32_t)4U; i++)
         {
           uint64_t t1 = t5[(uint32_t)4U * i];
           uint64_t t210 = t25[(uint32_t)4U * i];
@@ -9089,7 +9900,7 @@ Hacl_P256_ecdsa_verif_p256_sha384(
         };
       uint32_t len104 = (uint32_t)4U;
       uint64_t c7 = (uint64_t)0U;
-      for (uint32_t i = (uint32_t)0U; i < len104 / (uint32_t)4U * (uint32_t)4U / (uint32_t)4U; i++)
+      for (uint32_t i = (uint32_t)0U; i < len104 / (uint32_t)4U; i++)
       {
         uint64_t t1 = x_4[(uint32_t)4U * i];
         uint64_t t210 = p14[(uint32_t)4U * i];
@@ -9129,19 +9940,13 @@ Hacl_P256_ecdsa_verif_p256_sha384(
       uint64_t t6[(uint32_t)2U * len68];
       memset(t6, 0U, (uint32_t)2U * len68 * sizeof (uint64_t));
       uint32_t len710 = (uint32_t)4U;
-      uint32_t resLen5 = len710 + len710;
-      memset(t6, 0U, resLen5 * sizeof (uint64_t));
+      memset(t6, 0U, (len710 + len710) * sizeof (uint64_t));
       for (uint32_t i0 = (uint32_t)0U; i0 < len710; i0++)
       {
         uint64_t bj = x1[i0];
         uint64_t *res_j = t6 + i0;
         uint64_t c = (uint64_t)0U;
-        for
-        (uint32_t
-          i = (uint32_t)0U;
-          i
-          < len710 / (uint32_t)4U * (uint32_t)4U / (uint32_t)4U;
-          i++)
+        for (uint32_t i = (uint32_t)0U; i < len710 / (uint32_t)4U; i++)
         {
           uint64_t a_i = sq_z2[(uint32_t)4U * i];
           uint64_t *res_i0 = res_j + (uint32_t)4U * i;
@@ -9203,7 +10008,7 @@ Hacl_P256_ecdsa_verif_p256_sha384(
         mul64(f3, t10, o3, o4);
         uint32_t len97 = (uint32_t)4U * (uint32_t)2U;
         uint64_t c = (uint64_t)0U;
-        for (uint32_t i = (uint32_t)0U; i < len97 / (uint32_t)4U * (uint32_t)4U / (uint32_t)4U; i++)
+        for (uint32_t i = (uint32_t)0U; i < len97 / (uint32_t)4U; i++)
         {
           uint64_t t1 = t6[(uint32_t)4U * i];
           uint64_t t210 = t26[(uint32_t)4U * i];
@@ -9256,7 +10061,7 @@ Hacl_P256_ecdsa_verif_p256_sha384(
         };
       uint32_t len105 = (uint32_t)4U;
       uint64_t c8 = (uint64_t)0U;
-      for (uint32_t i = (uint32_t)0U; i < len105 / (uint32_t)4U * (uint32_t)4U / (uint32_t)4U; i++)
+      for (uint32_t i = (uint32_t)0U; i < len105 / (uint32_t)4U; i++)
       {
         uint64_t t1 = x_5[(uint32_t)4U * i];
         uint64_t t210 = p15[(uint32_t)4U * i];
@@ -9296,19 +10101,13 @@ Hacl_P256_ecdsa_verif_p256_sha384(
       uint64_t t7[(uint32_t)2U * len69];
       memset(t7, 0U, (uint32_t)2U * len69 * sizeof (uint64_t));
       uint32_t len712 = (uint32_t)4U;
-      uint32_t resLen6 = len712 + len712;
-      memset(t7, 0U, resLen6 * sizeof (uint64_t));
+      memset(t7, 0U, (len712 + len712) * sizeof (uint64_t));
       for (uint32_t i0 = (uint32_t)0U; i0 < len712; i0++)
       {
         uint64_t bj = y2[i0];
         uint64_t *res_j = t7 + i0;
         uint64_t c = (uint64_t)0U;
-        for
-        (uint32_t
-          i = (uint32_t)0U;
-          i
-          < len712 / (uint32_t)4U * (uint32_t)4U / (uint32_t)4U;
-          i++)
+        for (uint32_t i = (uint32_t)0U; i < len712 / (uint32_t)4U; i++)
         {
           uint64_t a_i = tr_z1[(uint32_t)4U * i];
           uint64_t *res_i0 = res_j + (uint32_t)4U * i;
@@ -9370,7 +10169,7 @@ Hacl_P256_ecdsa_verif_p256_sha384(
         mul64(f3, t10, o3, o4);
         uint32_t len98 = (uint32_t)4U * (uint32_t)2U;
         uint64_t c = (uint64_t)0U;
-        for (uint32_t i = (uint32_t)0U; i < len98 / (uint32_t)4U * (uint32_t)4U / (uint32_t)4U; i++)
+        for (uint32_t i = (uint32_t)0U; i < len98 / (uint32_t)4U; i++)
         {
           uint64_t t1 = t7[(uint32_t)4U * i];
           uint64_t t210 = t27[(uint32_t)4U * i];
@@ -9423,7 +10222,7 @@ Hacl_P256_ecdsa_verif_p256_sha384(
         };
       uint32_t len106 = (uint32_t)4U;
       uint64_t c9 = (uint64_t)0U;
-      for (uint32_t i = (uint32_t)0U; i < len106 / (uint32_t)4U * (uint32_t)4U / (uint32_t)4U; i++)
+      for (uint32_t i = (uint32_t)0U; i < len106 / (uint32_t)4U; i++)
       {
         uint64_t t1 = x_6[(uint32_t)4U * i];
         uint64_t t210 = p16[(uint32_t)4U * i];
@@ -9463,14 +10262,13 @@ Hacl_P256_ecdsa_verif_p256_sha384(
       uint64_t t8[(uint32_t)2U * len610];
       memset(t8, 0U, (uint32_t)2U * len610 * sizeof (uint64_t));
       uint32_t len7 = (uint32_t)4U;
-      uint32_t resLen = len7 + len7;
-      memset(t8, 0U, resLen * sizeof (uint64_t));
+      memset(t8, 0U, (len7 + len7) * sizeof (uint64_t));
       for (uint32_t i0 = (uint32_t)0U; i0 < len7; i0++)
       {
         uint64_t bj = y1[i0];
         uint64_t *res_j = t8 + i0;
         uint64_t c = (uint64_t)0U;
-        for (uint32_t i = (uint32_t)0U; i < len7 / (uint32_t)4U * (uint32_t)4U / (uint32_t)4U; i++)
+        for (uint32_t i = (uint32_t)0U; i < len7 / (uint32_t)4U; i++)
         {
           uint64_t a_i = tr_z2[(uint32_t)4U * i];
           uint64_t *res_i0 = res_j + (uint32_t)4U * i;
@@ -9532,7 +10330,7 @@ Hacl_P256_ecdsa_verif_p256_sha384(
         mul64(f3, t10, o3, o4);
         uint32_t len99 = (uint32_t)4U * (uint32_t)2U;
         uint64_t c = (uint64_t)0U;
-        for (uint32_t i = (uint32_t)0U; i < len99 / (uint32_t)4U * (uint32_t)4U / (uint32_t)4U; i++)
+        for (uint32_t i = (uint32_t)0U; i < len99 / (uint32_t)4U; i++)
         {
           uint64_t t1 = t8[(uint32_t)4U * i];
           uint64_t t210 = t2[(uint32_t)4U * i];
@@ -9585,7 +10383,7 @@ Hacl_P256_ecdsa_verif_p256_sha384(
         };
       uint32_t len10 = (uint32_t)4U;
       uint64_t c = (uint64_t)0U;
-      for (uint32_t i = (uint32_t)0U; i < len10 / (uint32_t)4U * (uint32_t)4U / (uint32_t)4U; i++)
+      for (uint32_t i = (uint32_t)0U; i < len10 / (uint32_t)4U; i++)
       {
         uint64_t t1 = x_[(uint32_t)4U * i];
         uint64_t t210 = p1[(uint32_t)4U * i];
@@ -9789,7 +10587,7 @@ Hacl_P256_ecdsa_verif_p256_sha512(
       };
     uint32_t len31 = (uint32_t)4U;
     uint64_t c1 = (uint64_t)0U;
-    for (uint32_t i = (uint32_t)0U; i < len31 / (uint32_t)4U * (uint32_t)4U / (uint32_t)4U; i++)
+    for (uint32_t i = (uint32_t)0U; i < len31 / (uint32_t)4U; i++)
     {
       uint64_t t1 = rAsFelem[(uint32_t)4U * i];
       uint64_t t20 = p0[(uint32_t)4U * i];
@@ -9844,7 +10642,7 @@ Hacl_P256_ecdsa_verif_p256_sha512(
       };
     uint32_t len33 = (uint32_t)4U;
     uint64_t c2 = (uint64_t)0U;
-    for (uint32_t i = (uint32_t)0U; i < len33 / (uint32_t)4U * (uint32_t)4U / (uint32_t)4U; i++)
+    for (uint32_t i = (uint32_t)0U; i < len33 / (uint32_t)4U; i++)
     {
       uint64_t t1 = sAsFelem[(uint32_t)4U * i];
       uint64_t t20 = p2[(uint32_t)4U * i];
@@ -10042,15 +10840,14 @@ Hacl_P256_ecdsa_verif_p256_sha512(
       uint64_t t[(uint32_t)2U * len6];
       memset(t, 0U, (uint32_t)2U * len6 * sizeof (uint64_t));
       uint32_t len70 = (uint32_t)4U;
-      uint32_t resLen0 = len70 + len70;
-      memset(t, 0U, resLen0 * sizeof (uint64_t));
+      memset(t, 0U, (len70 + len70) * sizeof (uint64_t));
       for (uint32_t i0 = (uint32_t)0U; i0 < len70; i0++)
       {
         uint64_t *ab = z1;
         uint64_t a_j = z1[i0];
         uint64_t *res_j = t + i0;
         uint64_t c = (uint64_t)0U;
-        for (uint32_t i = (uint32_t)0U; i < i0 / (uint32_t)4U * (uint32_t)4U / (uint32_t)4U; i++)
+        for (uint32_t i = (uint32_t)0U; i < i0 / (uint32_t)4U; i++)
         {
           uint64_t a_i = ab[(uint32_t)4U * i];
           uint64_t *res_i0 = res_j + (uint32_t)4U * i;
@@ -10074,10 +10871,10 @@ Hacl_P256_ecdsa_verif_p256_sha512(
         uint64_t r12 = c;
         t[i0 + i0] = r12;
       }
-      uint64_t c00 = bn_add_eq_len_u64(resLen0, t, t, t);
-      KRML_CHECK_SIZE(sizeof (uint64_t), resLen0);
-      uint64_t tmp3[resLen0];
-      memset(tmp3, 0U, resLen0 * sizeof (uint64_t));
+      uint64_t c00 = bn_add_eq_len_u64(len70 + len70, t, t, t);
+      KRML_CHECK_SIZE(sizeof (uint64_t), len70 + len70);
+      uint64_t tmp3[len70 + len70];
+      memset(tmp3, 0U, (len70 + len70) * sizeof (uint64_t));
       for (uint32_t i = (uint32_t)0U; i < len70; i++)
       {
         uint128_t res = (uint128_t)z1[i] * z1[i];
@@ -10086,7 +10883,7 @@ Hacl_P256_ecdsa_verif_p256_sha512(
         tmp3[(uint32_t)2U * i] = lo;
         tmp3[(uint32_t)2U * i + (uint32_t)1U] = hi;
       }
-      uint64_t c10 = bn_add_eq_len_u64(resLen0, t, tmp3, t);
+      uint64_t c10 = bn_add_eq_len_u64(len70 + len70, t, tmp3, t);
       uint32_t len71 = (uint32_t)4U;
       KRML_CHECK_SIZE(sizeof (uint64_t), (uint32_t)2U * len71);
       uint64_t t20[(uint32_t)2U * len71];
@@ -10125,7 +10922,7 @@ Hacl_P256_ecdsa_verif_p256_sha512(
         mul64(f3, t10, o3, o4);
         uint32_t len92 = (uint32_t)4U * (uint32_t)2U;
         uint64_t c = (uint64_t)0U;
-        for (uint32_t i = (uint32_t)0U; i < len92 / (uint32_t)4U * (uint32_t)4U / (uint32_t)4U; i++)
+        for (uint32_t i = (uint32_t)0U; i < len92 / (uint32_t)4U; i++)
         {
           uint64_t t1 = t[(uint32_t)4U * i];
           uint64_t t210 = t20[(uint32_t)4U * i];
@@ -10178,7 +10975,7 @@ Hacl_P256_ecdsa_verif_p256_sha512(
         };
       uint32_t len100 = (uint32_t)4U;
       uint64_t c3 = (uint64_t)0U;
-      for (uint32_t i = (uint32_t)0U; i < len100 / (uint32_t)4U * (uint32_t)4U / (uint32_t)4U; i++)
+      for (uint32_t i = (uint32_t)0U; i < len100 / (uint32_t)4U; i++)
       {
         uint64_t t1 = x_0[(uint32_t)4U * i];
         uint64_t t210 = p10[(uint32_t)4U * i];
@@ -10218,15 +11015,14 @@ Hacl_P256_ecdsa_verif_p256_sha512(
       uint64_t t0[(uint32_t)2U * len64];
       memset(t0, 0U, (uint32_t)2U * len64 * sizeof (uint64_t));
       uint32_t len72 = (uint32_t)4U;
-      uint32_t resLen1 = len72 + len72;
-      memset(t0, 0U, resLen1 * sizeof (uint64_t));
+      memset(t0, 0U, (len72 + len72) * sizeof (uint64_t));
       for (uint32_t i0 = (uint32_t)0U; i0 < len72; i0++)
       {
         uint64_t *ab = z2;
         uint64_t a_j = z2[i0];
         uint64_t *res_j = t0 + i0;
         uint64_t c = (uint64_t)0U;
-        for (uint32_t i = (uint32_t)0U; i < i0 / (uint32_t)4U * (uint32_t)4U / (uint32_t)4U; i++)
+        for (uint32_t i = (uint32_t)0U; i < i0 / (uint32_t)4U; i++)
         {
           uint64_t a_i = ab[(uint32_t)4U * i];
           uint64_t *res_i0 = res_j + (uint32_t)4U * i;
@@ -10250,10 +11046,10 @@ Hacl_P256_ecdsa_verif_p256_sha512(
         uint64_t r13 = c;
         t0[i0 + i0] = r13;
       }
-      uint64_t c0 = bn_add_eq_len_u64(resLen1, t0, t0, t0);
-      KRML_CHECK_SIZE(sizeof (uint64_t), resLen1);
-      uint64_t tmp4[resLen1];
-      memset(tmp4, 0U, resLen1 * sizeof (uint64_t));
+      uint64_t c0 = bn_add_eq_len_u64(len72 + len72, t0, t0, t0);
+      KRML_CHECK_SIZE(sizeof (uint64_t), len72 + len72);
+      uint64_t tmp4[len72 + len72];
+      memset(tmp4, 0U, (len72 + len72) * sizeof (uint64_t));
       for (uint32_t i = (uint32_t)0U; i < len72; i++)
       {
         uint128_t res = (uint128_t)z2[i] * z2[i];
@@ -10262,7 +11058,7 @@ Hacl_P256_ecdsa_verif_p256_sha512(
         tmp4[(uint32_t)2U * i] = lo;
         tmp4[(uint32_t)2U * i + (uint32_t)1U] = hi;
       }
-      uint64_t c11 = bn_add_eq_len_u64(resLen1, t0, tmp4, t0);
+      uint64_t c11 = bn_add_eq_len_u64(len72 + len72, t0, tmp4, t0);
       uint32_t len73 = (uint32_t)4U;
       KRML_CHECK_SIZE(sizeof (uint64_t), (uint32_t)2U * len73);
       uint64_t t22[(uint32_t)2U * len73];
@@ -10301,7 +11097,7 @@ Hacl_P256_ecdsa_verif_p256_sha512(
         mul64(f3, t10, o3, o4);
         uint32_t len93 = (uint32_t)4U * (uint32_t)2U;
         uint64_t c = (uint64_t)0U;
-        for (uint32_t i = (uint32_t)0U; i < len93 / (uint32_t)4U * (uint32_t)4U / (uint32_t)4U; i++)
+        for (uint32_t i = (uint32_t)0U; i < len93 / (uint32_t)4U; i++)
         {
           uint64_t t1 = t0[(uint32_t)4U * i];
           uint64_t t210 = t22[(uint32_t)4U * i];
@@ -10354,7 +11150,7 @@ Hacl_P256_ecdsa_verif_p256_sha512(
         };
       uint32_t len101 = (uint32_t)4U;
       uint64_t c4 = (uint64_t)0U;
-      for (uint32_t i = (uint32_t)0U; i < len101 / (uint32_t)4U * (uint32_t)4U / (uint32_t)4U; i++)
+      for (uint32_t i = (uint32_t)0U; i < len101 / (uint32_t)4U; i++)
       {
         uint64_t t1 = x_1[(uint32_t)4U * i];
         uint64_t t210 = p11[(uint32_t)4U * i];
@@ -10394,14 +11190,13 @@ Hacl_P256_ecdsa_verif_p256_sha512(
       uint64_t t3[(uint32_t)2U * len65];
       memset(t3, 0U, (uint32_t)2U * len65 * sizeof (uint64_t));
       uint32_t len74 = (uint32_t)4U;
-      uint32_t resLen2 = len74 + len74;
-      memset(t3, 0U, resLen2 * sizeof (uint64_t));
+      memset(t3, 0U, (len74 + len74) * sizeof (uint64_t));
       for (uint32_t i0 = (uint32_t)0U; i0 < len74; i0++)
       {
         uint64_t bj = z1[i0];
         uint64_t *res_j = t3 + i0;
         uint64_t c = (uint64_t)0U;
-        for (uint32_t i = (uint32_t)0U; i < len74 / (uint32_t)4U * (uint32_t)4U / (uint32_t)4U; i++)
+        for (uint32_t i = (uint32_t)0U; i < len74 / (uint32_t)4U; i++)
         {
           uint64_t a_i = sq_z1[(uint32_t)4U * i];
           uint64_t *res_i0 = res_j + (uint32_t)4U * i;
@@ -10463,7 +11258,7 @@ Hacl_P256_ecdsa_verif_p256_sha512(
         mul64(f3, t10, o3, o4);
         uint32_t len94 = (uint32_t)4U * (uint32_t)2U;
         uint64_t c = (uint64_t)0U;
-        for (uint32_t i = (uint32_t)0U; i < len94 / (uint32_t)4U * (uint32_t)4U / (uint32_t)4U; i++)
+        for (uint32_t i = (uint32_t)0U; i < len94 / (uint32_t)4U; i++)
         {
           uint64_t t1 = t3[(uint32_t)4U * i];
           uint64_t t210 = t23[(uint32_t)4U * i];
@@ -10516,7 +11311,7 @@ Hacl_P256_ecdsa_verif_p256_sha512(
         };
       uint32_t len102 = (uint32_t)4U;
       uint64_t c5 = (uint64_t)0U;
-      for (uint32_t i = (uint32_t)0U; i < len102 / (uint32_t)4U * (uint32_t)4U / (uint32_t)4U; i++)
+      for (uint32_t i = (uint32_t)0U; i < len102 / (uint32_t)4U; i++)
       {
         uint64_t t1 = x_2[(uint32_t)4U * i];
         uint64_t t210 = p12[(uint32_t)4U * i];
@@ -10556,14 +11351,13 @@ Hacl_P256_ecdsa_verif_p256_sha512(
       uint64_t t4[(uint32_t)2U * len66];
       memset(t4, 0U, (uint32_t)2U * len66 * sizeof (uint64_t));
       uint32_t len76 = (uint32_t)4U;
-      uint32_t resLen3 = len76 + len76;
-      memset(t4, 0U, resLen3 * sizeof (uint64_t));
+      memset(t4, 0U, (len76 + len76) * sizeof (uint64_t));
       for (uint32_t i0 = (uint32_t)0U; i0 < len76; i0++)
       {
         uint64_t bj = z2[i0];
         uint64_t *res_j = t4 + i0;
         uint64_t c = (uint64_t)0U;
-        for (uint32_t i = (uint32_t)0U; i < len76 / (uint32_t)4U * (uint32_t)4U / (uint32_t)4U; i++)
+        for (uint32_t i = (uint32_t)0U; i < len76 / (uint32_t)4U; i++)
         {
           uint64_t a_i = sq_z2[(uint32_t)4U * i];
           uint64_t *res_i0 = res_j + (uint32_t)4U * i;
@@ -10625,7 +11419,7 @@ Hacl_P256_ecdsa_verif_p256_sha512(
         mul64(f3, t10, o3, o4);
         uint32_t len95 = (uint32_t)4U * (uint32_t)2U;
         uint64_t c = (uint64_t)0U;
-        for (uint32_t i = (uint32_t)0U; i < len95 / (uint32_t)4U * (uint32_t)4U / (uint32_t)4U; i++)
+        for (uint32_t i = (uint32_t)0U; i < len95 / (uint32_t)4U; i++)
         {
           uint64_t t1 = t4[(uint32_t)4U * i];
           uint64_t t210 = t24[(uint32_t)4U * i];
@@ -10678,7 +11472,7 @@ Hacl_P256_ecdsa_verif_p256_sha512(
         };
       uint32_t len103 = (uint32_t)4U;
       uint64_t c6 = (uint64_t)0U;
-      for (uint32_t i = (uint32_t)0U; i < len103 / (uint32_t)4U * (uint32_t)4U / (uint32_t)4U; i++)
+      for (uint32_t i = (uint32_t)0U; i < len103 / (uint32_t)4U; i++)
       {
         uint64_t t1 = x_3[(uint32_t)4U * i];
         uint64_t t210 = p13[(uint32_t)4U * i];
@@ -10718,14 +11512,13 @@ Hacl_P256_ecdsa_verif_p256_sha512(
       uint64_t t5[(uint32_t)2U * len67];
       memset(t5, 0U, (uint32_t)2U * len67 * sizeof (uint64_t));
       uint32_t len78 = (uint32_t)4U;
-      uint32_t resLen4 = len78 + len78;
-      memset(t5, 0U, resLen4 * sizeof (uint64_t));
+      memset(t5, 0U, (len78 + len78) * sizeof (uint64_t));
       for (uint32_t i0 = (uint32_t)0U; i0 < len78; i0++)
       {
         uint64_t bj = x2[i0];
         uint64_t *res_j = t5 + i0;
         uint64_t c = (uint64_t)0U;
-        for (uint32_t i = (uint32_t)0U; i < len78 / (uint32_t)4U * (uint32_t)4U / (uint32_t)4U; i++)
+        for (uint32_t i = (uint32_t)0U; i < len78 / (uint32_t)4U; i++)
         {
           uint64_t a_i = sq_z1[(uint32_t)4U * i];
           uint64_t *res_i0 = res_j + (uint32_t)4U * i;
@@ -10787,7 +11580,7 @@ Hacl_P256_ecdsa_verif_p256_sha512(
         mul64(f3, t10, o3, o4);
         uint32_t len96 = (uint32_t)4U * (uint32_t)2U;
         uint64_t c = (uint64_t)0U;
-        for (uint32_t i = (uint32_t)0U; i < len96 / (uint32_t)4U * (uint32_t)4U / (uint32_t)4U; i++)
+        for (uint32_t i = (uint32_t)0U; i < len96 / (uint32_t)4U; i++)
         {
           uint64_t t1 = t5[(uint32_t)4U * i];
           uint64_t t210 = t25[(uint32_t)4U * i];
@@ -10840,7 +11633,7 @@ Hacl_P256_ecdsa_verif_p256_sha512(
         };
       uint32_t len104 = (uint32_t)4U;
       uint64_t c7 = (uint64_t)0U;
-      for (uint32_t i = (uint32_t)0U; i < len104 / (uint32_t)4U * (uint32_t)4U / (uint32_t)4U; i++)
+      for (uint32_t i = (uint32_t)0U; i < len104 / (uint32_t)4U; i++)
       {
         uint64_t t1 = x_4[(uint32_t)4U * i];
         uint64_t t210 = p14[(uint32_t)4U * i];
@@ -10880,19 +11673,13 @@ Hacl_P256_ecdsa_verif_p256_sha512(
       uint64_t t6[(uint32_t)2U * len68];
       memset(t6, 0U, (uint32_t)2U * len68 * sizeof (uint64_t));
       uint32_t len710 = (uint32_t)4U;
-      uint32_t resLen5 = len710 + len710;
-      memset(t6, 0U, resLen5 * sizeof (uint64_t));
+      memset(t6, 0U, (len710 + len710) * sizeof (uint64_t));
       for (uint32_t i0 = (uint32_t)0U; i0 < len710; i0++)
       {
         uint64_t bj = x1[i0];
         uint64_t *res_j = t6 + i0;
         uint64_t c = (uint64_t)0U;
-        for
-        (uint32_t
-          i = (uint32_t)0U;
-          i
-          < len710 / (uint32_t)4U * (uint32_t)4U / (uint32_t)4U;
-          i++)
+        for (uint32_t i = (uint32_t)0U; i < len710 / (uint32_t)4U; i++)
         {
           uint64_t a_i = sq_z2[(uint32_t)4U * i];
           uint64_t *res_i0 = res_j + (uint32_t)4U * i;
@@ -10954,7 +11741,7 @@ Hacl_P256_ecdsa_verif_p256_sha512(
         mul64(f3, t10, o3, o4);
         uint32_t len97 = (uint32_t)4U * (uint32_t)2U;
         uint64_t c = (uint64_t)0U;
-        for (uint32_t i = (uint32_t)0U; i < len97 / (uint32_t)4U * (uint32_t)4U / (uint32_t)4U; i++)
+        for (uint32_t i = (uint32_t)0U; i < len97 / (uint32_t)4U; i++)
         {
           uint64_t t1 = t6[(uint32_t)4U * i];
           uint64_t t210 = t26[(uint32_t)4U * i];
@@ -11007,7 +11794,7 @@ Hacl_P256_ecdsa_verif_p256_sha512(
         };
       uint32_t len105 = (uint32_t)4U;
       uint64_t c8 = (uint64_t)0U;
-      for (uint32_t i = (uint32_t)0U; i < len105 / (uint32_t)4U * (uint32_t)4U / (uint32_t)4U; i++)
+      for (uint32_t i = (uint32_t)0U; i < len105 / (uint32_t)4U; i++)
       {
         uint64_t t1 = x_5[(uint32_t)4U * i];
         uint64_t t210 = p15[(uint32_t)4U * i];
@@ -11047,19 +11834,13 @@ Hacl_P256_ecdsa_verif_p256_sha512(
       uint64_t t7[(uint32_t)2U * len69];
       memset(t7, 0U, (uint32_t)2U * len69 * sizeof (uint64_t));
       uint32_t len712 = (uint32_t)4U;
-      uint32_t resLen6 = len712 + len712;
-      memset(t7, 0U, resLen6 * sizeof (uint64_t));
+      memset(t7, 0U, (len712 + len712) * sizeof (uint64_t));
       for (uint32_t i0 = (uint32_t)0U; i0 < len712; i0++)
       {
         uint64_t bj = y2[i0];
         uint64_t *res_j = t7 + i0;
         uint64_t c = (uint64_t)0U;
-        for
-        (uint32_t
-          i = (uint32_t)0U;
-          i
-          < len712 / (uint32_t)4U * (uint32_t)4U / (uint32_t)4U;
-          i++)
+        for (uint32_t i = (uint32_t)0U; i < len712 / (uint32_t)4U; i++)
         {
           uint64_t a_i = tr_z1[(uint32_t)4U * i];
           uint64_t *res_i0 = res_j + (uint32_t)4U * i;
@@ -11121,7 +11902,7 @@ Hacl_P256_ecdsa_verif_p256_sha512(
         mul64(f3, t10, o3, o4);
         uint32_t len98 = (uint32_t)4U * (uint32_t)2U;
         uint64_t c = (uint64_t)0U;
-        for (uint32_t i = (uint32_t)0U; i < len98 / (uint32_t)4U * (uint32_t)4U / (uint32_t)4U; i++)
+        for (uint32_t i = (uint32_t)0U; i < len98 / (uint32_t)4U; i++)
         {
           uint64_t t1 = t7[(uint32_t)4U * i];
           uint64_t t210 = t27[(uint32_t)4U * i];
@@ -11174,7 +11955,7 @@ Hacl_P256_ecdsa_verif_p256_sha512(
         };
       uint32_t len106 = (uint32_t)4U;
       uint64_t c9 = (uint64_t)0U;
-      for (uint32_t i = (uint32_t)0U; i < len106 / (uint32_t)4U * (uint32_t)4U / (uint32_t)4U; i++)
+      for (uint32_t i = (uint32_t)0U; i < len106 / (uint32_t)4U; i++)
       {
         uint64_t t1 = x_6[(uint32_t)4U * i];
         uint64_t t210 = p16[(uint32_t)4U * i];
@@ -11214,14 +11995,13 @@ Hacl_P256_ecdsa_verif_p256_sha512(
       uint64_t t8[(uint32_t)2U * len610];
       memset(t8, 0U, (uint32_t)2U * len610 * sizeof (uint64_t));
       uint32_t len7 = (uint32_t)4U;
-      uint32_t resLen = len7 + len7;
-      memset(t8, 0U, resLen * sizeof (uint64_t));
+      memset(t8, 0U, (len7 + len7) * sizeof (uint64_t));
       for (uint32_t i0 = (uint32_t)0U; i0 < len7; i0++)
       {
         uint64_t bj = y1[i0];
         uint64_t *res_j = t8 + i0;
         uint64_t c = (uint64_t)0U;
-        for (uint32_t i = (uint32_t)0U; i < len7 / (uint32_t)4U * (uint32_t)4U / (uint32_t)4U; i++)
+        for (uint32_t i = (uint32_t)0U; i < len7 / (uint32_t)4U; i++)
         {
           uint64_t a_i = tr_z2[(uint32_t)4U * i];
           uint64_t *res_i0 = res_j + (uint32_t)4U * i;
@@ -11283,7 +12063,7 @@ Hacl_P256_ecdsa_verif_p256_sha512(
         mul64(f3, t10, o3, o4);
         uint32_t len99 = (uint32_t)4U * (uint32_t)2U;
         uint64_t c = (uint64_t)0U;
-        for (uint32_t i = (uint32_t)0U; i < len99 / (uint32_t)4U * (uint32_t)4U / (uint32_t)4U; i++)
+        for (uint32_t i = (uint32_t)0U; i < len99 / (uint32_t)4U; i++)
         {
           uint64_t t1 = t8[(uint32_t)4U * i];
           uint64_t t210 = t2[(uint32_t)4U * i];
@@ -11336,7 +12116,7 @@ Hacl_P256_ecdsa_verif_p256_sha512(
         };
       uint32_t len10 = (uint32_t)4U;
       uint64_t c = (uint64_t)0U;
-      for (uint32_t i = (uint32_t)0U; i < len10 / (uint32_t)4U * (uint32_t)4U / (uint32_t)4U; i++)
+      for (uint32_t i = (uint32_t)0U; i < len10 / (uint32_t)4U; i++)
       {
         uint64_t t1 = x_[(uint32_t)4U * i];
         uint64_t t210 = p1[(uint32_t)4U * i];
@@ -11542,7 +12322,7 @@ Hacl_P256_ecdsa_verif_without_hash(
       };
     uint32_t len31 = (uint32_t)4U;
     uint64_t c1 = (uint64_t)0U;
-    for (uint32_t i = (uint32_t)0U; i < len31 / (uint32_t)4U * (uint32_t)4U / (uint32_t)4U; i++)
+    for (uint32_t i = (uint32_t)0U; i < len31 / (uint32_t)4U; i++)
     {
       uint64_t t1 = rAsFelem[(uint32_t)4U * i];
       uint64_t t20 = p0[(uint32_t)4U * i];
@@ -11597,7 +12377,7 @@ Hacl_P256_ecdsa_verif_without_hash(
       };
     uint32_t len33 = (uint32_t)4U;
     uint64_t c2 = (uint64_t)0U;
-    for (uint32_t i = (uint32_t)0U; i < len33 / (uint32_t)4U * (uint32_t)4U / (uint32_t)4U; i++)
+    for (uint32_t i = (uint32_t)0U; i < len33 / (uint32_t)4U; i++)
     {
       uint64_t t1 = sAsFelem[(uint32_t)4U * i];
       uint64_t t20 = p2[(uint32_t)4U * i];
@@ -11795,15 +12575,14 @@ Hacl_P256_ecdsa_verif_without_hash(
       uint64_t t[(uint32_t)2U * len6];
       memset(t, 0U, (uint32_t)2U * len6 * sizeof (uint64_t));
       uint32_t len70 = (uint32_t)4U;
-      uint32_t resLen0 = len70 + len70;
-      memset(t, 0U, resLen0 * sizeof (uint64_t));
+      memset(t, 0U, (len70 + len70) * sizeof (uint64_t));
       for (uint32_t i0 = (uint32_t)0U; i0 < len70; i0++)
       {
         uint64_t *ab = z1;
         uint64_t a_j = z1[i0];
         uint64_t *res_j = t + i0;
         uint64_t c = (uint64_t)0U;
-        for (uint32_t i = (uint32_t)0U; i < i0 / (uint32_t)4U * (uint32_t)4U / (uint32_t)4U; i++)
+        for (uint32_t i = (uint32_t)0U; i < i0 / (uint32_t)4U; i++)
         {
           uint64_t a_i = ab[(uint32_t)4U * i];
           uint64_t *res_i0 = res_j + (uint32_t)4U * i;
@@ -11827,10 +12606,10 @@ Hacl_P256_ecdsa_verif_without_hash(
         uint64_t r12 = c;
         t[i0 + i0] = r12;
       }
-      uint64_t c00 = bn_add_eq_len_u64(resLen0, t, t, t);
-      KRML_CHECK_SIZE(sizeof (uint64_t), resLen0);
-      uint64_t tmp3[resLen0];
-      memset(tmp3, 0U, resLen0 * sizeof (uint64_t));
+      uint64_t c00 = bn_add_eq_len_u64(len70 + len70, t, t, t);
+      KRML_CHECK_SIZE(sizeof (uint64_t), len70 + len70);
+      uint64_t tmp3[len70 + len70];
+      memset(tmp3, 0U, (len70 + len70) * sizeof (uint64_t));
       for (uint32_t i = (uint32_t)0U; i < len70; i++)
       {
         uint128_t res = (uint128_t)z1[i] * z1[i];
@@ -11839,7 +12618,7 @@ Hacl_P256_ecdsa_verif_without_hash(
         tmp3[(uint32_t)2U * i] = lo;
         tmp3[(uint32_t)2U * i + (uint32_t)1U] = hi;
       }
-      uint64_t c10 = bn_add_eq_len_u64(resLen0, t, tmp3, t);
+      uint64_t c10 = bn_add_eq_len_u64(len70 + len70, t, tmp3, t);
       uint32_t len71 = (uint32_t)4U;
       KRML_CHECK_SIZE(sizeof (uint64_t), (uint32_t)2U * len71);
       uint64_t t20[(uint32_t)2U * len71];
@@ -11878,7 +12657,7 @@ Hacl_P256_ecdsa_verif_without_hash(
         mul64(f3, t10, o3, o4);
         uint32_t len92 = (uint32_t)4U * (uint32_t)2U;
         uint64_t c = (uint64_t)0U;
-        for (uint32_t i = (uint32_t)0U; i < len92 / (uint32_t)4U * (uint32_t)4U / (uint32_t)4U; i++)
+        for (uint32_t i = (uint32_t)0U; i < len92 / (uint32_t)4U; i++)
         {
           uint64_t t1 = t[(uint32_t)4U * i];
           uint64_t t210 = t20[(uint32_t)4U * i];
@@ -11931,7 +12710,7 @@ Hacl_P256_ecdsa_verif_without_hash(
         };
       uint32_t len100 = (uint32_t)4U;
       uint64_t c3 = (uint64_t)0U;
-      for (uint32_t i = (uint32_t)0U; i < len100 / (uint32_t)4U * (uint32_t)4U / (uint32_t)4U; i++)
+      for (uint32_t i = (uint32_t)0U; i < len100 / (uint32_t)4U; i++)
       {
         uint64_t t1 = x_0[(uint32_t)4U * i];
         uint64_t t210 = p10[(uint32_t)4U * i];
@@ -11971,15 +12750,14 @@ Hacl_P256_ecdsa_verif_without_hash(
       uint64_t t0[(uint32_t)2U * len64];
       memset(t0, 0U, (uint32_t)2U * len64 * sizeof (uint64_t));
       uint32_t len72 = (uint32_t)4U;
-      uint32_t resLen1 = len72 + len72;
-      memset(t0, 0U, resLen1 * sizeof (uint64_t));
+      memset(t0, 0U, (len72 + len72) * sizeof (uint64_t));
       for (uint32_t i0 = (uint32_t)0U; i0 < len72; i0++)
       {
         uint64_t *ab = z2;
         uint64_t a_j = z2[i0];
         uint64_t *res_j = t0 + i0;
         uint64_t c = (uint64_t)0U;
-        for (uint32_t i = (uint32_t)0U; i < i0 / (uint32_t)4U * (uint32_t)4U / (uint32_t)4U; i++)
+        for (uint32_t i = (uint32_t)0U; i < i0 / (uint32_t)4U; i++)
         {
           uint64_t a_i = ab[(uint32_t)4U * i];
           uint64_t *res_i0 = res_j + (uint32_t)4U * i;
@@ -12003,10 +12781,10 @@ Hacl_P256_ecdsa_verif_without_hash(
         uint64_t r13 = c;
         t0[i0 + i0] = r13;
       }
-      uint64_t c0 = bn_add_eq_len_u64(resLen1, t0, t0, t0);
-      KRML_CHECK_SIZE(sizeof (uint64_t), resLen1);
-      uint64_t tmp4[resLen1];
-      memset(tmp4, 0U, resLen1 * sizeof (uint64_t));
+      uint64_t c0 = bn_add_eq_len_u64(len72 + len72, t0, t0, t0);
+      KRML_CHECK_SIZE(sizeof (uint64_t), len72 + len72);
+      uint64_t tmp4[len72 + len72];
+      memset(tmp4, 0U, (len72 + len72) * sizeof (uint64_t));
       for (uint32_t i = (uint32_t)0U; i < len72; i++)
       {
         uint128_t res = (uint128_t)z2[i] * z2[i];
@@ -12015,7 +12793,7 @@ Hacl_P256_ecdsa_verif_without_hash(
         tmp4[(uint32_t)2U * i] = lo;
         tmp4[(uint32_t)2U * i + (uint32_t)1U] = hi;
       }
-      uint64_t c11 = bn_add_eq_len_u64(resLen1, t0, tmp4, t0);
+      uint64_t c11 = bn_add_eq_len_u64(len72 + len72, t0, tmp4, t0);
       uint32_t len73 = (uint32_t)4U;
       KRML_CHECK_SIZE(sizeof (uint64_t), (uint32_t)2U * len73);
       uint64_t t22[(uint32_t)2U * len73];
@@ -12054,7 +12832,7 @@ Hacl_P256_ecdsa_verif_without_hash(
         mul64(f3, t10, o3, o4);
         uint32_t len93 = (uint32_t)4U * (uint32_t)2U;
         uint64_t c = (uint64_t)0U;
-        for (uint32_t i = (uint32_t)0U; i < len93 / (uint32_t)4U * (uint32_t)4U / (uint32_t)4U; i++)
+        for (uint32_t i = (uint32_t)0U; i < len93 / (uint32_t)4U; i++)
         {
           uint64_t t1 = t0[(uint32_t)4U * i];
           uint64_t t210 = t22[(uint32_t)4U * i];
@@ -12107,7 +12885,7 @@ Hacl_P256_ecdsa_verif_without_hash(
         };
       uint32_t len101 = (uint32_t)4U;
       uint64_t c4 = (uint64_t)0U;
-      for (uint32_t i = (uint32_t)0U; i < len101 / (uint32_t)4U * (uint32_t)4U / (uint32_t)4U; i++)
+      for (uint32_t i = (uint32_t)0U; i < len101 / (uint32_t)4U; i++)
       {
         uint64_t t1 = x_1[(uint32_t)4U * i];
         uint64_t t210 = p11[(uint32_t)4U * i];
@@ -12147,14 +12925,13 @@ Hacl_P256_ecdsa_verif_without_hash(
       uint64_t t3[(uint32_t)2U * len65];
       memset(t3, 0U, (uint32_t)2U * len65 * sizeof (uint64_t));
       uint32_t len74 = (uint32_t)4U;
-      uint32_t resLen2 = len74 + len74;
-      memset(t3, 0U, resLen2 * sizeof (uint64_t));
+      memset(t3, 0U, (len74 + len74) * sizeof (uint64_t));
       for (uint32_t i0 = (uint32_t)0U; i0 < len74; i0++)
       {
         uint64_t bj = z1[i0];
         uint64_t *res_j = t3 + i0;
         uint64_t c = (uint64_t)0U;
-        for (uint32_t i = (uint32_t)0U; i < len74 / (uint32_t)4U * (uint32_t)4U / (uint32_t)4U; i++)
+        for (uint32_t i = (uint32_t)0U; i < len74 / (uint32_t)4U; i++)
         {
           uint64_t a_i = sq_z1[(uint32_t)4U * i];
           uint64_t *res_i0 = res_j + (uint32_t)4U * i;
@@ -12216,7 +12993,7 @@ Hacl_P256_ecdsa_verif_without_hash(
         mul64(f3, t10, o3, o4);
         uint32_t len94 = (uint32_t)4U * (uint32_t)2U;
         uint64_t c = (uint64_t)0U;
-        for (uint32_t i = (uint32_t)0U; i < len94 / (uint32_t)4U * (uint32_t)4U / (uint32_t)4U; i++)
+        for (uint32_t i = (uint32_t)0U; i < len94 / (uint32_t)4U; i++)
         {
           uint64_t t1 = t3[(uint32_t)4U * i];
           uint64_t t210 = t23[(uint32_t)4U * i];
@@ -12269,7 +13046,7 @@ Hacl_P256_ecdsa_verif_without_hash(
         };
       uint32_t len102 = (uint32_t)4U;
       uint64_t c5 = (uint64_t)0U;
-      for (uint32_t i = (uint32_t)0U; i < len102 / (uint32_t)4U * (uint32_t)4U / (uint32_t)4U; i++)
+      for (uint32_t i = (uint32_t)0U; i < len102 / (uint32_t)4U; i++)
       {
         uint64_t t1 = x_2[(uint32_t)4U * i];
         uint64_t t210 = p12[(uint32_t)4U * i];
@@ -12309,14 +13086,13 @@ Hacl_P256_ecdsa_verif_without_hash(
       uint64_t t4[(uint32_t)2U * len66];
       memset(t4, 0U, (uint32_t)2U * len66 * sizeof (uint64_t));
       uint32_t len76 = (uint32_t)4U;
-      uint32_t resLen3 = len76 + len76;
-      memset(t4, 0U, resLen3 * sizeof (uint64_t));
+      memset(t4, 0U, (len76 + len76) * sizeof (uint64_t));
       for (uint32_t i0 = (uint32_t)0U; i0 < len76; i0++)
       {
         uint64_t bj = z2[i0];
         uint64_t *res_j = t4 + i0;
         uint64_t c = (uint64_t)0U;
-        for (uint32_t i = (uint32_t)0U; i < len76 / (uint32_t)4U * (uint32_t)4U / (uint32_t)4U; i++)
+        for (uint32_t i = (uint32_t)0U; i < len76 / (uint32_t)4U; i++)
         {
           uint64_t a_i = sq_z2[(uint32_t)4U * i];
           uint64_t *res_i0 = res_j + (uint32_t)4U * i;
@@ -12378,7 +13154,7 @@ Hacl_P256_ecdsa_verif_without_hash(
         mul64(f3, t10, o3, o4);
         uint32_t len95 = (uint32_t)4U * (uint32_t)2U;
         uint64_t c = (uint64_t)0U;
-        for (uint32_t i = (uint32_t)0U; i < len95 / (uint32_t)4U * (uint32_t)4U / (uint32_t)4U; i++)
+        for (uint32_t i = (uint32_t)0U; i < len95 / (uint32_t)4U; i++)
         {
           uint64_t t1 = t4[(uint32_t)4U * i];
           uint64_t t210 = t24[(uint32_t)4U * i];
@@ -12431,7 +13207,7 @@ Hacl_P256_ecdsa_verif_without_hash(
         };
       uint32_t len103 = (uint32_t)4U;
       uint64_t c6 = (uint64_t)0U;
-      for (uint32_t i = (uint32_t)0U; i < len103 / (uint32_t)4U * (uint32_t)4U / (uint32_t)4U; i++)
+      for (uint32_t i = (uint32_t)0U; i < len103 / (uint32_t)4U; i++)
       {
         uint64_t t1 = x_3[(uint32_t)4U * i];
         uint64_t t210 = p13[(uint32_t)4U * i];
@@ -12471,14 +13247,13 @@ Hacl_P256_ecdsa_verif_without_hash(
       uint64_t t5[(uint32_t)2U * len67];
       memset(t5, 0U, (uint32_t)2U * len67 * sizeof (uint64_t));
       uint32_t len78 = (uint32_t)4U;
-      uint32_t resLen4 = len78 + len78;
-      memset(t5, 0U, resLen4 * sizeof (uint64_t));
+      memset(t5, 0U, (len78 + len78) * sizeof (uint64_t));
       for (uint32_t i0 = (uint32_t)0U; i0 < len78; i0++)
       {
         uint64_t bj = x2[i0];
         uint64_t *res_j = t5 + i0;
         uint64_t c = (uint64_t)0U;
-        for (uint32_t i = (uint32_t)0U; i < len78 / (uint32_t)4U * (uint32_t)4U / (uint32_t)4U; i++)
+        for (uint32_t i = (uint32_t)0U; i < len78 / (uint32_t)4U; i++)
         {
           uint64_t a_i = sq_z1[(uint32_t)4U * i];
           uint64_t *res_i0 = res_j + (uint32_t)4U * i;
@@ -12540,7 +13315,7 @@ Hacl_P256_ecdsa_verif_without_hash(
         mul64(f3, t10, o3, o4);
         uint32_t len96 = (uint32_t)4U * (uint32_t)2U;
         uint64_t c = (uint64_t)0U;
-        for (uint32_t i = (uint32_t)0U; i < len96 / (uint32_t)4U * (uint32_t)4U / (uint32_t)4U; i++)
+        for (uint32_t i = (uint32_t)0U; i < len96 / (uint32_t)4U; i++)
         {
           uint64_t t1 = t5[(uint32_t)4U * i];
           uint64_t t210 = t25[(uint32_t)4U * i];
@@ -12593,7 +13368,7 @@ Hacl_P256_ecdsa_verif_without_hash(
         };
       uint32_t len104 = (uint32_t)4U;
       uint64_t c7 = (uint64_t)0U;
-      for (uint32_t i = (uint32_t)0U; i < len104 / (uint32_t)4U * (uint32_t)4U / (uint32_t)4U; i++)
+      for (uint32_t i = (uint32_t)0U; i < len104 / (uint32_t)4U; i++)
       {
         uint64_t t1 = x_4[(uint32_t)4U * i];
         uint64_t t210 = p14[(uint32_t)4U * i];
@@ -12633,19 +13408,13 @@ Hacl_P256_ecdsa_verif_without_hash(
       uint64_t t6[(uint32_t)2U * len68];
       memset(t6, 0U, (uint32_t)2U * len68 * sizeof (uint64_t));
       uint32_t len710 = (uint32_t)4U;
-      uint32_t resLen5 = len710 + len710;
-      memset(t6, 0U, resLen5 * sizeof (uint64_t));
+      memset(t6, 0U, (len710 + len710) * sizeof (uint64_t));
       for (uint32_t i0 = (uint32_t)0U; i0 < len710; i0++)
       {
         uint64_t bj = x1[i0];
         uint64_t *res_j = t6 + i0;
         uint64_t c = (uint64_t)0U;
-        for
-        (uint32_t
-          i = (uint32_t)0U;
-          i
-          < len710 / (uint32_t)4U * (uint32_t)4U / (uint32_t)4U;
-          i++)
+        for (uint32_t i = (uint32_t)0U; i < len710 / (uint32_t)4U; i++)
         {
           uint64_t a_i = sq_z2[(uint32_t)4U * i];
           uint64_t *res_i0 = res_j + (uint32_t)4U * i;
@@ -12707,7 +13476,7 @@ Hacl_P256_ecdsa_verif_without_hash(
         mul64(f3, t10, o3, o4);
         uint32_t len97 = (uint32_t)4U * (uint32_t)2U;
         uint64_t c = (uint64_t)0U;
-        for (uint32_t i = (uint32_t)0U; i < len97 / (uint32_t)4U * (uint32_t)4U / (uint32_t)4U; i++)
+        for (uint32_t i = (uint32_t)0U; i < len97 / (uint32_t)4U; i++)
         {
           uint64_t t1 = t6[(uint32_t)4U * i];
           uint64_t t210 = t26[(uint32_t)4U * i];
@@ -12760,7 +13529,7 @@ Hacl_P256_ecdsa_verif_without_hash(
         };
       uint32_t len105 = (uint32_t)4U;
       uint64_t c8 = (uint64_t)0U;
-      for (uint32_t i = (uint32_t)0U; i < len105 / (uint32_t)4U * (uint32_t)4U / (uint32_t)4U; i++)
+      for (uint32_t i = (uint32_t)0U; i < len105 / (uint32_t)4U; i++)
       {
         uint64_t t1 = x_5[(uint32_t)4U * i];
         uint64_t t210 = p15[(uint32_t)4U * i];
@@ -12800,19 +13569,13 @@ Hacl_P256_ecdsa_verif_without_hash(
       uint64_t t7[(uint32_t)2U * len69];
       memset(t7, 0U, (uint32_t)2U * len69 * sizeof (uint64_t));
       uint32_t len712 = (uint32_t)4U;
-      uint32_t resLen6 = len712 + len712;
-      memset(t7, 0U, resLen6 * sizeof (uint64_t));
+      memset(t7, 0U, (len712 + len712) * sizeof (uint64_t));
       for (uint32_t i0 = (uint32_t)0U; i0 < len712; i0++)
       {
         uint64_t bj = y2[i0];
         uint64_t *res_j = t7 + i0;
         uint64_t c = (uint64_t)0U;
-        for
-        (uint32_t
-          i = (uint32_t)0U;
-          i
-          < len712 / (uint32_t)4U * (uint32_t)4U / (uint32_t)4U;
-          i++)
+        for (uint32_t i = (uint32_t)0U; i < len712 / (uint32_t)4U; i++)
         {
           uint64_t a_i = tr_z1[(uint32_t)4U * i];
           uint64_t *res_i0 = res_j + (uint32_t)4U * i;
@@ -12874,7 +13637,7 @@ Hacl_P256_ecdsa_verif_without_hash(
         mul64(f3, t10, o3, o4);
         uint32_t len98 = (uint32_t)4U * (uint32_t)2U;
         uint64_t c = (uint64_t)0U;
-        for (uint32_t i = (uint32_t)0U; i < len98 / (uint32_t)4U * (uint32_t)4U / (uint32_t)4U; i++)
+        for (uint32_t i = (uint32_t)0U; i < len98 / (uint32_t)4U; i++)
         {
           uint64_t t1 = t7[(uint32_t)4U * i];
           uint64_t t210 = t27[(uint32_t)4U * i];
@@ -12927,7 +13690,7 @@ Hacl_P256_ecdsa_verif_without_hash(
         };
       uint32_t len106 = (uint32_t)4U;
       uint64_t c9 = (uint64_t)0U;
-      for (uint32_t i = (uint32_t)0U; i < len106 / (uint32_t)4U * (uint32_t)4U / (uint32_t)4U; i++)
+      for (uint32_t i = (uint32_t)0U; i < len106 / (uint32_t)4U; i++)
       {
         uint64_t t1 = x_6[(uint32_t)4U * i];
         uint64_t t210 = p16[(uint32_t)4U * i];
@@ -12967,14 +13730,13 @@ Hacl_P256_ecdsa_verif_without_hash(
       uint64_t t8[(uint32_t)2U * len610];
       memset(t8, 0U, (uint32_t)2U * len610 * sizeof (uint64_t));
       uint32_t len7 = (uint32_t)4U;
-      uint32_t resLen = len7 + len7;
-      memset(t8, 0U, resLen * sizeof (uint64_t));
+      memset(t8, 0U, (len7 + len7) * sizeof (uint64_t));
       for (uint32_t i0 = (uint32_t)0U; i0 < len7; i0++)
       {
         uint64_t bj = y1[i0];
         uint64_t *res_j = t8 + i0;
         uint64_t c = (uint64_t)0U;
-        for (uint32_t i = (uint32_t)0U; i < len7 / (uint32_t)4U * (uint32_t)4U / (uint32_t)4U; i++)
+        for (uint32_t i = (uint32_t)0U; i < len7 / (uint32_t)4U; i++)
         {
           uint64_t a_i = tr_z2[(uint32_t)4U * i];
           uint64_t *res_i0 = res_j + (uint32_t)4U * i;
@@ -13036,7 +13798,7 @@ Hacl_P256_ecdsa_verif_without_hash(
         mul64(f3, t10, o3, o4);
         uint32_t len99 = (uint32_t)4U * (uint32_t)2U;
         uint64_t c = (uint64_t)0U;
-        for (uint32_t i = (uint32_t)0U; i < len99 / (uint32_t)4U * (uint32_t)4U / (uint32_t)4U; i++)
+        for (uint32_t i = (uint32_t)0U; i < len99 / (uint32_t)4U; i++)
         {
           uint64_t t1 = t8[(uint32_t)4U * i];
           uint64_t t210 = t2[(uint32_t)4U * i];
@@ -13089,7 +13851,7 @@ Hacl_P256_ecdsa_verif_without_hash(
         };
       uint32_t len10 = (uint32_t)4U;
       uint64_t c = (uint64_t)0U;
-      for (uint32_t i = (uint32_t)0U; i < len10 / (uint32_t)4U * (uint32_t)4U / (uint32_t)4U; i++)
+      for (uint32_t i = (uint32_t)0U; i < len10 / (uint32_t)4U; i++)
       {
         uint64_t t1 = x_[(uint32_t)4U * i];
         uint64_t t210 = p1[(uint32_t)4U * i];
@@ -13260,48 +14022,53 @@ uint64_t Hacl_P256_ecp256dh_i(uint8_t *result, uint8_t *scalar)
   uint32_t len1 = (uint32_t)4U;
   uint64_t *q = tempBuffer;
   uint64_t *buff = tempBuffer + (uint32_t)3U * len1;
-  uint32_t len20 = (uint32_t)4U;
-  uint64_t *x = q;
-  uint64_t *y = q + len20;
-  uint64_t *z = q + (uint32_t)2U * len20;
-  uint32_t len3 = (uint32_t)4U;
-  for (uint32_t i = (uint32_t)0U; i < len3; i++)
-  {
-    x[i] = (uint64_t)0U;
-  }
-  uint32_t len30 = (uint32_t)4U;
-  for (uint32_t i = (uint32_t)0U; i < len30; i++)
-  {
-    y[i] = (uint64_t)0U;
-  }
-  uint32_t len31 = (uint32_t)4U;
-  for (uint32_t i = (uint32_t)0U; i < len31; i++)
-  {
-    z[i] = (uint64_t)0U;
-  }
-  resultBuffer[0U] = (uint64_t)0x79e730d418a9143cU;
-  resultBuffer[1U] = (uint64_t)0x75ba95fc5fedb601U;
-  resultBuffer[2U] = (uint64_t)0x79fb732b77622510U;
-  resultBuffer[3U] = (uint64_t)0x18905f76a53755c6U;
-  resultBuffer[4U] = (uint64_t)0xddf25357ce95560aU;
-  resultBuffer[5U] = (uint64_t)0x8b4ab8e4ba19e45cU;
-  resultBuffer[6U] = (uint64_t)0xd2e88688dd21f325U;
-  resultBuffer[7U] = (uint64_t)0x8571ff1825885d85U;
-  resultBuffer[8U] = (uint64_t)0x1U;
-  resultBuffer[9U] = (uint64_t)0xffffffff00000000U;
-  resultBuffer[10U] = (uint64_t)0xffffffffffffffffU;
-  resultBuffer[11U] = (uint64_t)0xfffffffeU;
-  uint32_t half = (uint32_t)(krml_checked_int_t)0 >> (uint32_t)1U;
-  uint32_t word = (uint32_t)scalar[half];
-  uint32_t bitShift = (uint32_t)(krml_checked_int_t)0 & (uint32_t)1U;
-  uint32_t bitShiftAsPrivate = bitShift;
-  uint64_t mask = (uint64_t)0U - (uint64_t)bitShiftAsPrivate;
-  uint32_t mask0 = (uint32_t)0xf0U ^ (uint32_t)(mask & (uint64_t)(uint32_t)255U);
-  uint64_t mask1 = (uint64_t)0U - (uint64_t)bitShift;
-  uint32_t shiftMask = (uint32_t)0x4U ^ (uint32_t)(mask1 & (uint64_t)(uint32_t)4U);
-  uint32_t result1 = word & mask0;
-  uint32_t bits = result1 >> shiftMask;
-  const uint64_t *pointToStart = points_radix_16 + bits * (uint32_t)8U;
+  uint32_t
+  bit =
+    (uint32_t)4U
+    * (uint32_t)8U
+    * (uint32_t)8U
+    - (uint32_t)1U
+    - ((uint32_t)(krml_checked_int_t)0 << (uint32_t)2U);
+  uint64_t
+  bit0 =
+    (uint64_t)(scalar[(uint32_t)4U
+    * (uint32_t)8U
+    - (uint32_t)1U
+    - bit / (uint32_t)8U]
+    >> bit % (uint32_t)8U
+    & (uint8_t)1U)
+    << (uint32_t)3U;
+  uint64_t
+  bit1 =
+    (uint64_t)(scalar[(uint32_t)4U
+    * (uint32_t)8U
+    - (uint32_t)1U
+    - (bit - (uint32_t)1U) / (uint32_t)8U]
+    >> (bit - (uint32_t)1U) % (uint32_t)8U
+    & (uint8_t)1U)
+    << (uint32_t)2U;
+  uint64_t
+  bit2 =
+    (uint64_t)(scalar[(uint32_t)4U
+    * (uint32_t)8U
+    - (uint32_t)1U
+    - (bit - (uint32_t)2U) / (uint32_t)8U]
+    >> (bit - (uint32_t)2U) % (uint32_t)8U
+    & (uint8_t)1U)
+    << (uint32_t)1U;
+  uint64_t
+  bit3 =
+    (uint64_t)(scalar[(uint32_t)4U
+    * (uint32_t)8U
+    - (uint32_t)1U
+    - (bit - (uint32_t)3U) / (uint32_t)8U]
+    >> (bit - (uint32_t)3U) % (uint32_t)8U
+    & (uint8_t)1U)
+    << (uint32_t)0U;
+  uint64_t bits = (bit0 ^ bit1) ^ (bit2 ^ bit3);
+  const
+  uint64_t
+  *pointToStart = points_radix_p256_16 + (uint32_t)(bits * (uint64_t)(uint32_t)8U);
   memcpy(resultBuffer, (uint64_t *)pointToStart, (uint32_t)8U * sizeof (uint64_t));
   resultBuffer[8U] = (uint64_t)1U;
   resultBuffer[9U] = (uint64_t)0U;
@@ -13310,7 +14077,7 @@ uint64_t Hacl_P256_ecp256dh_i(uint8_t *result, uint8_t *scalar)
   for (uint32_t i = (uint32_t)1U; i < (uint32_t)64U; i++)
   {
     uint64_t pointToAdd[8U] = { 0U };
-    getPointPrecomputedMixed_p256(scalar, i, pointToAdd);
+    getPointPrecomputedMixed_p256((void *)scalar, i, pointToAdd);
     point_double_p256(resultBuffer, resultBuffer, buff);
     point_double_p256(resultBuffer, resultBuffer, buff);
     point_double_p256(resultBuffer, resultBuffer, buff);
@@ -13350,54 +14117,53 @@ uint64_t Hacl_P256_ecp384dh_i(uint8_t *result, uint8_t *scalar)
   uint32_t len1 = (uint32_t)6U;
   uint64_t *q = tempBuffer;
   uint64_t *buff = tempBuffer + (uint32_t)3U * len1;
-  uint32_t len20 = (uint32_t)6U;
-  uint64_t *x = q;
-  uint64_t *y = q + len20;
-  uint64_t *z = q + (uint32_t)2U * len20;
-  uint32_t len3 = (uint32_t)6U;
-  for (uint32_t i = (uint32_t)0U; i < len3; i++)
-  {
-    x[i] = (uint64_t)0U;
-  }
-  uint32_t len30 = (uint32_t)6U;
-  for (uint32_t i = (uint32_t)0U; i < len30; i++)
-  {
-    y[i] = (uint64_t)0U;
-  }
-  uint32_t len31 = (uint32_t)6U;
-  for (uint32_t i = (uint32_t)0U; i < len31; i++)
-  {
-    z[i] = (uint64_t)0U;
-  }
-  resultBuffer[0U] = (uint64_t)0x3dd0756649c0b528U;
-  resultBuffer[1U] = (uint64_t)0x20e378e2a0d6ce38U;
-  resultBuffer[2U] = (uint64_t)0x879c3afc541b4d6eU;
-  resultBuffer[3U] = (uint64_t)0x6454868459a30effU;
-  resultBuffer[4U] = (uint64_t)0x812ff723614ede2bU;
-  resultBuffer[5U] = (uint64_t)0x4d3aadc2299e1513U;
-  resultBuffer[6U] = (uint64_t)0x23043dad4b03a4feU;
-  resultBuffer[7U] = (uint64_t)0xa1bfa8bf7bb4a9acU;
-  resultBuffer[8U] = (uint64_t)0x8bade7562e83b050U;
-  resultBuffer[9U] = (uint64_t)0xc6c3521968f4ffd9U;
-  resultBuffer[10U] = (uint64_t)0xdd8002263969a840U;
-  resultBuffer[11U] = (uint64_t)0x2b78abc25a15c5e9U;
-  resultBuffer[12U] = (uint64_t)0xffffffff00000001U;
-  resultBuffer[13U] = (uint64_t)0xffffffffU;
-  resultBuffer[14U] = (uint64_t)0x1U;
-  resultBuffer[15U] = (uint64_t)0U;
-  resultBuffer[16U] = (uint64_t)0U;
-  resultBuffer[17U] = (uint64_t)0U;
-  uint32_t half = (uint32_t)(krml_checked_int_t)0 >> (uint32_t)1U;
-  uint32_t word = (uint32_t)scalar[half];
-  uint32_t bitShift = (uint32_t)(krml_checked_int_t)0 & (uint32_t)1U;
-  uint32_t bitShiftAsPrivate = bitShift;
-  uint64_t mask = (uint64_t)0U - (uint64_t)bitShiftAsPrivate;
-  uint32_t mask0 = (uint32_t)0xf0U ^ (uint32_t)(mask & (uint64_t)(uint32_t)255U);
-  uint64_t mask1 = (uint64_t)0U - (uint64_t)bitShift;
-  uint32_t shiftMask = (uint32_t)0x4U ^ (uint32_t)(mask1 & (uint64_t)(uint32_t)4U);
-  uint32_t result1 = word & mask0;
-  uint32_t bits = result1 >> shiftMask;
-  const uint64_t *pointToStart = points_radix_16 + bits * (uint32_t)8U;
+  uint32_t
+  bit =
+    (uint32_t)6U
+    * (uint32_t)8U
+    * (uint32_t)8U
+    - (uint32_t)1U
+    - ((uint32_t)(krml_checked_int_t)0 << (uint32_t)2U);
+  uint64_t
+  bit0 =
+    (uint64_t)(scalar[(uint32_t)6U
+    * (uint32_t)8U
+    - (uint32_t)1U
+    - bit / (uint32_t)8U]
+    >> bit % (uint32_t)8U
+    & (uint8_t)1U)
+    << (uint32_t)3U;
+  uint64_t
+  bit1 =
+    (uint64_t)(scalar[(uint32_t)6U
+    * (uint32_t)8U
+    - (uint32_t)1U
+    - (bit - (uint32_t)1U) / (uint32_t)8U]
+    >> (bit - (uint32_t)1U) % (uint32_t)8U
+    & (uint8_t)1U)
+    << (uint32_t)2U;
+  uint64_t
+  bit2 =
+    (uint64_t)(scalar[(uint32_t)6U
+    * (uint32_t)8U
+    - (uint32_t)1U
+    - (bit - (uint32_t)2U) / (uint32_t)8U]
+    >> (bit - (uint32_t)2U) % (uint32_t)8U
+    & (uint8_t)1U)
+    << (uint32_t)1U;
+  uint64_t
+  bit3 =
+    (uint64_t)(scalar[(uint32_t)6U
+    * (uint32_t)8U
+    - (uint32_t)1U
+    - (bit - (uint32_t)3U) / (uint32_t)8U]
+    >> (bit - (uint32_t)3U) % (uint32_t)8U
+    & (uint8_t)1U)
+    << (uint32_t)0U;
+  uint64_t bits = (bit0 ^ bit1) ^ (bit2 ^ bit3);
+  const
+  uint64_t
+  *pointToStart = points_radix_p256_16 + (uint32_t)(bits * (uint64_t)(uint32_t)8U);
   memcpy(resultBuffer, (uint64_t *)pointToStart, (uint32_t)8U * sizeof (uint64_t));
   resultBuffer[8U] = (uint64_t)1U;
   resultBuffer[9U] = (uint64_t)0U;
@@ -13406,12 +14172,12 @@ uint64_t Hacl_P256_ecp384dh_i(uint8_t *result, uint8_t *scalar)
   for (uint32_t i = (uint32_t)1U; i < (uint32_t)64U; i++)
   {
     uint64_t pointToAdd[8U] = { 0U };
-    getPointPrecomputedMixed_p256(scalar, i, pointToAdd);
+    getPointPrecomputedMixed_p256((void *)scalar, i, pointToAdd);
     point_double_p384(resultBuffer, resultBuffer, buff);
     point_double_p384(resultBuffer, resultBuffer, buff);
     point_double_p384(resultBuffer, resultBuffer, buff);
     point_double_p384(resultBuffer, resultBuffer, buff);
-    point_add_mixed_p256(resultBuffer, pointToAdd, resultBuffer, buff);
+    point_add_mixed_p384(resultBuffer, pointToAdd, resultBuffer, buff);
   }
   memcpy(q, resultBuffer, (uint32_t)18U * sizeof (uint64_t));
   norm_p384(q, resultBuffer, buff);
