code/ecdsa/dist/Hacl_P256.h
@@ -32,6 +32,7 @@
 
 #include "Hacl_Kremlib.h"
 #include "Hacl_Hash_SHA2.h"
+#include "Hacl_Spec.h"
 
 /*
  Input: result buffer: uint8[64], 
