code/ecdsa/dist/Hacl_Spec.h
@@ -43,6 +43,12 @@
 
 typedef uint8_t Spec_Hash_Definitions_hash_alg;
 
+#define Spec_ECC_Curves_P256 0
+#define Spec_ECC_Curves_P384 1
+#define Spec_ECC_Curves_Default 2
+
+typedef uint8_t Spec_ECC_Curves_curve;
+
 
 #define __Hacl_Spec_H_DEFINED
 #endif
