specs/ecdsa/Spec.ECC.fst
@@ -206,4 +206,444 @@ let pointAdd #curve (p:point_nat_prime #curve) (q:point_nat_prime #curve) : poin
     _point_add p q
 
 
-let point_mult #c i (p: point_nat_prime #c) : point_nat_prime #c  = repeat ((i - 1) % getOrder #c) (fun x -> pointAdd #c p x) p
+val _ml_step0: #c: curve -> r0: point_nat_prime #c -> r1: point_nat_prime #c -> tuple2 (point_nat_prime #c) (point_nat_prime #c) 
+
+let _ml_step0 #c r0 r1 =
+  let r0 = pointAdd r1 r0 in
+  let r1 = pointAdd r1 r1 in
+  (r0, r1)
+
+
+val _ml_step1: #c: curve -> r0: point_nat_prime #c -> r1: point_nat_prime #c -> tuple2 (point_nat_prime #c) (point_nat_prime #c)
+
+let _ml_step1 #c r0 r1 =
+  let r1 = pointAdd r0 r1 in
+  let r0 = pointAdd r0 r0 in
+  (r0, r1)
+
+
+val _ml_step: #c: curve -> k: scalar_bytes #c -> i: nat{i < v (getScalarLen c)} 
+  -> r: tuple2 (point_nat_prime #c) (point_nat_prime #c)
+  -> tuple2 (point_nat_prime #c) (point_nat_prime #c)
+
+let _ml_step #c k i (p, q) =
+  let bit = v (getScalarLen c) - 1 - i in
+  let bit = ith_bit k bit in
+  if uint_to_nat bit = 0 then
+    _ml_step1 p q
+  else
+    _ml_step0 p q
+
+(* P + R == P + Q <==> R == Q --> P + P == P + Q <==> P == Q *)
+assume val curve_point_equality: #c: curve -> p: point_nat_prime #c -> q: point_nat_prime #c -> Lemma 
+  (pointEqual (pointAdd p q) (pointAdd p p) <==> pointEqual p q)
+
+(* P + Q == Q + P *)
+assume val curve_commutativity_lemma: #c: curve -> p: point_nat_prime #c -> q: point_nat_prime #c -> Lemma 
+  (pointEqual (pointAdd p q) (pointAdd q p))
+
+(* P == P' ==> P + Q == P' + Q *)
+assume val curve_compatibility_with_translation_lemma: #c: curve -> p: point_nat_prime #c -> p1: point_nat_prime #c {pointEqual p p1}
+  -> q: point_nat_prime #c -> 
+  Lemma (pointEqual (pointAdd p q) (pointAdd p1 q))
+
+(* order is the smallest number such that P * order == 0 *)
+
+assume val curve_order_is_the_smallest: #c: curve -> p: point_nat_prime #c -> Lemma
+  (forall (n: nat {repeat n (fun x -> pointAdd #c p x) p == pointAtInfinity}). n >= getOrder #c)
+
+(* order * P == 0 *)
+assume val curve_multiplication_by_order: #c: curve -> i: int {(i + 1) % getOrder #c = 0} -> p: point_nat_prime -> 
+  Lemma (repeat (i % getOrder #c) (fun x -> pointAdd #c p x) p == pointAtInfinity)
+
+(* P + 0 == P *)
+assume val curve_point_at_infinity_property: #c: curve -> q: point_nat_prime #c -> Lemma (pointEqual (pointAdd pointAtInfinity q) q)
+
+assume val curve_associativity: #c: curve -> p: point_nat_prime #c -> q: point_nat_prime #c -> r: point_nat_prime #c -> Lemma 
+  (pointEqual (pointAdd (pointAdd p q) r) (pointAdd p (pointAdd q r)))
+
+val point_mult: #c: curve -> i: int -> p: point_nat_prime #c -> point_nat_prime #c
+
+let point_mult #c i p = repeat ((i - 1) % getOrder #c) (fun x -> pointAdd #c p x) p
+
+val point_mult_0: #c: curve -> p: point_nat_prime #c -> i: int {i % getOrder #c = 0} -> 
+  Lemma (point_mult #c i p == pointAtInfinity)
+
+let point_mult_0 #c p i = curve_multiplication_by_order #c (getOrder #c - 1) p
+
+
+val point_mult_1: #c: curve ->p: point_nat_prime #c ->  Lemma (point_mult #c 1 p == p)
+
+let point_mult_1 #c p = eq_repeat0 (fun x -> pointAdd #c p x) p 
+
+
+val point_mult_ext: #c: curve -> i: int -> p: point_nat_prime #c -> Lemma (
+  let f = (fun x -> pointAdd #c p x) in  
+  pointEqual (f (point_mult #c i p)) (point_mult #c (i + 1) p))
+
+let point_mult_ext #c i p = 
+  let f = (fun x -> pointAdd #c p x) in 
+  if i % getOrder #c = 0 then 
+    begin
+      point_mult_0 #c p 0;
+      curve_point_at_infinity_property p;  
+      curve_commutativity_lemma pointAtInfinity p; 
+      point_mult_1 #c p
+    end
+  else 
+    begin
+      unfold_repeat (getOrder #c) f p ((i - 1) % getOrder #c);
+      lemma_mod_add_distr 1 (i - 1) (getOrder #c)
+    end
+
+val lemma_scalar_reduce: #c: curve -> p: point_nat_prime #c -> pk: int -> Lemma (point_mult pk p == point_mult #c (pk % getOrder #c) p)
+
+let lemma_scalar_reduce #c p pk = 
+  assert(point_mult pk p == repeat ((pk - 1) % getOrder #c) (fun x -> pointAdd #c p x) p);
+  assert(point_mult #c (pk % getOrder #c) p == repeat ((pk - 1) % getOrder #c % getOrder #c) (fun x -> pointAdd #c p x) p);
+  lemma_mod_twice (pk - 1) (getOrder #c)
+
+
+val point_mult_def: #c: curve -> i: int -> p: point_nat_prime #c -> Lemma 
+  (point_mult #c i p == repeat ((i - 1) % getOrder #c) (fun x -> pointAdd #c p x) p)
+
+let point_mult_def #c i p = ()
+
+#push-options "--z3rlimit 500"
+
+
+val lemma_commutativity_extended: #c: curve -> p0: point_nat_prime #c  -> a: point_nat_prime #c -> b: point_nat_prime #c -> 
+  Lemma (
+    let f = (fun x -> pointAdd #c p0 x) in 
+    pointEqual (pointAdd (f a) b) (pointAdd (f b) a))
+
+let lemma_commutativity_extended #c p0 a b = 
+  let f = (fun x -> pointAdd #c p0 x) in 
+  curve_commutativity_lemma (f b) a;
+  curve_commutativity_lemma (pointAdd a (pointAdd p0 b)) (pointAdd (pointAdd p0 b) a);
+  curve_commutativity_lemma p0 a; 
+  curve_compatibility_with_translation_lemma (pointAdd p0 a) (pointAdd a p0) b;
+  curve_associativity a p0 b
+  
+
+val lemma_point_add_minus_plus_same_value: #c: curve -> p0: point_nat_prime #c -> pk: nat -> qk: nat -> i: nat -> Lemma ( 
+  let p = pointAdd (point_mult pk p0) (point_mult qk p0) in 
+  let p_i = pointAdd (point_mult (pk - i) p0) (point_mult (qk + i) p0) in 
+  pointEqual p p_i)
+
+let rec lemma_point_add_minus_plus_same_value #curve p0 pk qk i = 
+   match i with 
+  |0 -> ()
+  | _ -> 
+    let o = getOrder #curve in  
+    let f = (fun x -> pointAdd #curve p0 x) in 
+    lemma_point_add_minus_plus_same_value #curve p0 pk qk (i - 1);
+    
+    let p = pointAdd (point_mult pk p0) (point_mult qk p0) in 
+  
+    let a = (point_mult (pk - i + 1) p0) in 
+    let b = (point_mult (qk + i - 1) p0) in 
+    let c = (point_mult (pk - i) p0) in 
+    let d = (point_mult (qk + i) p0) in 
+
+    let p_i1 = pointAdd (point_mult (pk - i + 1) p0) (point_mult (qk + i - 1) p0) in 
+    let p_i = pointAdd (point_mult (pk - i) p0) (point_mult (qk + i) p0) in  
+
+    point_mult_def (pk - i + 1) p0;
+    point_mult_def (pk - i) p0;
+    unfold_repeat o f p0 ((pk - i - 1) % o);
+
+    curve_point_at_infinity_property #curve p0;
+    curve_commutativity_lemma pointAtInfinity p0;
+
+    if ((pk - i - 1) % o + 1) < o then 
+      begin
+	small_mod (((pk - i - 1) % o + 1)) o;
+	lemma_mod_add_distr 1 (pk - i - 1) o;
+	assert(pointEqual a (f c))
+      end 
+    else begin
+      curve_multiplication_by_order #curve ((pk - i - 1) % o) p0;
+      lemma_mod_add_distr 1 (pk - i - 1) o;
+      eq_repeat0 f p0;
+      assert(pointEqual a (f c))
+    end;
+
+    point_mult_def (qk + i - 1) p0;
+    point_mult_def (qk + i) p0;
+    unfold_repeat o f p0 ((qk + i - 1 - 1) % o);
+
+    if ((qk + i - 1 - 1) % o + 1) < o then 
+      begin 
+	small_mod (((qk + i - 1 - 1) % o) + 1) o;
+	lemma_mod_add_distr 1 (qk + i - 2) o;
+	assert (pointEqual d (f b))
+      end
+    else begin 
+      curve_multiplication_by_order #curve ((qk + i - 1 - 1) % o) p0;
+      lemma_mod_add_distr 1 (qk + i - 1) o;
+      eq_repeat0 f p0;
+      assert (pointEqual d (f b))
+    end;
+
+    curve_compatibility_with_translation_lemma a (f c) b;
+    curve_compatibility_with_translation_lemma d (f b) c;
+    curve_commutativity_lemma #curve d c;
+
+    lemma_commutativity_extended p0 c b;
+    assert(pointEqual p_i1 p_i)
+
+
+val lemmaApplPointDouble: #c: curve 
+  -> p0: point_nat_prime #c 
+  -> pk: int
+  -> p: point_nat_prime #c {pointEqual p (point_mult pk p0)} ->
+  Lemma (pointEqual (pointAdd p p) (point_mult (2 * pk) p0))
+
+let lemmaApplPointDouble #c p0 pk p =  
+  let o = getOrder #c in 
+
+  let pk_p = point_mult pk p0 in 
+
+  lemma_point_add_minus_plus_same_value #c p0 (pk % o) (pk % o) ((pk - 1) % o);
+  lemma_scalar_reduce p0 pk;
+
+  calc (==) {
+    point_mult (pk % o - ((pk - 1) % o)) p0;
+    (==) {lemma_scalar_reduce p0 (pk % o - ((pk - 1) % o))}
+    point_mult ((pk % o - ((pk - 1) % o)) % o) p0;
+    (==) {lemma_mod_add_distr (- ((pk - 1) % o)) pk o}
+    point_mult ((pk - ((pk - 1) % o)) % o) p0;
+    (==) {lemma_mod_sub_distr pk (pk - 1) o}
+    point_mult ((pk - (pk - 1)) % o) p0;
+    (==) {lemma_scalar_reduce p0 (pk - (pk - 1))}
+    point_mult ((pk - (pk - 1))) p0;
+  };
+
+  calc (==) {
+    point_mult (pk % o + ((pk - 1) % o)) p0;
+    (==) {lemma_scalar_reduce p0 (pk % o + ((pk - 1) % o))}
+    point_mult ((pk % o + ((pk - 1) % o)) % o) p0;
+    (==) {lemma_mod_add_distr ((pk - 1) % o) pk o}
+    point_mult ((pk + ((pk - 1) % o)) % o) p0;
+    (==) {lemma_mod_add_distr pk (pk - 1) o}
+    point_mult ((pk + pk - 1) % o) p0;
+    (==) {lemma_scalar_reduce p0 (pk + pk - 1)}
+    point_mult ((pk + pk - 1)) p0;
+    
+  };
+    
+  point_mult_1 p0;
+  point_mult_ext (2 * pk - 1) p0;
+
+  curve_compatibility_with_translation_lemma p pk_p pk_p
+
+
+val lemmaApplPointAdd: #c: curve -> p0: point_nat_prime #c 
+  -> pk: int
+  -> p: point_nat_prime #c {pointEqual p (point_mult pk p0)} 
+  -> qk: int
+  -> q: point_nat_prime #c {pointEqual q (point_mult qk p0)} -> 
+  Lemma (pointEqual (pointAdd p q) (point_mult (pk + qk) p0))
+
+let lemmaApplPointAdd #c p0 pk p qk q = 
+  let pk_p = point_mult pk p0 in 
+  let qk_p = point_mult qk p0 in 
+  
+  let o = getOrder #c in 
+
+  lemma_point_add_minus_plus_same_value #c p0 (qk % o) (pk % o) ((qk - 1) % o);
+  lemma_scalar_reduce p0 qk;
+  lemma_scalar_reduce p0 pk;
+
+  assert(pointEqual (pointAdd (point_mult qk p0) (point_mult pk p0)) 
+    (pointAdd (point_mult ((qk % o) - ((qk - 1) % o)) p0) (point_mult (pk % o + ((qk - 1) % o)) p0)));
+
+  calc (==) {
+    point_mult ((qk % o) - ((qk - 1) % o)) p0;
+    (==) {lemma_scalar_reduce p0 ((qk % o) - ((qk - 1) % o))}
+    point_mult (((qk % o) - ((qk - 1) % o)) % o) p0;
+    (==) {lemma_mod_add_distr (- ((qk - 1) % o)) qk o}
+    point_mult ((qk - ((qk - 1) % o)) % o) p0;
+    (==) {lemma_mod_sub_distr qk (qk - 1) o}
+    point_mult ((qk - qk + 1) % o) p0;
+    (==) {lemma_scalar_reduce p0 1}
+    point_mult 1 p0;
+  };
+
+  calc (==) {
+    point_mult (pk % o + ((qk - 1) % o)) p0;
+    (==) {lemma_scalar_reduce p0 (pk % o + ((qk - 1) % o))}
+    point_mult ((pk % o + ((qk - 1) % o)) % o) p0;    
+    (==) {lemma_mod_add_distr ((qk - 1) % o) pk o}
+    point_mult ((pk + ((qk - 1) % o)) % o) p0;    
+    (==) {lemma_mod_add_distr pk (qk - 1) o}
+    point_mult ((pk + qk - 1) % o) p0;    
+    (==) {lemma_scalar_reduce p0 (pk + qk - 1)}
+    point_mult (pk + qk - 1) p0;  
+  };
+
+  point_mult_1 p0;
+  
+  point_mult_ext (pk + qk - 1) p0; 
+  curve_compatibility_with_translation_lemma p pk_p qk_p;
+  curve_compatibility_with_translation_lemma q qk_p p;
+   
+  curve_commutativity_lemma pk_p qk_p;
+  curve_commutativity_lemma p qk_p;
+  curve_commutativity_lemma q p
+
+
+
+val mlStep0AsPointAdd: #c: curve 
+  -> p0: point_nat_prime #c 
+  -> pk: nat
+  -> p: point_nat_prime #c {pointEqual p (point_mult #c pk p0)}  
+  -> qk: nat 
+  -> q: point_nat_prime #c {pointEqual q (point_mult #c qk p0)} -> 
+  Lemma
+  (ensures (
+    let p_i, q_i = _ml_step0 p q in 
+    pointEqual p_i (point_mult #c (pk + qk) p0) /\
+    pointEqual q_i (point_mult #c (2 * qk) p0)))
+
+
+let mlStep0AsPointAdd #c p0 p_k p q_k q = 
+  curve_commutativity_lemma p q; 
+  lemmaApplPointAdd p0 p_k p q_k q;
+  lemmaApplPointDouble p0 q_k q
+
+
+val mlStep1AsPointAdd: #c: curve
+  -> p0: point_nat_prime #c
+  -> pk: nat
+  -> p: point_nat_prime #c {pointEqual p (point_mult #c pk p0)} 
+  -> qk: nat 
+  -> q: point_nat_prime #c {pointEqual q (point_mult #c qk p0)} -> 
+  Lemma
+  (ensures (
+    let p_i, q_i = _ml_step1 p q in 
+    pointEqual q_i (point_mult (pk + qk) p0) /\ 
+    pointEqual p_i (point_mult (2 * pk) p0)))
+      
+let mlStep1AsPointAdd #c p0 pk p qk q = 
+  lemmaApplPointAdd p0 pk p qk q;
+  lemmaApplPointDouble p0 pk p
+
+
+val point_mult_0_lemma: #c: curve -> p: point_nat_prime #c ->  Lemma (point_mult 1 p == p)
+
+let point_mult_0_lemma #c p = 
+  Lib.LoopCombinators.eq_repeat0 (fun x -> pointAdd #c p x) p 
+
+
+val scalar_as_nat_: #c: curve -> scalar_bytes #c -> i: nat {i <= v (getScalarLen c)} -> nat
+
+let rec scalar_as_nat_ #c s i = 
+  if i = 0 then 0 else 
+  let bit = ith_bit s (v (getScalarLen c) - i) in 
+  scalar_as_nat_ #c s (i - 1) * 2 + uint_to_nat bit 
+
+#push-options "--fuel 1 --ifuel 1 --z3rlimit 100"
+
+val scalar_as_nat_zero: #c: curve -> s: scalar_bytes #c -> Lemma (scalar_as_nat_ s 0 == 0)
+
+let scalar_as_nat_zero #c s = ()
+
+
+val scalar_as_nat_def: #c: curve -> s: scalar_bytes #c -> i: nat {i > 0 /\ i <= v (getScalarLen c)} -> Lemma (
+  scalar_as_nat_ #c s i == 2 * scalar_as_nat_ #c s (i - 1) + uint_to_nat (ith_bit s (v (getScalarLen c) - i)))
+
+let scalar_as_nat_def #c s i = ()
+
+
+val scalar_as_nat: #c: curve -> scalar_bytes #c -> nat
+
+let scalar_as_nat #c s = scalar_as_nat_ #c s (v (getScalarLen c))
+
+
+
+val montgomery_ladder_spec_left: #c: curve -> s: scalar_bytes #c 
+  -> i: tuple2 (point_nat_prime #c) (point_nat_prime #c) {let i0, i1 = i in pointEqual i0 (point_mult #c 0 i1)} 
+  -> r: tuple2 (point_nat_prime #c) (point_nat_prime #c) {
+    let r0, r1 = r in let i0, i1 = i in
+    r == repeati (v (getScalarLen c)) (_ml_step #c s) i /\
+    pointEqual r0 (point_mult (scalar_as_nat #c s) i1)}
+
+
+val pred0: #c: curve -> x: tuple2 (point_nat_prime #c) (point_nat_prime #c) -> s: scalar_bytes ->
+  p: tuple2 (point_nat_prime #c) (point_nat_prime #c) -> i: nat {i < v (getScalarLen c)} ->
+  Lemma (
+    let f = _ml_step #c s in 
+    let pred i r =  
+      let p_i, q_i = r in 
+      let p0, q0 = p in 
+      let si = scalar_as_nat_ #c s i in 
+      let si1 = scalar_as_nat_ #c s i + 1 in
+      pointEqual p_i (point_mult #c si q0) /\ pointEqual q_i (point_mult #c si1 q0)  in 
+    (pred i x ==> pred (i + 1) (f i x))) 
+
+let pred0 #c x s p i =  (*
+      let pk = scalar_as_nat_ #c s i in 
+      assume (pointEqual p_i (point_mult pk p0));
+      assume (pointEqual q_i (point_mult (pk + 1) p0));
+      admit();
+      mlStep0AsPointAdd q0 pk p_i (pk + 1) q_i; admit();
+      mlStep1AsPointAdd q0 pk p_i (pk + 1) q_i; 
+      scalar_as_nat_def #c s (i + 1);  *) admit()
+
+
+val lemma_predicate0:  #c: curve ->  s: scalar_bytes 
+  -> p: tuple2 (point_nat_prime #c) (point_nat_prime #c) -> 
+  Lemma (
+    let f = _ml_step #c s in 
+    let pred i r =  
+      let p_i, q_i = r in 
+      let p0, q0 = p in 
+      let si = scalar_as_nat_ #c s i in 
+      let si1 = scalar_as_nat_ #c s i + 1 in
+      pointEqual p_i (point_mult #c si q0) /\ pointEqual q_i (point_mult #c si1 q0)  in 
+    forall (i:nat{i < v (getScalarLen c)}) (x: (tuple2 (point_nat_prime #c) (point_nat_prime #c))). 
+    pred i x ==> pred (i + 1) (f i x))
+
+let lemma_predicate0 #c s p = 
+  let pred = pred0 #c in
+  Classical.forall_intro_4 pred
+
+
+
+let montgomery_ladder_spec_left #c s (p0, q0) = 
+  let len : nat  = v (getScalarLen c) in 
+  
+  let pred i r = (
+    let p_i, q_i = r in 
+    let si = scalar_as_nat_ #c s i in 
+    let si1 = scalar_as_nat_ #c s i + 1 in
+    pointEqual p_i (point_mult #c si q0) /\
+    pointEqual q_i (point_mult #c si1 q0)) in
+    
+  let f = _ml_step #c s in 
+
+  lemma_predicate0 s (p0, q0);
+  point_mult_0_lemma #c q0;
+  repeati_inductive' #(tuple2 (point_nat_prime #c) (point_nat_prime #c)) len pred f (p0, q0)
+
+#pop-options
+
+
+val scalar_multiplication: #c: curve -> scalar_bytes #c -> 
+  p: point_nat_prime #c {~ (isPointAtInfinity p)} -> 
+  point_nat_prime #c 
+
+let scalar_multiplication #c k p =
+  point_mult_0 p 0; 
+  let q, f = montgomery_ladder_spec_left k (pointAtInfinity, p) in
+  _norm #c q
+
+val secret_to_public: #c: curve -> scalar_bytes #c -> point_nat_prime #c
+
+let secret_to_public #c k =
+  point_mult_0 (basePoint #c) 0;
+  let q, f = montgomery_ladder_spec_left #c k (pointAtInfinity, (basePoint #c)) in
+  _norm #c q
+
